
@prefix rdf: <http://www.w3.org/1999/02/22-rdf-syntax-ns#> .
@prefix rdfs: <http://www.w3.org/2000/01/rdf-schema#> .
@prefix owl: <http://www.w3.org/2002/07/owl#> .
@prefix sh: <http://www.w3.org/ns/shacl#> .
@prefix xs: <http://www.w3.org/2001/XMLSchema#> .
@prefix dcterms: <http://purl.org/dc/terms/> .
@prefix FMC: <http://fmc-modeling.org#> .
@prefix IREB: <https://cpre.ireb.org/en/downloads-and-resources/glossary#> .
@prefix ReqIF: <https://www.prostep.org/fileadmin/downloads/PSI_ImplementationGuide_ReqIF_V1-7.pdf#> .
@prefix ReqIF-WF: <https://www.prostep.org/fileadmin/downloads/Recommendation_ReqIF_V2_RZ3.pdf#> .
@prefix oslc_rm: <http://open-services.net/ns/rm#> .
@prefix pig: <https://product-information-graph.org/v0.2/metamodel#> .
@prefix SpecIF: <https://specif.de/v1.2/schema#> .
@prefix pigShapes_dcterms: <https://product-information-graph.org/v0.2/ontology/shapes/dcterms:#> .
@prefix pigShapes_rdfs: <https://product-information-graph.org/v0.2/ontology/shapes/rdfs:#> .
@prefix pigShapes_FMC: <https://product-information-graph.org/v0.2/ontology/shapes/FMC:#> .
@prefix pigShapes_IREB: <https://product-information-graph.org/v0.2/ontology/shapes/IREB:#> .
@prefix pigShapes_oslc_rm: <https://product-information-graph.org/v0.2/ontology/shapes/oslc_rm:#> .
@prefix pigShapes_ReqIF: <https://product-information-graph.org/v0.2/ontology/shapes/ReqIF:#> .
@prefix pigShapes_ReqIF-WF: <https://product-information-graph.org/v0.2/ontology/shapes/ReqIF-WF:#> .
@prefix pigShapes_SpecIF: <https://product-information-graph.org/v0.2/ontology/shapes/SpecIF:#> .
@prefix pigShapes_pig: <https://product-information-graph.org/v0.2/ontology/shapes/pig:#> .

@prefix o: <https://product-information-graph.org/v0.2/ontology#> .
@prefix d: <https://product-information-graph.org/examples/Dimmer.specifz#> .

#################################################################
# Project Metadata
#################################################################

d:
	rdf:type owl:Ontology ;
	rdfs:label "Dimmer - Semantically Integrated Specification (2021-01-28)" ;
	rdfs:comment "This specification method integrates and represents:\n- processes, system composition and requirements (dynamic, static and detail views)\n- mechanic, electric and software components with their interfaces.\n\nIt is important to understand, that all plans (diagrams) are views of a common system engineering model, sometimes called 'system repository'. Thus, consistency is always maintained.\n\nThe model elements are connected with relations, most of which are defined by positioning graph elements. For example, if a system component is drawn within another, a relationship 'contains' is created in the logic representation of the engineering model. Other relations, such as a system component 'satisfies' a requirement are created manually.  \n\nAlso, the documents are generated from the system engineering model. The ordering is in most projects (it can be rearranged, however, if appropriate):\n- All plans\n- A glossary with descriptions of all model elements appearing on one or more plans\n- A hierarchically ordered list of requirements\n- A list of open issues.\nPlease note that plans list related model elements and model elements list related requirements .. and vice versa. Active hyper-links are used, so that it is easy to jump between related model elements.\n\nFurther information is given in Appendix 'Method'." ;
	owl:imports <http://www.w3.org/1999/02/22-rdf-syntax-ns#> ,
		<http://www.w3.org/2000/01/rdf-schema#> ;
	dcterms:license <https://creativecommons.org/licenses/by-sa/4.0/> ;
	dcterms:creator "<mailto:od@enso-managers.de>" ;
	dcterms:modified "2026-01-17T22:39:33.066Z" .

#################################################################
# PIG Metamodel (pig:)
#################################################################

pig:Entity
	rdf:type owl:Class ;
	rdfs:label "Entity" ;
	rdfs:comment "A PIG meta-model element used for entities (aka resources or artifacts)." .

pigShapes_pig:Entity
	rdf:type sh:NodeShape ;
	sh:targetClass pig:Entity ;
	sh:property pigShapes_rdfs:label ,
		pigShapes_rdfs:comment ,
		pigShapes_pig:category ,
		pigShapes_pig:icon .

pig:Organizer
	rdfs:subClassOf pig:Entity ;
	rdfs:label "Organizer" ;
	rdfs:comment "An element organizing model elements. An example is a list of requirements or a diagram using a certain notation." .

pigShapes_pig:Organizer
	rdf:type sh:NodeShape ;
	sh:targetClass pig:Organizer ;
	sh:property pigShapes_rdfs:label ,
		pigShapes_rdfs:comment ,
		pigShapes_pig:category .

pig:HierarchyRoot
	rdfs:subClassOf pig:Organizer ;
	rdfs:label "Hierarchy Root" ;
	rdfs:comment "A subclass of PIG organizer serving as a root for hierarchically organized graph elements." .

pigShapes_pig:HierarchyRoot
	rdf:type sh:NodeShape ;
	sh:targetClass pig:HierarchyRoot ;
	sh:property pigShapes_rdfs:label ,
		pigShapes_rdfs:comment ,
		pigShapes_pig:lists .

pig:Outline
	rdfs:subClassOf pig:Organizer ;
	rdfs:label "Outline" ;
	rdfs:comment "A subclass of PIG organizer comprising all information items of a human-readable document. As usual, the outline is hierarchically organized." .

pigShapes_pig:Outline
	rdf:type sh:NodeShape ;
	sh:targetClass pig:Outline ;
	sh:property pigShapes_rdfs:label ,
		pigShapes_rdfs:comment ,
		pigShapes_pig:category ,
		pigShapes_pig:lists .

pig:View
	rdfs:subClassOf pig:Organizer ;
	rdfs:label "View" ;
	rdfs:comment "A subclass of PIG organizer representing a model view (diagram) using a certain notation showing selected model elements." .

pigShapes_pig:View
	rdf:type sh:NodeShape ;
	sh:targetClass pig:View ;
	sh:property pigShapes_rdfs:label ,
		pigShapes_rdfs:comment ,
		pigShapes_pig:category ,
		pigShapes_pig:icon ,
		pigShapes_pig:shows ,
		pigShapes_pig:depicts .

pig:Relationship
	rdf:type owl:Class ;
	rdfs:label "Relationship" ;
	rdfs:comment "A PIG meta-model element used for reified relationships (aka predicates)." .

pigShapes_pig:Relationship
	rdf:type sh:NodeShape ;
	sh:targetClass pig:Relationship ;
	sh:property pigShapes_rdfs:label ,
		pigShapes_rdfs:comment ,
		pigShapes_pig:category ,
		pigShapes_pig:icon ,
		pigShapes_pig:SourceLink ,
		pigShapes_pig:TargetLink .

pig:Property
	rdf:type owl:DatatypeProperty ;
	rdfs:label "Property" ;
	rdfs:comment "A PIG meta-model element used for properties (aka attributes)." .

pigShapes_pig:Property
	rdf:type sh:PropertyShape ;
	sh:path pig:Property ;
	sh:datatype xs:anyType .

pig:icon
	rdfs:subPropertyOf pig:Property ;
	rdfs:label "has icon" ;
	rdfs:comment "Specifies an icon for a model element (entity or relationship)." .

pigShapes_pig:icon
	rdf:type sh:PropertyShape ;
	sh:path pig:icon ;
	sh:datatype xs:string ;
	sh:minCount "0" ;
	sh:maxCount "1" .

pig:category
	rdfs:subPropertyOf dcterms:type ;
	rdfs:label "has category" ;
	rdfs:comment "Specifies a category for an element (entity, relationship or organizer)." .

pigShapes_pig:category
	rdf:type sh:PropertyShape ;
	sh:path pig:category ;
	sh:datatype xs:string ;
	sh:maxLength "32" ;
	sh:minCount "0" ;
	sh:maxCount "1" .

pig:Link
	rdf:type owl:ObjectProperty ;
	rdfs:range [ owl:unionOf(
			pig:Entity
			pig:Relationship
		)] ;
	rdfs:label "linked with" ;
	rdfs:comment "Connects a reified relationship with its source or target. Also connects an organizer to a model element" .

pigShapes_pig:Link
	rdf:type sh:PropertyShape ;
	sh:path pig:Link ;
	sh:or (
			[ sh:class pig:Entity ]
			[ sh:class pig:Relationship ]
		) .

pig:SourceLink
	rdfs:subPropertyOf pig:Link ;
	rdfs:range [ owl:unionOf(
			pig:Entity
			pig:Relationship
		)] ;
	rdfs:label "to source" ;
	rdfs:comment "Connects the source of a reified relationship." .

pigShapes_pig:SourceLink
	rdf:type sh:PropertyShape ;
	sh:path pig:SourceLink ;
	sh:or (
			[ sh:class pig:Entity ]
			[ sh:class pig:Relationship ]
		) .

pig:TargetLink
	rdfs:subPropertyOf pig:Link ;
	rdfs:range [ owl:unionOf(
			pig:Entity
			pig:Relationship
		)] ;
	rdfs:label "to target" ;
	rdfs:comment "Connects the target of a reified relationship or an organizer." .

pigShapes_pig:TargetLink
	rdf:type sh:PropertyShape ;
	sh:path pig:TargetLink ;
	sh:or (
			[ sh:class pig:Entity ]
			[ sh:class pig:Relationship ]
		) .

pig:lists
	rdfs:subPropertyOf pig:TargetLink ;
	rdfs:range [ owl:unionOf(
			pig:Entity
			pig:Relationship
			pig:Organizer
		)] ;
	rdfs:label "lists" ;
	rdfs:comment "Lists an entity, a relationship or a subordinated organizer." .

pigShapes_pig:lists
	rdf:type sh:PropertyShape ;
	sh:path pig:lists ;
	sh:or (
			[ sh:class pig:Entity ]
			[ sh:class pig:Relationship ]
			[ sh:class pig:Organizer ]
		) .

pig:shows
	rdfs:subPropertyOf pig:TargetLink ;
	rdfs:range [ owl:unionOf(
			pig:Entity
			pig:Relationship
		)] ;
	rdfs:label "shows" ;
	rdfs:comment "Shows an entity or a relationship." .

pigShapes_pig:shows
	rdf:type sh:PropertyShape ;
	sh:path pig:shows ;
	sh:or (
			[ sh:class pig:Entity ]
			[ sh:class pig:Relationship ]
		) .

pig:depicts
	rdfs:subPropertyOf pig:TargetLink ;
	rdfs:range pig:Entity ;
	rdfs:label "depicts" ;
	rdfs:comment "Depicts an entity; inverse of uml:ownedDiagram." .

pigShapes_pig:depicts
	rdf:type sh:PropertyShape ;
	sh:path pig:depicts ;
	sh:or (
			[ sh:class pig:Entity ]
		) .

#################################################################
# Data Types with Enumerated Values
#################################################################

SpecIF:LifecycleStatus-Value
	rdf:type owl:Class ;
	rdfs:label "Lifecycle"@en ,
		"Lebenszyklus"@de ,
		"Cycle de vie"@fr ;
	rdfs:comment "The 'Lifecycle Status' of the resource."@en ,
		"Der 'Lebenszyklusstatus' der Ressource."@de ,
		"L'état du cycle de vie de la ressource."@fr ;
	owl:oneOf (
			SpecIF:LifecycleStatusDeprecated
			SpecIF:LifecycleStatusRejected
			SpecIF:LifecycleStatusInitial
			SpecIF:LifecycleStatusDrafted
			SpecIF:LifecycleStatusSubmitted
			SpecIF:LifecycleStatusApproved
			SpecIF:LifecycleStatusDone
			SpecIF:LifecycleStatusReleased
		) .
SpecIF:LifecycleStatusDeprecated
	rdf:type SpecIF:LifecycleStatus-Value ;
	rdfs:label "deprecated"@en ,
		"veraltet"@de ,
		"dépassé"@fr .
SpecIF:LifecycleStatusRejected
	rdf:type SpecIF:LifecycleStatus-Value ;
	rdfs:label "rejected"@en ,
		"abgelehnt"@de ,
		"rejeté"@fr .
SpecIF:LifecycleStatusInitial
	rdf:type SpecIF:LifecycleStatus-Value ;
	rdfs:label "initial"@en .
SpecIF:LifecycleStatusDrafted
	rdf:type SpecIF:LifecycleStatus-Value ;
	rdfs:label "drafted"@en ,
		"entworfen"@de ,
		"rédigé"@fr .
SpecIF:LifecycleStatusSubmitted
	rdf:type SpecIF:LifecycleStatus-Value ;
	rdfs:label "submitted"@en ,
		"vorgelegt"@de ,
		"soumis"@fr .
SpecIF:LifecycleStatusApproved
	rdf:type SpecIF:LifecycleStatus-Value ;
	rdfs:label "approved"@en ,
		"genehmigt"@de ,
		"approuvé"@fr .
SpecIF:LifecycleStatusDone
	rdf:type SpecIF:LifecycleStatus-Value ;
	rdfs:label "done"@en ,
		"erledigt ('done')"@de .
SpecIF:LifecycleStatusReleased
	rdf:type SpecIF:LifecycleStatus-Value ;
	rdfs:label "released"@en ,
		"freigegeben"@de ,
		"publié"@fr .

SpecIF:Priority-Value
	rdf:type owl:Class ;
	rdfs:label "Priority"@en ,
		"Priorität"@de ,
		"Priorité"@fr ;
	rdfs:comment "Enumerated values for the 'Priority' of the resource."@en ;
	owl:oneOf (
			SpecIF:priorityHigh
			SpecIF:priorityMedium
			SpecIF:priorityLow
		) .
SpecIF:priorityHigh
	rdf:type SpecIF:Priority-Value ;
	rdfs:label "high"@en ,
		"hoch"@de ,
		"haut"@fr .
SpecIF:priorityMedium
	rdf:type SpecIF:Priority-Value ;
	rdfs:label "medium"@en ,
		"mittel"@de ,
		"moyen"@fr .
SpecIF:priorityLow
	rdf:type SpecIF:Priority-Value ;
	rdfs:label "low"@en ,
		"niedrig"@de ,
		"bas"@fr .

SpecIF:StakeholderGroup-Value
	rdf:type owl:Class ;
	rdfs:label "Stakeholder Group"@en ;
	rdfs:comment "Enumerated values for the 'Stakehoder Group' addressed by the term."@en ;
	owl:oneOf (
			SpecIF:StakeholderGroupBusiness
			SpecIF:StakeholderGroupUser
			SpecIF:StakeholderGroupSystem
		) .
SpecIF:StakeholderGroupBusiness
	rdf:type SpecIF:StakeholderGroup-Value ;
	rdfs:label "Business"@en .
SpecIF:StakeholderGroupUser
	rdf:type SpecIF:StakeholderGroup-Value ;
	rdfs:label "User"@en .
SpecIF:StakeholderGroupSystem
	rdf:type SpecIF:StakeholderGroup-Value ;
	rdfs:label "System"@en .

SpecIF:EngineeringDiscipline-Value
	rdf:type owl:Class ;
	rdfs:label "Engineering Discipline"@en ,
		"Ingenieurdisziplin"@de ,
		"Discipline d'ingénierie"@fr ;
	rdfs:comment "The engineering discipline involved by a development artefact."@en ;
	owl:oneOf (
			SpecIF:EngineeringDisciplineMechanics
			SpecIF:EngineeringDisciplineElectronics
			SpecIF:EngineeringDisciplineSoftware
			SpecIF:EngineeringDisciplineSafety
		) .
SpecIF:EngineeringDisciplineMechanics
	rdf:type SpecIF:EngineeringDiscipline-Value ;
	rdfs:label "Mechanics"@en ,
		"Mechanik"@de ,
		"Mecanique"@fr .
SpecIF:EngineeringDisciplineElectronics
	rdf:type SpecIF:EngineeringDiscipline-Value ;
	rdfs:label "Electronics"@en ,
		"Elektronik"@de ,
		"Électronique"@fr .
SpecIF:EngineeringDisciplineSoftware
	rdf:type SpecIF:EngineeringDiscipline-Value ;
	rdfs:label "Software"@en ,
		"Logiciel"@fr .
SpecIF:EngineeringDisciplineSafety
	rdf:type SpecIF:EngineeringDiscipline-Value ;
	rdfs:label "Safety"@en ,
		"Sicherheit"@de ,
		"Sécurité"@fr .

ReqIF-WF:SupplierStatus-Value
	rdf:type owl:Class ;
	rdfs:label "Supplier Status"@en ,
		"Zustand Lieferant"@de ,
		"Statut coté Fournisseur"@fr ;
	owl:oneOf (
			SpecIF:NotApplicable
			ReqIF-WF:CustomerStatus.ToBeClarified
			ReqIF-WF:SupplierStatus.Agreed
			ReqIF-WF:SupplierStatus.AgreedWithComment
			ReqIF-WF:SupplierStatus.NotAgreed
		) .
SpecIF:NotApplicable
	rdf:type ReqIF-WF:SupplierStatus-Value ;
	rdfs:label "not applicable"@en ,
		"nicht anwendbar"@de ,
		"sans objet"@fr .
ReqIF-WF:CustomerStatus.ToBeClarified
	rdf:type ReqIF-WF:SupplierStatus-Value ;
	rdfs:label "to be clarified"@en ,
		"zu klären"@de ,
		"à préciser"@fr .
ReqIF-WF:SupplierStatus.Agreed
	rdf:type ReqIF-WF:SupplierStatus-Value ;
	rdfs:label "agreed"@en ,
		"zugestimmt"@de ,
		"approuvé"@fr .
ReqIF-WF:SupplierStatus.AgreedWithComment
	rdf:type ReqIF-WF:SupplierStatus-Value ;
	rdfs:label "agreed with comment"@en ,
		"zugestimmt mit Kommentar"@de ,
		"approuvé avec commentaire"@fr .
ReqIF-WF:SupplierStatus.NotAgreed
	rdf:type ReqIF-WF:SupplierStatus-Value ;
	rdfs:label "not agreed"@en ,
		"nicht zugestimmt"@de ,
		"non approuvé"@fr .

ReqIF-WF:CustomerStatus-Value
	rdf:type owl:Class ;
	rdfs:label "Customer Status"@en ,
		"Zustand Kunde"@de ,
		"Statut coté Client"@fr ;
	owl:oneOf (
			ReqIF-WF:CustomerStatus.NotToEvaluate
			ReqIF-WF:CustomerStatus.ToEvaluate
			ReqIF-WF:CustomerStatus.Accepted
			ReqIF-WF:CustomerStatus.NotAccepted
		) .
ReqIF-WF:CustomerStatus.NotToEvaluate
	rdf:type ReqIF-WF:CustomerStatus-Value ;
	rdfs:label "not to evaluate"@en ,
		"nicht zu evaluieren"@de ,
		"ne pas évaluer"@fr .
ReqIF-WF:CustomerStatus.ToEvaluate
	rdf:type ReqIF-WF:CustomerStatus-Value ;
	rdfs:label "to evaluate"@en ,
		"zu evaluieren"@de ,
		"pour évaluer"@fr .
ReqIF-WF:CustomerStatus.Accepted
	rdf:type ReqIF-WF:CustomerStatus-Value ;
	rdfs:label "accepted"@en ,
		"akzeptiert"@de ,
		"accepté"@fr .
ReqIF-WF:CustomerStatus.NotAccepted
	rdf:type ReqIF-WF:CustomerStatus-Value ;
	rdfs:label "not accepted"@en ,
		"nicht akzeptiert"@de ,
		"non accepté"@fr .

o:DT-IssueStatus
	rdf:type owl:Class ;
	rdfs:label "SpecIF:LifecycleStatusIssue" ;
	rdfs:comment "Enumerated values for issue status" ;
	owl:oneOf (
			o:V-Iss-Status-0
			o:V-Iss-Status-1
			o:V-Iss-Status-2
			oslc_cm:Inprogress
			oslc_cm:Closed
			o:V-Iss-Status-5
			o:V-Iss-Status-6
		) .
o:V-Iss-Status-0
	rdf:type o:DT-IssueStatus ;
	rdfs:label "undefined" .
o:V-Iss-Status-1
	rdf:type o:DT-IssueStatus ;
	rdfs:label "open" .
o:V-Iss-Status-2
	rdf:type o:DT-IssueStatus ;
	rdfs:label "assigned" .
oslc_cm:Inprogress
	rdf:type o:DT-IssueStatus ;
	rdfs:label "in progress"@en .
oslc_cm:Closed
	rdf:type o:DT-IssueStatus ;
	rdfs:label "closed"@en .
o:V-Iss-Status-5
	rdf:type o:DT-IssueStatus ;
	rdfs:label "reopened" .
o:V-Iss-Status-6
	rdf:type o:DT-IssueStatus ;
	rdfs:label "SpecIF:LifecycleStatusRejected" .

#################################################################
# Ontology - Property Classes
#################################################################

# Skipping implicit property: rdfs:label

# Skipping implicit property: rdfs:comment

SpecIF:Diagram
	rdf:type owl:DatatypeProperty ;
	rdfs:label "Diagram"@en ,
		"Diagramm"@de ,
		"Diagramme"@fr ;
	rdfs:comment "A diagram illustrating the resource or a link to a diagram."@en .

pigShapes_SpecIF:Diagram
	rdf:type sh:PropertyShape ;
	sh:path SpecIF:Diagram ;
	sh:datatype xs:string .

# Skipping implicit property: pig:category

SpecIF:Notation
	rdf:type owl:DatatypeProperty ;
	rdfs:label "Notation"@en ;
	rdfs:comment "The notation used by a model diagram, e.g. 'BPMN 2.0', 'SysML Activity Diagram' or 'FMC Block Diagram'."@en .

pigShapes_SpecIF:Notation
	rdf:type sh:PropertyShape ;
	sh:path SpecIF:Notation ;
	sh:maxCount "1" ;
	sh:datatype xs:string ;
	sh:maxLength "256" .

SpecIF:Priority
	rdf:type owl:ObjectProperty ;
	rdfs:label "Priority"@en ,
		"Priorität"@de ,
		"Priorité"@fr ;
	rdfs:comment "Enumerated values for the 'Priority' of the resource."@en ;
	rdfs:range SpecIF:Priority-Value .

pigShapes_SpecIF:Priority
	rdf:type sh:PropertyShape ;
	sh:path SpecIF:Priority ;
	sh:maxCount "1" ;
	sh:class SpecIF:Priority-Value .

SpecIF:LifecycleStatus
	rdf:type owl:ObjectProperty ;
	rdfs:label "Lifecycle"@en ,
		"Lebenszyklus"@de ,
		"Cycle de vie"@fr ;
	rdfs:comment "The 'Lifecycle Status' of the resource."@en ,
		"Der 'Lebenszyklusstatus' der Ressource."@de ,
		"L'état du cycle de vie de la ressource."@fr ;
	rdfs:range SpecIF:LifecycleStatus-Value .

pigShapes_SpecIF:LifecycleStatus
	rdf:type sh:PropertyShape ;
	sh:path SpecIF:LifecycleStatus ;
	sh:maxCount "1" ;
	sh:class SpecIF:LifecycleStatus-Value .

ReqIF-WF:SupplierStatus
	rdf:type owl:ObjectProperty ;
	rdfs:label "Supplier Status"@en ,
		"Zustand Lieferant"@de ,
		"Statut coté Fournisseur"@fr ;
	rdfs:range ReqIF-WF:SupplierStatus-Value .

pigShapes_ReqIF-WF:SupplierStatus
	rdf:type sh:PropertyShape ;
	sh:path ReqIF-WF:SupplierStatus ;
	sh:maxCount "1" ;
	sh:class ReqIF-WF:SupplierStatus-Value .

ReqIF-WF:SupplierComment
	rdf:type owl:DatatypeProperty ;
	rdfs:label "Supplier Comment"@en ,
		"Kommentar Lieferant"@de ,
		"Commentaire du Client"@fr .

pigShapes_ReqIF-WF:SupplierComment
	rdf:type sh:PropertyShape ;
	sh:path ReqIF-WF:SupplierComment ;
	sh:maxCount "1" ;
	sh:datatype xs:string .

ReqIF-WF:CustomerStatus
	rdf:type owl:ObjectProperty ;
	rdfs:label "Customer Status"@en ,
		"Zustand Kunde"@de ,
		"Statut coté Client"@fr ;
	rdfs:range ReqIF-WF:CustomerStatus-Value .

pigShapes_ReqIF-WF:CustomerStatus
	rdf:type sh:PropertyShape ;
	sh:path ReqIF-WF:CustomerStatus ;
	sh:maxCount "1" ;
	sh:class ReqIF-WF:CustomerStatus-Value .

ReqIF-WF:CustomerComment
	rdf:type owl:DatatypeProperty ;
	rdfs:label "Customer Comment"@en ,
		"Kommentar Kunde"@de ,
		"Commentaire du Client"@fr .

pigShapes_ReqIF-WF:CustomerComment
	rdf:type sh:PropertyShape ;
	sh:path ReqIF-WF:CustomerComment ;
	sh:maxCount "1" ;
	sh:datatype xs:string .

dcterms:identifier
	rdf:type owl:DatatypeProperty ;
	rdfs:label "Identifier"@en ,
		"Bezeichner"@de ,
		"Identifiant"@fr ;
	rdfs:comment "<p>A unique reference to the resource within a given context. <small>(<i>source: <a href=\"http://purl.org/dc/elements/1.1/identifier\">DCMI</a></i>)</small></p><p>An identifier for a resource. This identifier may be unique with a scope that is defined by the RM provider. Assigned by the service provider when a resource is created. Not intended for end-user display. <small>(<i>source: <a href=\"http://open-services.net/\">OSLC</a></i>)</small></p>"@en .

pigShapes_dcterms:identifier
	rdf:type sh:PropertyShape ;
	sh:path dcterms:identifier ;
	sh:maxCount "1" ;
	sh:datatype xs:string ;
	sh:maxLength "256" .

SpecIF:StakeholderGroup
	rdf:type owl:ObjectProperty ;
	rdfs:label "Stakeholder Group"@en ;
	rdfs:comment "Enumerated values for the 'Stakehoder Group' addressed by the term."@en ;
	rdfs:range SpecIF:StakeholderGroup-Value .

pigShapes_SpecIF:StakeholderGroup
	rdf:type sh:PropertyShape ;
	sh:path SpecIF:StakeholderGroup ;
	sh:maxCount "1" ;
	sh:class SpecIF:StakeholderGroup-Value .

SpecIF:EngineeringDiscipline
	rdf:type owl:ObjectProperty ;
	rdfs:label "Engineering Discipline"@en ,
		"Ingenieurdisziplin"@de ,
		"Discipline d'ingénierie"@fr ;
	rdfs:comment "The engineering discipline involved by a development artefact."@en ;
	rdfs:range SpecIF:EngineeringDiscipline-Value .

pigShapes_SpecIF:EngineeringDiscipline
	rdf:type sh:PropertyShape ;
	sh:path SpecIF:EngineeringDiscipline ;
	sh:class SpecIF:EngineeringDiscipline-Value .

o:PC-IssueStatus
	rdf:type owl:ObjectProperty ;
	rdfs:label "SpecIF:LifecycleStatusIssue" ;
	rdfs:range o:DT-IssueStatus .

o:PC-IssueStatus_shape
	rdf:type sh:PropertyShape ;
	sh:path o:PC-IssueStatus ;
	sh:maxCount "1" ;
	sh:class o:DT-IssueStatus .

SpecIF:Responsible
	rdf:type owl:DatatypeProperty ;
	rdfs:label "Responsible"@en ,
		"Verantwortliche(r)"@de ,
		"Responsable"@fr ;
	rdfs:comment "The 'Person' being responsible for the resource."@en .

pigShapes_SpecIF:Responsible
	rdf:type sh:PropertyShape ;
	sh:path SpecIF:Responsible ;
	sh:maxCount "1" ;
	sh:datatype xs:string ;
	sh:maxLength "256" .

SpecIF:DueDate
	rdf:type owl:DatatypeProperty ;
	rdfs:label "Due Date"@en ,
		"Termin"@de ,
		"Date limite"@fr ;
	rdfs:comment "A 'Due Date' for the resource."@en .

pigShapes_SpecIF:DueDate
	rdf:type sh:PropertyShape ;
	sh:path SpecIF:DueDate ;
	sh:maxCount "1" ;
	sh:datatype xs:dateTime .

#################################################################
# Ontology - Entity Classes
#################################################################

SpecIF:Paragraph
	rdfs:subClassOf pig:Entity ;
	rdfs:label "Paragraph"@en ,
		"Textabsatz"@de ,
		"Paragraphe"@fr ;
	rdfs:comment "<p>A 'Paragraph' is an unspecified information in a document at any level.</p>"@en ,
		"<p>Ein 'Textabschnitt' in einem Dokument auf beliebiger Ebene.</p>"@de .

pigShapes_SpecIF:Paragraph
	rdf:type sh:NodeShape ;
	sh:targetClass SpecIF:Paragraph ;
	sh:property pigShapes_rdfs:label ,
		pigShapes_rdfs:comment ,
		pigShapes_SpecIF:Diagram ,
		pigShapes_pig:category .

FMC:Actor
	rdfs:subClassOf pig:Entity ;
	rdfs:label "Actor"@en ,
		"Akteur"@de ,
		"Acteur"@fr ;
	rdfs:comment "<p>An 'Actor' is a fundamental model element type representing an active entity, be it an activity, a process step, a function, a system component or a role.</p><p>The  particular use or original type is specified with a [[dcterms:type]] property of the 'FMC:Actor'. A value of that property should be an ontology-term, such as [[bpmn:processStep]].</p>"@en ,
		"<p>Ein 'Akteur' ist ein fundamentaler Modellelementtyp, der eine aktive Entität darstellt, sei es eine Aktivität, ein Prozessschritt, eine Funktion, eine Systemkomponente oder eine Rolle.</p><p>Die spezielle Verwendung oder der ursprüngliche Typ wird mit einer [[dcterms:type]] Eigenschaft von 'FMC:Actor' spezifiziert. Die Werte dieser Eigenschaft können Ontologiebegriffe sein, wie z.B. [[bpmn:timer]].</p>"@de ,
		"<p>Un 'Acteur' est un type d'élément de modèle fondamental représentant une entité active, qu'il s'agisse d'une activité, d'une étape de processus, d'une fonction, d'un composant de système ou d'un rôle.</p><p>L'utilisation particulière ou le type original est spécifié avec une propriété [[dcterms:type]] de 'FMC:Actor'. Les valeurs de cette propriété peuvent être des termes d'ontologie, tels que [[bpmn:timer]].</p>"@fr ;
	pig:icon "&#x25A1;" .

pigShapes_FMC:Actor
	rdf:type sh:NodeShape ;
	sh:targetClass FMC:Actor ;
	sh:property pigShapes_rdfs:label ,
		pigShapes_rdfs:comment ,
		pigShapes_SpecIF:Diagram .

FMC:State
	rdfs:subClassOf pig:Entity ;
	rdfs:label "State"@en ,
		"Zustand"@de ,
		"État"@fr ;
	rdfs:comment "<p>A 'State' is a fundamental model element type representing a passive entity, be it a value, a condition, an information storage or even a physical shape.</p><p>The particular use or the original type is specified with a [[dcterms:type]] property of the 'FMC:State'. A value of that property should bean  ontology-term, such as [[bpmn:dataObject]].</p>"@en ,
		"<p>Ein 'Zustand' ist ein fundamentaler Modellelementtyp, der eine passive Entität darstellt, sei es ein Wert, ein Dokument, ein Informationsspeicher, eine Bedingung oder eine physische Beschaffenheit.</p><p>Die spezielle Verwendung oder der ursprüngliche Typ wird mit einer [[dcterms:type]] Eigenschaft von 'FMC:State' spezifiziert. Die Werte dieser Eigenschaft können Ontologiebegriffe sein, wie z.B. [[ArchiMate:DataObject]].</p>"@de ,
		"<p>Un 'État' est un type d'élément de modèle fondamental représentant une entité passive, qu'il s'agisse d'une valeur, d'une condition, d'un stockage d'informations ou même d'une forme physique.</p><p>L'utilisation particulière ou le type original est spécifié avec une propriété [[dcterms:type]] de 'FMC:State'. Les valeurs de cette propriété peuvent être des termes d'ontologie, tels que [[ArchiMate:DataObject]].</p>"@fr ;
	pig:icon "&#x25CB;" .

pigShapes_FMC:State
	rdf:type sh:NodeShape ;
	sh:targetClass FMC:State ;
	sh:property pigShapes_rdfs:label ,
		pigShapes_rdfs:comment .

FMC:Event
	rdfs:subClassOf pig:Entity ;
	rdfs:label "Event"@en ,
		"Ereignis"@de ,
		"Évenement"@fr ;
	rdfs:comment "<p>An 'Event' is a fundamental model element type representing a time reference, a change in condition/value or more generally a synchronization primitive.</p><p>The particular use or the original type is specified with a [[dcterms:type]] property of the 'FMC:Event'. A value of that property should be an ontology-term, such as [[bpmn:startEvent]].</p>"@en ,
		"<p>Ein 'Ereignis' ist ein fundamentaler Modellelementtyp, der eine Zeitreferenz, eine Änderung einer Bedingung/eines Wertes oder allgemeiner ein Synchronisationsmittel darstellt.</p><p>Die spezielle Verwendung oder der ursprüngliche Typ wird mit einer [[dcterms:type]] Eigenschaft von 'FMC:Event' spezifiziert. Die Werte dieser Eigenschaft sollen Ontologiebegriffe sein, wie z.B. [[bpmn:startEvent]].</p>"@de ,
		"<p>Un 'Événement' est un type d'élément de modèle fondamental représentant une référence temporelle, un changement de condition/valeur ou plus généralement une primitive de synchronisation.</p><p>L'utilisation particulière ou le type original est spécifié avec une propriété [[dcterms:type]] de 'FMC:Event'. Les valeurs de cette propriété peuvent être des termes d'ontologie, tels que [[bpmn:startEvent]].</p>"@fr ;
	pig:icon "&#x2662;" .

pigShapes_FMC:Event
	rdf:type sh:NodeShape ;
	sh:targetClass FMC:Event ;
	sh:property pigShapes_rdfs:label ,
		pigShapes_rdfs:comment .

IREB:Requirement
	rdfs:subClassOf pig:Entity ;
	rdfs:label "Requirement"@en ,
		"Anforderung"@de ,
		"Exigence"@fr ;
	rdfs:comment "<p>A 'Requirement' is a singular documented physical and functional need that a particular design, product or process must be able to perform. <small>(<i>source: <a href=\"https://en.wikipedia.org/wiki/Requirement\">Wikipedia</a></i>)</small></p><p>Definition:</p><ol><li>A condition or capability needed by a user to solve a problem or achieve an objective.</li><li>A condition or capability that must be met or possessed by a system or system component to satisfy a contract, standard, specification, or other formally imposed documents.</li><li>A documented representation of a condition or capability as in (1) or (2).</li></ol><p>Note: The definition above is the classic one from IEEE Std 610.12 of 1990. Alternatively, we also give a more modern definition:</p><ol><li>A need perceived by a stakeholder.</li><li>A capability or property that a system shall have.</li><li>A documented representation of a need, capability or property.</li></ol>"@en ,
		"<p>Eine 'Anforderung' ist ein einzelnes dokumentiertes physisches und funktionales Bedürfnis, das ein bestimmter Entwurf, ein Produkt oder ein Prozess erfüllen muss. <small>(<i>source: <a href=\"https://en.wikipedia.org/wiki/Requirement\">Wikipedia</a></i>)</small></p><p>Definition:</p><ol><li>Eine Bedingung oder Fähigkeit, die ein Benutzer benötigt, um ein Problem zu lösen oder ein Ziel zu erreichen.</li><li>Eine Bedingung oder Fähigkeit, die ein System oder eine Systemkomponente erfüllen oder besitzen muss, um einen Vertrag, eine Norm, eine Spezifikation oder ein anderes formal vorgeschriebenes Dokument zu erfüllen.</li><li>Eine dokumentierte Darstellung einer Bedingung oder Fähigkeit wie in (1) oder (2).</li></ol><p>Anmerkung: Die obige Definition ist die klassische Definition aus IEEE Std 610.12 von 1990. Alternativ geben wir auch eine modernere Definition an:</p><ol><li>Ein von einem Stakeholder wahrgenommener Bedarf.</li><li>Eine Fähigkeit oder Eigenschaft, die ein System haben soll.</li><li>Eine dokumentierte Darstellung eines Bedarfs, einer Fähigkeit oder Eigenschaft.</li></ol>"@de ,
		"<p>Une 'Exigence' est un besoin physique et fonctionnel unique et documenté qu'une conception, un produit ou un processus particulier doit pouvoir satisfaire. <small>(<i>source: <a href=\"https://en.wikipedia.org/wiki/Requirement\">Wikipedia</a></i>)</small></p><p>Définition:</p><ol><li>Condition ou capacité dont un utilisateur a besoin pour résoudre un problème ou atteindre un objectif.</li><li>Condition ou capacité qui doit être remplie ou possédée par un système ou un composant de système pour satisfaire à un contrat, à une norme, à une spécification ou à d'autres documents imposés officiellement.</li><li>Une représentation documentée d'une condition ou d'une capacité comme dans (1) ou (2).</li></ol><p>Remarque: La définition ci-dessus est la définition classique de la norme IEEE 610.12 de 1990. Nous donnons également une définition plus moderne:</p><ol><li>Un besoin perçu par une partie prenante;</li><li>Une capacité ou une propriété qu'un système doit avoir.</li><li>Une représentation documentée d'un besoin, d'une capacité ou d'une propriété.</li></ol>"@fr ;
	pig:icon "&#8623;" .

pigShapes_IREB:Requirement
	rdf:type sh:NodeShape ;
	sh:targetClass IREB:Requirement ;
	sh:property pigShapes_dcterms:identifier ,
		pigShapes_rdfs:label ,
		pigShapes_rdfs:comment ,
		pigShapes_SpecIF:LifecycleStatus ,
		pigShapes_SpecIF:Priority ,
		pigShapes_SpecIF:StakeholderGroup ,
		pigShapes_SpecIF:EngineeringDiscipline ,
		pigShapes_ReqIF-WF:SupplierStatus ,
		pigShapes_ReqIF-WF:SupplierComment ,
		pigShapes_ReqIF-WF:CustomerStatus ,
		pigShapes_ReqIF-WF:CustomerComment .

SpecIF:Issue
	rdfs:subClassOf pig:Entity ;
	rdfs:label "Open Issue"@en ,
		"Offener Punkt"@de ,
		"Problème"@fr ;
	rdfs:comment "An 'Issue' is a question to answer or decision to take which is worth tracking."@en ,
		"Ein 'Offener Punkt ist eine zu beantwortende Frage oder eine zu treffende Entscheidung."@de ,
		"Un 'problème' est une question à laquelle il faut répondre ou une décision à prendre qui mérite d'être suivie."@fr .

pigShapes_SpecIF:Issue
	rdf:type sh:NodeShape ;
	sh:targetClass SpecIF:Issue ;
	sh:property pigShapes_dcterms:identifier ,
		pigShapes_rdfs:label ,
		pigShapes_rdfs:comment ,
		o:PC-IssueStatus_shape ,
		pigShapes_SpecIF:Priority ,
		pigShapes_SpecIF:Responsible ,
		pigShapes_SpecIF:DueDate .

#################################################################
# Ontology - Relationship Classes
#################################################################

SpecIF:contains
	rdfs:subClassOf pig:Relationship ;
	rdfs:label "contains"@en ,
		"enthält"@de ,
		"contient"@fr ;
	rdfs:comment "General containment, such as:\n- Package-A *contains* Diagram-B\n- Collection-1 *contains* DataObject-1.1\n\nNot to confound with *[[dcterms:hasPart]]*."@en .

SpecIF:contains-toSource
	rdfs:subPropertyOf pig:SourceLink ;
	rdfs:label "SpecIF:contains to source" ;
	rdfs:comment "Connects the source of SpecIF:contains" ;
	rdfs:domain SpecIF:contains ;
	rdfs:range [ owl:unionOf(
			FMC:Actor
			FMC:State
			FMC:Event
		)] .

SpecIF:contains-toTarget
	rdfs:subPropertyOf pig:TargetLink ;
	rdfs:label "SpecIF:contains to target" ;
	rdfs:comment "Connects the target of SpecIF:contains" ;
	rdfs:domain SpecIF:contains ;
	rdfs:range [ owl:unionOf(
			FMC:Actor
			FMC:State
			FMC:Event
		)] .

pigShapes_SpecIF:contains
	rdf:type sh:NodeShape ;
	sh:targetClass SpecIF:contains ;
	sh:property [ 
		sh:path SpecIF:contains-toSource ;
		sh:or (
			[ sh:class FMC:Actor ]
			[ sh:class FMC:State ]
			[ sh:class FMC:Event ]
		) ;
		sh:minCount 1 ;
		sh:maxCount 1
	] ;
	sh:property [ 
		sh:path SpecIF:contains-toTarget ;
		sh:or (
			[ sh:class FMC:Actor ]
			[ sh:class FMC:State ]
			[ sh:class FMC:Event ]
		) ;
		sh:minCount 1 ;
		sh:maxCount 1
	] .

o:SC-stores
	rdfs:subClassOf pig:Relationship ;
	rdfs:label "SpecIF:modifies" ;
	rdfs:comment "Relation: Actor (Role, Function) writes and reads State (Information)" .

o:SC-stores-toSource
	rdfs:subPropertyOf pig:SourceLink ;
	rdfs:label "o:SC-stores to source" ;
	rdfs:comment "Connects the source of o:SC-stores" ;
	rdfs:domain o:SC-stores ;
	rdfs:range FMC:Actor .

o:SC-stores-toTarget
	rdfs:subPropertyOf pig:TargetLink ;
	rdfs:label "o:SC-stores to target" ;
	rdfs:comment "Connects the target of o:SC-stores" ;
	rdfs:domain o:SC-stores ;
	rdfs:range FMC:State .

o:SC-stores_shape
	rdf:type sh:NodeShape ;
	sh:targetClass o:SC-stores ;
	sh:property [ 
		sh:path o:SC-stores-toSource ;
		sh:or (
			[ sh:class FMC:Actor ]
		) ;
		sh:minCount 1 ;
		sh:maxCount 1
	] ;
	sh:property [ 
		sh:path o:SC-stores-toTarget ;
		sh:or (
			[ sh:class FMC:State ]
		) ;
		sh:minCount 1 ;
		sh:maxCount 1
	] .

SpecIF:writes
	rdfs:subClassOf pig:Relationship ;
	rdfs:label "writes"@en ,
		"schreibt"@de ,
		"écrit"@fr ;
	rdfs:comment "A [[FMC:Actor]] 'writes' (changes) a [[FMC:State]]."@en .

SpecIF:writes-toSource
	rdfs:subPropertyOf pig:SourceLink ;
	rdfs:label "SpecIF:writes to source" ;
	rdfs:comment "Connects the source of SpecIF:writes" ;
	rdfs:domain SpecIF:writes ;
	rdfs:range FMC:Actor .

SpecIF:writes-toTarget
	rdfs:subPropertyOf pig:TargetLink ;
	rdfs:label "SpecIF:writes to target" ;
	rdfs:comment "Connects the target of SpecIF:writes" ;
	rdfs:domain SpecIF:writes ;
	rdfs:range FMC:State .

pigShapes_SpecIF:writes
	rdf:type sh:NodeShape ;
	sh:targetClass SpecIF:writes ;
	sh:property [ 
		sh:path SpecIF:writes-toSource ;
		sh:or (
			[ sh:class FMC:Actor ]
		) ;
		sh:minCount 1 ;
		sh:maxCount 1
	] ;
	sh:property [ 
		sh:path SpecIF:writes-toTarget ;
		sh:or (
			[ sh:class FMC:State ]
		) ;
		sh:minCount 1 ;
		sh:maxCount 1
	] .

SpecIF:reads
	rdfs:subClassOf pig:Relationship ;
	rdfs:label "reads"@en ,
		"liest"@de ,
		"lit"@fr ;
	rdfs:comment "A [[FMC:Actor]] 'reads' a [[FMC:State]]."@en .

SpecIF:reads-toSource
	rdfs:subPropertyOf pig:SourceLink ;
	rdfs:label "SpecIF:reads to source" ;
	rdfs:comment "Connects the source of SpecIF:reads" ;
	rdfs:domain SpecIF:reads ;
	rdfs:range FMC:Actor .

SpecIF:reads-toTarget
	rdfs:subPropertyOf pig:TargetLink ;
	rdfs:label "SpecIF:reads to target" ;
	rdfs:comment "Connects the target of SpecIF:reads" ;
	rdfs:domain SpecIF:reads ;
	rdfs:range FMC:State .

pigShapes_SpecIF:reads
	rdf:type sh:NodeShape ;
	sh:targetClass SpecIF:reads ;
	sh:property [ 
		sh:path SpecIF:reads-toSource ;
		sh:or (
			[ sh:class FMC:Actor ]
		) ;
		sh:minCount 1 ;
		sh:maxCount 1
	] ;
	sh:property [ 
		sh:path SpecIF:reads-toTarget ;
		sh:or (
			[ sh:class FMC:State ]
		) ;
		sh:minCount 1 ;
		sh:maxCount 1
	] .

SpecIF:dependsOn
	rdfs:subClassOf pig:Relationship ;
	rdfs:label "depends on"@en ,
		"hängt ab von"@de ,
		"depend de"@fr ;
	rdfs:comment "<p>A [[IREB:Requirement]] 'depends on' another [[IREB:Requirement]].</p>"@en .

SpecIF:dependsOn-toSource
	rdfs:subPropertyOf pig:SourceLink ;
	rdfs:label "SpecIF:dependsOn to source" ;
	rdfs:comment "Connects the source of SpecIF:dependsOn" ;
	rdfs:domain SpecIF:dependsOn ;
	rdfs:range IREB:Requirement .

SpecIF:dependsOn-toTarget
	rdfs:subPropertyOf pig:TargetLink ;
	rdfs:label "SpecIF:dependsOn to target" ;
	rdfs:comment "Connects the target of SpecIF:dependsOn" ;
	rdfs:domain SpecIF:dependsOn ;
	rdfs:range IREB:Requirement .

pigShapes_SpecIF:dependsOn
	rdf:type sh:NodeShape ;
	sh:targetClass SpecIF:dependsOn ;
	sh:property [ 
		sh:path SpecIF:dependsOn-toSource ;
		sh:or (
			[ sh:class IREB:Requirement ]
		) ;
		sh:minCount 1 ;
		sh:maxCount 1
	] ;
	sh:property [ 
		sh:path SpecIF:dependsOn-toTarget ;
		sh:or (
			[ sh:class IREB:Requirement ]
		) ;
		sh:minCount 1 ;
		sh:maxCount 1
	] .

oslc_rm:satisfies
	rdfs:subClassOf pig:Relationship ;
	rdfs:label "satisfies"@en ,
		"erfüllt"@de ,
		"satisfait"@fr ;
	rdfs:comment "<p>The object is satisfied by the subject. <small>(<i>source: <a href=\"http://open-services.net/\">OSLC</a></i>)</small></p><p>SpecIF suggests that the subject is confined to a model element, e.g, a [[FMC:Actor]] or [[FMC:State]], and the object is confined to a [[IREB:Requirement]]. More concretely, an example for this type of statement is 'Component-X <em>satisfies</em> 'Requirement-4711'.</p>"@en .

oslc_rm:satisfies-toSource
	rdfs:subPropertyOf pig:SourceLink ;
	rdfs:label "oslc_rm:satisfies to source" ;
	rdfs:comment "Connects the source of oslc_rm:satisfies" ;
	rdfs:domain oslc_rm:satisfies ;
	rdfs:range [ owl:unionOf(
			FMC:Actor
			FMC:State
			FMC:Event
		)] .

oslc_rm:satisfies-toTarget
	rdfs:subPropertyOf pig:TargetLink ;
	rdfs:label "oslc_rm:satisfies to target" ;
	rdfs:comment "Connects the target of oslc_rm:satisfies" ;
	rdfs:domain oslc_rm:satisfies ;
	rdfs:range IREB:Requirement .

pigShapes_oslc_rm:satisfies
	rdf:type sh:NodeShape ;
	sh:targetClass oslc_rm:satisfies ;
	sh:property [ 
		sh:path oslc_rm:satisfies-toSource ;
		sh:or (
			[ sh:class FMC:Actor ]
			[ sh:class FMC:State ]
			[ sh:class FMC:Event ]
		) ;
		sh:minCount 1 ;
		sh:maxCount 1
	] ;
	sh:property [ 
		sh:path oslc_rm:satisfies-toTarget ;
		sh:or (
			[ sh:class IREB:Requirement ]
		) ;
		sh:minCount 1 ;
		sh:maxCount 1
	] .

SpecIF:refersTo
	rdfs:subClassOf pig:Relationship ;
	rdfs:label "refers to"@en ,
		"bezieht sich auf"@de ,
		"concerne"@fr ;
	rdfs:comment "<p>A resource 'refers to' any other resource.</p>"@en .

SpecIF:refersTo-toSource
	rdfs:subPropertyOf pig:SourceLink ;
	rdfs:label "SpecIF:refersTo to source" ;
	rdfs:comment "Connects the source of SpecIF:refersTo" ;
	rdfs:domain SpecIF:refersTo ;
	rdfs:range SpecIF:Issue .

SpecIF:refersTo-toTarget
	rdfs:subPropertyOf pig:TargetLink ;
	rdfs:label "SpecIF:refersTo to target" ;
	rdfs:comment "Connects the target of SpecIF:refersTo" ;
	rdfs:domain SpecIF:refersTo ;
	rdfs:range [ owl:unionOf(
			pig:View
			FMC:Actor
			FMC:State
			FMC:Event
			IREB:Requirement
		)] .

pigShapes_SpecIF:refersTo
	rdf:type sh:NodeShape ;
	sh:targetClass SpecIF:refersTo ;
	sh:property [ 
		sh:path SpecIF:refersTo-toSource ;
		sh:or (
			[ sh:class SpecIF:Issue ]
		) ;
		sh:minCount 1 ;
		sh:maxCount 1
	] ;
	sh:property [ 
		sh:path SpecIF:refersTo-toTarget ;
		sh:or (
			[ sh:class pig:View ]
			[ sh:class FMC:Actor ]
			[ sh:class FMC:State ]
			[ sh:class FMC:Event ]
			[ sh:class IREB:Requirement ]
		) ;
		sh:minCount 1 ;
		sh:maxCount 1
	] .

#################################################################
# Entities
#################################################################

d:Pln-27420ffc0000c3a8013ab527ca1b71f5
	rdf:type pig:View ;
	rdfs:label "Color coding" ;
	SpecIF:Diagram "<div style=\"max-width: 480px;\" ><object data=\"files_and_images/27420ffc0000c3a8013ab527ca1b71f5.svg\" type=\"image/svg+xml\" >Color Coding</object></div>" ;
	SpecIF:Notation "FMC Block Diagram" ;
	SpecIF:LifecycleStatus SpecIF:LifecycleStatusApproved ;
	ReqIF-WF:SupplierStatus SpecIF:NotApplicable ;
	ReqIF-WF:CustomerStatus ReqIF-WF:CustomerStatus.NotToEvaluate ;
	pig:revision "18" ;
	dcterms:modified "2017-06-19T20:13:03+02:00" ;
	dcterms:creator "od" .

d:Pln-5a4755dd0000bca801375293a62c90a8
	rdf:type pig:View ;
	rdfs:label "SmartHome System" ;
	rdfs:comment "<div><p>The Smart-Home-System consists of sensors on the left side, the controller in the middle and the actuators on the right side. </p></div>" ;
	SpecIF:Diagram "<div style=\"max-width: 600px;\"><object data=\"files_and_images/5a4755dd0000bca801375293a62c90a8.svg\" type=\"image/svg+xml\" >files_and_images\\5a4755dd0000bca801375293a62c90a8.svg</object></div>" ;
	SpecIF:Notation "FMC Block Diagram" ;
	SpecIF:LifecycleStatus SpecIF:LifecycleStatusInitial ;
	ReqIF-WF:SupplierStatus ReqIF-WF:CustomerStatus.ToBeClarified ;
	ReqIF-WF:CustomerStatus ReqIF-WF:CustomerStatus.ToEvaluate ;
	pig:revision "19" ;
	dcterms:modified "2017-06-19T20:13:03+02:00" ;
	dcterms:creator "od" ;
	pig:shows (
			d:MEl-5bd6bd890000bca8013739588a3f43d6
			d:MEl-5a4dd77b0000bca8013736c6912ad291
			d:MEl-5a489c300000bca80137ee1373c16844
			d:MEl-5a4c80c20000bca8013753b6999a4da8
			d:MEl-5bcf35cf0000bca8013776d68023612a
			d:MEl-5a52b50c0000bca801377e3d15255f98
			d:MEl-5a51dd920000bca8013770a4395c83fc
			d:MEl-5a50d5b60000bca8013781532547ce93
			d:MEl-5bcfb01d0000bca80137f303272a5557
			d:MEl-803fd3750000c3a8013cf1fdb3b26d33
			d:MEl-5a4cfa830000bca801370d837f761f3e
			d:MEl-5a4d2bd00000bca80137a3f233cdffeb
			d:MEl-5a4d6dee0000bca80137c1caf2f42349
			d:MEl-5a47935a0000bca801377c17f8cb25b0
		) .

d:Pln-5a6cdea50000bca80137d6b2d6e8a3a0
	rdf:type pig:View ;
	rdfs:label "Flush-mounted Dimmer" ;
	rdfs:comment "<div><p> .. showing the components of the device with their interfaces. </p></div>" ;
	SpecIF:Diagram "<div style=\"max-width: 600px;\"><object data=\"files_and_images/5a6cdea50000bca80137d6b2d6e8a3a0.svg\" type=\"image/svg+xml\" >files_and_images\\5a6cdea50000bca80137d6b2d6e8a3a0.svg</object></div>" ;
	SpecIF:Notation "FMC Block Diagram" ;
	SpecIF:LifecycleStatus SpecIF:LifecycleStatusInitial ;
	ReqIF-WF:SupplierStatus ReqIF-WF:SupplierStatus.NotAgreed ;
	ReqIF-WF:CustomerStatus ReqIF-WF:CustomerStatus.NotAccepted ;
	pig:revision "19" ;
	dcterms:modified "2017-06-19T20:13:03+02:00" ;
	dcterms:creator "od" ;
	pig:shows (
			d:MEl-5a7776c50000bca8013765ae93af9209
			d:MEl-5a76365c0000bca8013776e91afd1e8e
			d:MEl-5a9ce0310000bca801378176dc4744e8
			d:MEl-5a752ccc0000bca80137479a2e8bab30
			d:MEl-5a71c4800000bca80137f2aaa7b63000
			d:MEl-5a4dd77b0000bca8013736c6912ad291
			d:MEl-5a489c300000bca80137ee1373c16844
			d:MEl-5a99c89c0000bca801375d44cf9a50ca
			d:MEl-5a9929510000bca80137d23c81f1ca54
			d:MEl-5c29fb8e0000bca80137eb9734c99bfd
			d:MEl-5a77385f0000bca80137e1c7dc0b1721
			d:MEl-5a9888810000bca801375410ce1cc142
			d:MEl-5a4d6dee0000bca80137c1caf2f42349
			d:MEl-5a9b7a9b0000bca80137d768644696b7
			d:MEl-463289cd0000c3a80141be3fc417034a
		) .

d:Pln-5a7f99af0000bca8013754f2ef12d3e5
	rdf:type pig:View ;
	rdfs:label "Dimmer Module" ;
	SpecIF:Diagram "<div style=\"max-width: 600px;\"><object data=\"files_and_images/5a7f99af0000bca8013754f2ef12d3e5.svg\" type=\"image/svg+xml\" >files_and_images\\5a7f99af0000bca8013754f2ef12d3e5.svg</object></div>" ;
	SpecIF:Notation "FMC Block Diagram" ;
	SpecIF:LifecycleStatus SpecIF:LifecycleStatusInitial ;
	ReqIF-WF:SupplierStatus ReqIF-WF:SupplierStatus.AgreedWithComment ;
	ReqIF-WF:CustomerStatus ReqIF-WF:CustomerStatus.ToEvaluate ;
	pig:revision "20" ;
	dcterms:modified "2017-06-19T20:13:04+02:00" ;
	dcterms:creator "od" ;
	pig:shows (
			d:MEl-5a9ce0310000bca801378176dc4744e8
			d:MEl-5a85347c0000bca80137ad485c7cd330
			d:MEl-5a808e2a0000bca80137bfd74268a84a
			d:MEl-5a752ccc0000bca80137479a2e8bab30
			d:MEl-5a844d820000bca8013750b9a0410b6b
			d:MEl-5a99c89c0000bca801375d44cf9a50ca
			d:MEl-5a8009a00000bca80137ef95bc3f643f
			d:MEl-5a87083e0000bca801379bb412523737
			d:MEl-5a9929510000bca80137d23c81f1ca54
			d:MEl-5c29fb8e0000bca80137eb9734c99bfd
			d:MEl-5a82ec6f0000bca801372ef053a71bdf
			d:MEl-5a86b8980000bca80137ca6fde1a125e
			d:MEl-5a77385f0000bca80137e1c7dc0b1721
			d:MEl-5a9888810000bca801375410ce1cc142
			d:MEl-5a820a3c0000bca801378c9093fb7d80
		) .

d:Pln-606e76c70000bca801376ec3133a1181
	rdf:type pig:View ;
	rdfs:label "User Activity" ;
	rdfs:comment "<div><p>This shows the defined sequences of manual operation to activate the device. </p></div>" ;
	SpecIF:Diagram "<div style=\"max-width: 600px;\"><object data=\"files_and_images/606e76c70000bca801376ec3133a1181.svg\" type=\"image/svg+xml\" >files_and_images\\606e76c70000bca801376ec3133a1181.svg</object></div>" ;
	SpecIF:Notation "BPMN Process Model" ;
	SpecIF:LifecycleStatus SpecIF:LifecycleStatusDrafted ;
	ReqIF-WF:SupplierStatus ReqIF-WF:SupplierStatus.Agreed ;
	ReqIF-WF:CustomerStatus ReqIF-WF:CustomerStatus.Accepted ;
	pig:revision "20" ;
	dcterms:modified "2017-06-19T20:13:04+02:00" ;
	dcterms:creator "od" ;
	pig:shows (
			d:MEl-608177820000bca801379179ebf3b6aa
			d:MEl-611366530000bca80137a97f194e96a3
			d:MEl-453862540000c3a801419d91bef48cfd
			d:MEl-45387c0b0000c3a801410aa03f6b9be4
			d:MEl-4538920b0000c3a801415c67e334b8a1
			d:MEl-608239830000bca801373690c7d2af0f
			d:MEl-610b07100000bca80137c10f96c46247
			d:MEl-610e0b010000bca80137ac40800bb1b8
			d:MEl-459b92580000c3a80141cb4acb521ab1
			d:MEl-45384cd10000c3a80141c1f85d7c26e6
			d:MEl-607f13b50000bca80137ba95f11856ab
			d:MEl-5a47935a0000bca801377c17f8cb25b0
		) .

d:Pln-45a1c8930000c3a801414cd1eaa70b5a
	rdf:type pig:View ;
	rdfs:label "Double-Button Observer Software" ;
	rdfs:comment "<div><p>This software module discriminates the user's activity (operation sequence) and submits corresponding events/commands to the actuator. This software is generic with respect to the actuator, it can be used for [[dimmer]]s, [[shading]] devices and others. </p></div>" ;
	SpecIF:Diagram "<div style=\"max-width: 600px;\"><object type=\"image/svg+xml\" data=\"files_and_images/45a1c8930000c3a801414cd1eaa70b5a.svg\">files_and_images\\45a1c8930000c3a801414cd1eaa70b5a.svg</object></div>" ;
	SpecIF:Notation "BPMN Process Model" ;
	SpecIF:LifecycleStatus SpecIF:LifecycleStatusDrafted ;
	ReqIF-WF:SupplierStatus ReqIF-WF:SupplierStatus.Agreed ;
	ReqIF-WF:CustomerStatus ReqIF-WF:CustomerStatus.Accepted ;
	pig:revision "253" ;
	dcterms:modified "2018-03-15T15:36:31+01:00" ;
	dcterms:creator "od" ;
	pig:shows (
			d:MEl-606f16ac0000bca801373587fda932b3
			d:MEl-45450be80000c3a801414f280f146c71
			d:MEl-4536b0350000c3a801415986f8ea806a
			d:MEl-453facbb0000c3a80141c43d2fb4f5e2
			d:MEl-4543fe900000c3a80141f5253ff13c35
			d:MEl-453d34af0000c3a80141918f84641161
			d:MEl-45a236e00000c3a801410f6503287e16
			d:MEl-45a3b13c0000c3a801415e97f5bc29d1
		) .

d:Pln-5af364560000bca80137b84017f4e832
	rdf:type pig:View ;
	rdfs:label "Dimmer Controller Software" ;
	rdfs:comment "<div><p>This software decodes the commands and controls the timely behavior of the actuator. </p></div>" ;
	SpecIF:Diagram "<div style=\"max-width: 720px;\"><object data=\"files_and_images/5af364560000bca80137b84017f4e832.svg\" type=\"image/svg+xml\" >files_and_images\\5af364560000bca80137b84017f4e832.svg</object></div>" ;
	SpecIF:Notation "Petri Net" ;
	SpecIF:LifecycleStatus SpecIF:LifecycleStatusDrafted ;
	ReqIF-WF:SupplierStatus ReqIF-WF:SupplierStatus.Agreed ;
	ReqIF-WF:CustomerStatus ReqIF-WF:CustomerStatus.Accepted ;
	pig:revision "22" ;
	dcterms:modified "2017-06-19T20:13:06+02:00" ;
	dcterms:creator "od" ;
	pig:shows (
			d:MEl-5b2f95ec0000bca8013709bfa81d701f
			d:MEl-5a85347c0000bca80137ad485c7cd330
			d:MEl-45450be80000c3a801414f280f146c71
			d:MEl-4536b0350000c3a801415986f8ea806a
			d:MEl-5b149eab0000bca80137aad99b6eea7b
			d:MEl-5b08ed8d0000bca8013719f554353b0e
			d:MEl-453dfb670000c3a8014191107df4565e
			d:MEl-5b094f8a0000bca801374c798a6587ad
			d:MEl-45428b930000c3a80141e28b7d4b5ae5
			d:MEl-5b078fa50000bca80137f36ed05c43cb
			d:MEl-453facbb0000c3a80141c43d2fb4f5e2
			d:MEl-5b2d29070000bca801378a6c020cf8f5
			d:MEl-5b1750f80000bca801373b2d143d7478
			d:MEl-5b2ddad80000bca80137c44d62ba97d8
			d:MEl-5b2449180000bca8013722c01c9d35a5
			d:MEl-5b0839b90000bca801376dcca41ca7d0
			d:MEl-5b07e6aa0000bca8013797aad9be69ae
			d:MEl-4543fe900000c3a80141f5253ff13c35
			d:MEl-453d34af0000c3a80141918f84641161
		) .

d:Req-d1c895230000c3a80150f8afd049f738
	rdf:type IREB:Requirement ;
	dcterms:identifier "REQ_014" ;
	rdfs:label "Dim an electric load" ;
	rdfs:comment "<div><p> The user can set the intensity level of an electric load such as a light [[bulb]]. Pressing a button 'up' or 'down', the intensity is increased or decreased following a quasi-stepless ramp. <br /></p></div>" ;
	SpecIF:LifecycleStatus SpecIF:LifecycleStatusApproved ;
	SpecIF:Priority SpecIF:priorityMedium ;
	SpecIF:StakeholderGroup SpecIF:StakeholderGroupUser ;
	SpecIF:EngineeringDiscipline SpecIF:EngineeringDisciplineMechanics ,
		SpecIF:EngineeringDisciplineElectronics ,
		SpecIF:EngineeringDisciplineSoftware ;
	ReqIF-WF:SupplierStatus ReqIF-WF:SupplierStatus.Agreed ;
	ReqIF-WF:SupplierComment "Our solution does this perfectly." ;
	pig:revision "23" ;
	dcterms:modified "2017-06-19T20:13:06+02:00" ;
	dcterms:creator "od" .

d:Req-d1d42a6a0000c3a8015091ec8d149b93
	rdf:type IREB:Requirement ;
	dcterms:identifier "REQ_016" ;
	rdfs:label "Switch an electric load" ;
	rdfs:comment "<div><p> The user can immediately switch 'on' or 'off' the electric load. The intensity set to the maximum resp. minimum level, as defined by installation parameters.</p></div>" ;
	SpecIF:LifecycleStatus SpecIF:LifecycleStatusApproved ;
	SpecIF:Priority SpecIF:priorityMedium ;
	SpecIF:StakeholderGroup SpecIF:StakeholderGroupUser ;
	SpecIF:EngineeringDiscipline SpecIF:EngineeringDisciplineElectronics ,
		SpecIF:EngineeringDisciplineSoftware ;
	pig:revision "243" ;
	dcterms:modified "2018-02-13T12:22:44+01:00" ;
	dcterms:creator "od" .

d:Req-d1cd7f370000c3a8015095e6ee21aab7
	rdf:type IREB:Requirement ;
	dcterms:identifier "REQ_015" ;
	rdfs:label "Set dimming parameters" ;
	rdfs:comment "<div><p> During system setup, the installer can modify the following parameters: </p><ul> <li> maximum intensity </li> <li> minimum intensity </li> <li> dimming speed (intensity ramp when dimming) </li></ul></div>" ;
	SpecIF:LifecycleStatus SpecIF:LifecycleStatusSubmitted ;
	SpecIF:Priority SpecIF:priorityMedium ;
	SpecIF:StakeholderGroup SpecIF:StakeholderGroupUser ;
	SpecIF:EngineeringDiscipline SpecIF:EngineeringDisciplineSoftware ;
	pig:revision "24" ;
	dcterms:modified "2017-06-19T20:13:07+02:00" ;
	dcterms:creator "od" .

d:Req-5ba3512b0000bca801371cc0617eb4c1
	rdf:type IREB:Requirement ;
	dcterms:identifier "REQ_009" ;
	rdfs:label "Minimum button size" ;
	rdfs:comment "<div><p>The button size must not be less than 2 cm in diameter.</p> </div>" ;
	SpecIF:LifecycleStatus SpecIF:LifecycleStatusApproved ;
	SpecIF:Priority SpecIF:priorityHigh ;
	SpecIF:StakeholderGroup SpecIF:StakeholderGroupUser ;
	SpecIF:EngineeringDiscipline SpecIF:EngineeringDisciplineMechanics ;
	ReqIF-WF:SupplierStatus ReqIF-WF:CustomerStatus.ToBeClarified ;
	ReqIF-WF:SupplierComment "We did not find the actual minimum dimensions of the buttons." ;
	pig:revision "25" ;
	dcterms:modified "2017-06-19T20:13:08+02:00" ;
	dcterms:creator "od" .

d:Req-5b8fbb300000bca80137c73e3ce4c737
	rdf:type IREB:Requirement ;
	dcterms:identifier "REQ_001" ;
	rdfs:label "Electric load is 120 W" ;
	rdfs:comment "<div><p>The power stage must allow an electric load of 120 W.</p> </div>" ;
	SpecIF:LifecycleStatus SpecIF:LifecycleStatusSubmitted ;
	SpecIF:Priority SpecIF:priorityHigh ;
	SpecIF:StakeholderGroup SpecIF:StakeholderGroupUser ;
	SpecIF:EngineeringDiscipline SpecIF:EngineeringDisciplineElectronics ;
	ReqIF-WF:SupplierStatus ReqIF-WF:CustomerStatus.ToBeClarified ;
	ReqIF-WF:SupplierComment "For which time period?  Permanent load?" ;
	pig:revision "25" ;
	dcterms:modified "2017-06-19T20:13:08+02:00" ;
	dcterms:creator "od" .

d:Req-5b944fc70000bca8013763f44fdc0e03
	rdf:type IREB:Requirement ;
	dcterms:identifier "REQ_003" ;
	rdfs:label "Instant use" ;
	rdfs:comment "<div><p>85% of an arbitrarily selected group of test users understands and can use the system without reading a manual.</p> </div>" ;
	SpecIF:LifecycleStatus SpecIF:LifecycleStatusApproved ;
	SpecIF:Priority SpecIF:priorityMedium ;
	SpecIF:StakeholderGroup SpecIF:StakeholderGroupUser ;
	SpecIF:EngineeringDiscipline SpecIF:EngineeringDisciplineMechanics ,
		SpecIF:EngineeringDisciplineSoftware ;
	ReqIF-WF:SupplierStatus ReqIF-WF:SupplierStatus.Agreed ;
	pig:revision "26" ;
	dcterms:modified "2017-06-19T20:13:09+02:00" ;
	dcterms:creator "od" .

d:Req-5ba140d60000bca801372b09f9888eca
	rdf:type IREB:Requirement ;
	dcterms:identifier "REQ_008" ;
	rdfs:label "Instantaneous reaction" ;
	rdfs:comment "<div><p> The reaction time of the system to user input is 'instantaneous' (&lt; 0,5 sec).</p></div>" ;
	SpecIF:LifecycleStatus SpecIF:LifecycleStatusDone ;
	SpecIF:Priority SpecIF:priorityHigh ;
	SpecIF:StakeholderGroup SpecIF:StakeholderGroupUser ;
	SpecIF:EngineeringDiscipline SpecIF:EngineeringDisciplineSoftware ;
	ReqIF-WF:SupplierStatus ReqIF-WF:SupplierStatus.Agreed ;
	ReqIF-WF:SupplierComment "Mais bien sûr." ;
	ReqIF-WF:CustomerStatus ReqIF-WF:CustomerStatus.ToEvaluate ;
	ReqIF-WF:CustomerComment "Das ist ganz wichtig für uns." ;
	pig:revision "252" ;
	dcterms:modified "2018-03-08T11:59:42+01:00" ;
	dcterms:creator "supplier" .

d:Req-ee452cf20000c3a8014035290669304d
	rdf:type IREB:Requirement ;
	dcterms:identifier "REQ_011" ;
	rdfs:label "Consistent system behavior" ;
	rdfs:comment "<div><p>The system's behavior must be consistent. For example, controlling a dimmer must correspond with controlling a shade.</p> </div>" ;
	SpecIF:LifecycleStatus SpecIF:LifecycleStatusApproved ;
	SpecIF:Priority SpecIF:priorityMedium ;
	SpecIF:StakeholderGroup SpecIF:StakeholderGroupUser ;
	SpecIF:EngineeringDiscipline SpecIF:EngineeringDisciplineMechanics ,
		SpecIF:EngineeringDisciplineSoftware ;
	pig:revision "27" ;
	dcterms:modified "2017-06-19T20:13:10+02:00" ;
	dcterms:creator "od" .

d:Req-ee43fc4c0000c3a8014063d42c77767f
	rdf:type IREB:Requirement ;
	dcterms:identifier "REQ_010" ;
	rdfs:label "No dead-locks" ;
	rdfs:comment "<div><p>Under no circumstances the system may get stuck in a dead-lock. I.e. every sequence of input stimulation must be supported, even arbitrary sequences. Input stimulation which is not supported in a given system state is either refused with an error message, if a feedback channel is available, or it is simply ignored, otherwise.</p> </div>" ;
	SpecIF:LifecycleStatus SpecIF:LifecycleStatusApproved ;
	SpecIF:Priority SpecIF:priorityHigh ;
	SpecIF:StakeholderGroup SpecIF:StakeholderGroupSystem ;
	SpecIF:EngineeringDiscipline SpecIF:EngineeringDisciplineElectronics ,
		SpecIF:EngineeringDisciplineSoftware ;
	pig:revision "28" ;
	dcterms:modified "2017-06-19T20:13:11+02:00" ;
	dcterms:creator "od" .

d:Req-5b9124bc0000bca80137fa2ce86f5eca
	rdf:type IREB:Requirement ;
	dcterms:identifier "REQ_002" ;
	rdfs:label "Overload protection" ;
	rdfs:comment "<div><p>The dimmer unit is protected against resistive overload and against any capacitive or inductive loads.</p> </div>" ;
	SpecIF:LifecycleStatus SpecIF:LifecycleStatusSubmitted ;
	SpecIF:Priority SpecIF:priorityMedium ;
	SpecIF:StakeholderGroup SpecIF:StakeholderGroupUser ;
	SpecIF:EngineeringDiscipline SpecIF:EngineeringDisciplineElectronics ;
	pig:revision "29" ;
	dcterms:modified "2017-06-19T20:13:11+02:00" ;
	dcterms:creator "od" .

d:Req-5b9e68530000bca801371362c49d2d08
	rdf:type IREB:Requirement ;
	dcterms:identifier "REQ_007" ;
	rdfs:label "Auto shut-off" ;
	rdfs:comment "<div><p>In case of over-temperature the device is shut-off automatically by an electronic circuit.</p> </div>" ;
	SpecIF:LifecycleStatus SpecIF:LifecycleStatusSubmitted ;
	SpecIF:Priority SpecIF:priorityMedium ;
	SpecIF:StakeholderGroup SpecIF:StakeholderGroupSystem ;
	SpecIF:EngineeringDiscipline SpecIF:EngineeringDisciplineElectronics ;
	pig:revision "29" ;
	dcterms:modified "2017-06-19T20:13:11+02:00" ;
	dcterms:creator "od" .

d:Req-eea1cd500000c3a80140fe00109eb7f4
	rdf:type IREB:Requirement ;
	dcterms:identifier "REQ_012" ;
	rdfs:label "Compliance with industry standards" ;
	rdfs:comment "<div><p>The system must comply with industry standards. Besides legal and safety requirements, compatibility with existing electrical installations, tools and commercial components is desired.</p> </div>" ;
	SpecIF:LifecycleStatus SpecIF:LifecycleStatusApproved ;
	SpecIF:Priority SpecIF:priorityMedium ;
	SpecIF:StakeholderGroup SpecIF:StakeholderGroupUser ;
	SpecIF:EngineeringDiscipline SpecIF:EngineeringDisciplineMechanics ,
		SpecIF:EngineeringDisciplineElectronics ,
		SpecIF:EngineeringDisciplineSafety ;
	pig:revision "31" ;
	dcterms:modified "2017-06-19T20:13:12+02:00" ;
	dcterms:creator "od" .

d:Req-5b95fae40000bca801372becc933682d
	rdf:type IREB:Requirement ;
	dcterms:identifier "REQ_004" ;
	rdfs:label "Industry-standard mounting" ;
	rdfs:comment "<div><p> The product fits into an industry-standard [[housing]] for flush-mounted devices (diameter &#x2300;68 mm). It is fixed with two screw-activated claws.</p></div>" ;
	SpecIF:LifecycleStatus SpecIF:LifecycleStatusSubmitted ;
	SpecIF:Priority SpecIF:priorityHigh ;
	SpecIF:StakeholderGroup SpecIF:StakeholderGroupSystem ;
	SpecIF:EngineeringDiscipline SpecIF:EngineeringDisciplineMechanics ;
	pig:revision "32" ;
	dcterms:modified "2017-06-19T20:13:12+02:00" ;
	dcterms:creator "od" .

d:Req-5b9ab8a50000bca801377ad0be3bbc89
	rdf:type IREB:Requirement ;
	dcterms:identifier "REQ_005" ;
	rdfs:label "Fire protection" ;
	rdfs:comment "<div><p> The product must withstand 650°C (VDE 0606-1).</p></div>" ;
	SpecIF:LifecycleStatus SpecIF:LifecycleStatusSubmitted ;
	SpecIF:Priority SpecIF:priorityHigh ;
	SpecIF:StakeholderGroup SpecIF:StakeholderGroupUser ;
	SpecIF:EngineeringDiscipline SpecIF:EngineeringDisciplineMechanics ,
		SpecIF:EngineeringDisciplineElectronics ;
	pig:revision "244" ;
	dcterms:modified "2018-02-16T10:29:48+01:00" ;
	dcterms:creator "od" .

d:Req-728c69c80018b1a8014b974542c36edc
	rdf:type IREB:Requirement ;
	dcterms:identifier "REQ_013" ;
	rdfs:label "Galvanic Isolation" ;
	rdfs:comment "<div><p>The load circuit with power stage is galvanically isolated from the controller.</p> </div>" ;
	SpecIF:LifecycleStatus SpecIF:LifecycleStatusSubmitted ;
	SpecIF:Priority SpecIF:priorityHigh ;
	SpecIF:StakeholderGroup SpecIF:StakeholderGroupSystem ;
	SpecIF:EngineeringDiscipline SpecIF:EngineeringDisciplineElectronics ;
	ReqIF-WF:SupplierComment "This is standard for all our products: expensive, but effective." ;
	ReqIF-WF:CustomerStatus ReqIF-WF:CustomerStatus.ToEvaluate ;
	pig:revision "247" ;
	dcterms:modified "2018-02-28T13:16:17+01:00" ;
	dcterms:creator "supplier" .

d:Req-5b9c950e0000bca801374f16615247b9
	rdf:type IREB:Requirement ;
	dcterms:identifier "REQ_006" ;
	rdfs:label "Complete state-machine" ;
	rdfs:comment "<div><p> The system is controlled by a complete state-machine and must not have any dead-lock state.</p></div>" ;
	SpecIF:LifecycleStatus SpecIF:LifecycleStatusApproved ;
	SpecIF:Priority SpecIF:priorityMedium ;
	SpecIF:StakeholderGroup SpecIF:StakeholderGroupSystem ;
	SpecIF:EngineeringDiscipline SpecIF:EngineeringDisciplineSoftware ;
	pig:revision "233" ;
	dcterms:modified "2017-10-27T11:44:20+02:00" ;
	dcterms:creator "od" .

d:MEl-5bd6bd890000bca8013739588a3f43d6
	rdf:type FMC:Actor ;
	rdfs:label "Bulb" ;
	rdfs:comment "<div><p> Dimmable candescent light-bulb 230V.</p></div>" ;
	pig:revision "239" ;
	dcterms:modified "2017-11-11T16:16:13+01:00" ;
	dcterms:creator "od" .

d:MEl-5bcfb01d0000bca80137f303272a5557
	rdf:type FMC:Actor ;
	rdfs:label "Shading" ;
	rdfs:comment "<div><p>Window-shade with 2 degrees of freedom: It can be moved up/down and the elements can be set straight/tilted. Both movements can be made proportionally with an electric drive.</p> </div>" ;
	pig:revision "50" ;
	dcterms:modified "2017-06-19T20:13:19+02:00" ;
	dcterms:creator "od" .

d:MEl-803fd3750000c3a8013cf1fdb3b26d33
	rdf:type FMC:State ;
	rdfs:label "SmartHome System" ;
	rdfs:comment "<div><p>The new system for controlling all major functions of the private home:</p> <ul> <li>light/illumination</li> <li>window shades</li> <li>heating</li> <li>consumption meters for electricity, heat, gas and water.</li></ul> </div>" ;
	pig:revision "73" ;
	dcterms:modified "2017-06-19T20:13:26+02:00" ;
	dcterms:creator "od" .

d:MEl-5a489c300000bca80137ee1373c16844
	rdf:type FMC:State ;
	rdfs:label "Flush-mounted Dimmer" ;
	rdfs:comment "<p>A dimmer for electric loads in an industry-standard mounting frame which is flush with the wall surface. In other words, the dimmer is sitting in the wall and just the buttons are visible.</p>" ;
	pig:revision "63" ;
	dcterms:modified "2017-06-19T20:13:23+02:00" ;
	dcterms:creator "od" .

d:MEl-5a7776c50000bca8013765ae93af9209
	rdf:type FMC:State ;
	rdfs:label "Actuator Rods" ;
	rdfs:comment "<div><p>Up to four actuator rods connecting the buttons to electrical contacts.</p> </div>" ;
	pig:revision "59" ;
	dcterms:modified "2017-06-19T20:13:22+02:00" ;
	dcterms:creator "od" .

d:MEl-5a76365c0000bca8013776e91afd1e8e
	rdf:type FMC:Actor ;
	rdfs:label "Assembly Frame" ;
	rdfs:comment "<div><p> Mounting frame screwed to or into a wall.</p></div>" ;
	pig:revision "39" ;
	dcterms:modified "2017-06-19T20:13:16+02:00" ;
	dcterms:creator "od" .

d:MEl-5a9ce0310000bca801378176dc4744e8
	rdf:type FMC:State ;
	rdfs:label "Control Signals" ;
	pig:revision "60" ;
	dcterms:modified "2017-06-19T20:13:22+02:00" ;
	dcterms:creator "od" .

d:MEl-5a752ccc0000bca80137479a2e8bab30
	rdf:type FMC:Actor ;
	rdfs:label "Dimmer Module" ;
	rdfs:comment "<div><p>The actuator module with dimmer function for resistive loads.</p> </div>" ;
	pig:revision "45" ;
	dcterms:modified "2017-06-19T20:13:17+02:00" ;
	dcterms:creator "od" .

d:MEl-5a85347c0000bca80137ad485c7cd330
	rdf:type FMC:Actor ;
	rdfs:label "Dimmer Controller Software" ;
	rdfs:comment "<div><p> Input commands (events):</p><ul> <li> up-long → increase brightness </li> <li> down-long → decrease brightness </li> <li> release → stop dimming, keep brightness </li> <li> up-short → switch to maximum </li> <li> down-short → switch to minimum </li> <li> inappropriate commands are ignored (e.g. up-long when maximum is set). </li> <li> set parameters </li></ul><p> Four parameters influence the behavior of the particular device:</p><ul> <li> minimum value (default: 0%) </li> <li> maximum value (default: 100%) </li> <li> ramp-up speed (default: 10% per sec) </li> <li> ramp-down speed (default: 10% per sec) </li></ul></div>" ;
	pig:revision "242" ;
	dcterms:modified "2017-12-09T10:38:29+01:00" ;
	dcterms:creator "od" .

d:MEl-5b2f95ec0000bca8013709bfa81d701f
	rdf:type FMC:Event ;
	rdfs:label "Decreasing" ;
	pig:revision "81" ;
	dcterms:modified "2017-06-19T20:13:28+02:00" ;
	dcterms:creator "od" .

d:MEl-45450be80000c3a801414f280f146c71
	rdf:type FMC:Event ;
	rdfs:label "down-long!" ;
	pig:revision "84" ;
	dcterms:modified "2017-06-19T20:13:29+02:00" ;
	dcterms:creator "od" .

d:MEl-4536b0350000c3a801415986f8ea806a
	rdf:type FMC:Event ;
	rdfs:label "down-short!" ;
	pig:revision "85" ;
	dcterms:modified "2017-06-19T20:13:30+02:00" ;
	dcterms:creator "od" .

d:MEl-5b149eab0000bca80137aad99b6eea7b
	rdf:type FMC:Event ;
	rdfs:label "Increasing" ;
	pig:revision "85" ;
	dcterms:modified "2017-06-19T20:13:30+02:00" ;
	dcterms:creator "od" .

d:MEl-5b08ed8d0000bca8013719f554353b0e
	rdf:type FMC:Event ;
	rdfs:label "Intermediate" ;
	pig:revision "86" ;
	dcterms:modified "2017-06-19T20:13:30+02:00" ;
	dcterms:creator "od" .

d:MEl-453dfb670000c3a8014191107df4565e
	rdf:type FMC:Event ;
	rdfs:label "max-reached!" ;
	pig:revision "87" ;
	dcterms:modified "2017-06-19T20:13:30+02:00" ;
	dcterms:creator "od" .

d:MEl-5b094f8a0000bca801374c798a6587ad
	rdf:type FMC:Event ;
	rdfs:label "Maximum" ;
	pig:revision "87" ;
	dcterms:modified "2017-06-19T20:13:30+02:00" ;
	dcterms:creator "od" .

d:MEl-45428b930000c3a80141e28b7d4b5ae5
	rdf:type FMC:Event ;
	rdfs:label "min-reached!" ;
	pig:revision "88" ;
	dcterms:modified "2017-06-19T20:13:30+02:00" ;
	dcterms:creator "od" .

d:MEl-5b078fa50000bca80137f36ed05c43cb
	rdf:type FMC:Event ;
	rdfs:label "Minimum" ;
	pig:revision "89" ;
	dcterms:modified "2017-06-19T20:13:31+02:00" ;
	dcterms:creator "od" .

d:MEl-453facbb0000c3a80141c43d2fb4f5e2
	rdf:type FMC:Event ;
	rdfs:label "released!" ;
	pig:revision "89" ;
	dcterms:modified "2017-06-19T20:13:31+02:00" ;
	dcterms:creator "od" .

d:MEl-5b2d29070000bca801378a6c020cf8f5
	rdf:type FMC:Actor ;
	rdfs:label "Start-decreasing" ;
	pig:revision "51" ;
	dcterms:modified "2017-06-19T20:13:19+02:00" ;
	dcterms:creator "od" .

d:MEl-5b1750f80000bca801373b2d143d7478
	rdf:type FMC:Actor ;
	rdfs:label "Start-increasing" ;
	pig:revision "51" ;
	dcterms:modified "2017-06-19T20:13:19+02:00" ;
	dcterms:creator "od" .

d:MEl-5b2ddad80000bca80137c44d62ba97d8
	rdf:type FMC:Actor ;
	rdfs:label "Stop-decreasing" ;
	pig:revision "52" ;
	dcterms:modified "2017-06-19T20:13:20+02:00" ;
	dcterms:creator "od" .

d:MEl-5b2449180000bca8013722c01c9d35a5
	rdf:type FMC:Actor ;
	rdfs:label "Stop-increasing" ;
	pig:revision "52" ;
	dcterms:modified "2017-06-19T20:13:20+02:00" ;
	dcterms:creator "od" .

d:MEl-5b0839b90000bca801376dcca41ca7d0
	rdf:type FMC:Actor ;
	rdfs:label "Switch-off" ;
	rdfs:comment "<div><p>Switch to programmed min-value.</p> </div>" ;
	pig:revision "53" ;
	dcterms:modified "2017-06-19T20:13:20+02:00" ;
	dcterms:creator "od" .

d:MEl-5b07e6aa0000bca8013797aad9be69ae
	rdf:type FMC:Actor ;
	rdfs:label "Switch-on" ;
	rdfs:comment "<div><p>Switch to programmed max-value.</p> </div>" ;
	pig:revision "54" ;
	dcterms:modified "2017-06-19T20:13:21+02:00" ;
	dcterms:creator "od" .

d:MEl-4543fe900000c3a80141f5253ff13c35
	rdf:type FMC:Event ;
	rdfs:label "up-long!" ;
	pig:revision "91" ;
	dcterms:modified "2017-06-19T20:13:32+02:00" ;
	dcterms:creator "od" .

d:MEl-453d34af0000c3a80141918f84641161
	rdf:type FMC:Event ;
	rdfs:label "up-short!" ;
	pig:revision "92" ;
	dcterms:modified "2017-06-19T20:13:33+02:00" ;
	dcterms:creator "od" .

d:MEl-5a808e2a0000bca80137bfd74268a84a
	rdf:type FMC:Actor ;
	rdfs:label "Dimmer Electronics" ;
	rdfs:comment "<div><p>The Dimmer Electronics is a printed circuit board with low-power micro-processor, memory, binary as well as analog I/O signals and a power stage supporting the specified electric load.</p></div>" ;
	SpecIF:Diagram "<div><p class=\"inline-label\">Diagramm:</p><p><object data=\"files_and_images/Schaltplan.gif\" name=\"Schaltplan.gif\" type=\"image/gif\"/></p> </div>" ;
	pig:revision "44" ;
	dcterms:modified "2017-06-19T20:13:17+02:00" ;
	dcterms:creator "od" .

d:MEl-5a844d820000bca8013750b9a0410b6b
	rdf:type FMC:State ;
	rdfs:label "Electro-Magnetic Resistance" ;
	rdfs:comment "<div><p>Electromagnetic characteristics, especially EM-shielding.</p> </div>" ;
	pig:revision "62" ;
	dcterms:modified "2017-06-19T20:13:23+02:00" ;
	dcterms:creator "od" .

d:MEl-5a8009a00000bca80137ef95bc3f643f
	rdf:type FMC:Actor ;
	rdfs:label "Housing" ;
	SpecIF:Diagram "<div> <p class=\"inline-label\">Diagramm:</p><p><object data=\"files_and_images/UP-Dose.png\" name=\"UP-Dose.png\" type=\"image/png\"/></p> </div>" ;
	pig:revision "47" ;
	dcterms:modified "2017-06-19T20:13:18+02:00" ;
	dcterms:creator "od" .

d:MEl-5a87083e0000bca801379bb412523737
	rdf:type FMC:State ;
	rdfs:label "I/O Pins" ;
	rdfs:comment "<div><p>per input and output signal:</p> <ul> <li>hardware-address</li> <li>number of significant bits</li></ul> </div>" ;
	pig:revision "65" ;
	dcterms:modified "2017-06-19T20:13:23+02:00" ;
	dcterms:creator "od" .

d:MEl-5a82ec6f0000bca801372ef053a71bdf
	rdf:type FMC:State ;
	rdfs:label "Physical Space" ;
	rdfs:comment "<div><p>Effective 3D interior space and mounting for electronics.</p> </div>" ;
	pig:revision "70" ;
	dcterms:modified "2017-06-19T20:13:25+02:00" ;
	dcterms:creator "od" .

d:MEl-5a86b8980000bca80137ca6fde1a125e
	rdf:type FMC:State ;
	rdfs:label "Processor RAM ROM" ;
	rdfs:comment "<div><p>EPROM-Size</p> <p>RAM-Size</p> <p>Processor type with instruction set and speed (MIPS)</p> </div>" ;
	pig:revision "71" ;
	dcterms:modified "2017-06-19T20:13:25+02:00" ;
	dcterms:creator "od" .

d:MEl-5a820a3c0000bca801378c9093fb7d80
	rdf:type FMC:State ;
	rdfs:label "Thermal Resistance" ;
	rdfs:comment "<div><p> Thermal resistance and thermal capacity of the [[housing]].</p></div>" ;
	pig:revision "77" ;
	dcterms:modified "2017-06-19T20:13:27+02:00" ;
	dcterms:creator "od" .

d:MEl-5a71c4800000bca80137f2aaa7b63000
	rdf:type FMC:Actor ;
	rdfs:label "Double Button" ;
	rdfs:comment "<div><p>The Double Button (a sensor unit) is a versatile all-mechanical unit used for multiple purposes. The mechanical position is transferred with a rod per button to the next unit where it is converted to an electrical signal.</p> </div>" ;
	pig:revision "46" ;
	dcterms:modified "2017-06-19T20:13:17+02:00" ;
	dcterms:creator "od" .

d:MEl-606f16ac0000bca801373587fda932b3
	rdf:type FMC:Actor ;
	rdfs:label "Double-Button Observer Software" ;
	rdfs:comment "<div><p>This is an observer of the double-button sensor. It distinguishes short and long pressing in the 'up' and 'down' directions. A discriminator may send five events:</p> <ul> <li>up-short</li> <li>down-short</li> <li>up-long</li> <li>down-long and </li> <li>release.</li> </ul><p>The events are interpreted and actions are initiated accordingly by the target actuator unit. The double button sensor and the observer have no notion of the underlying function.</p> </div>" ;
	pig:revision "47" ;
	dcterms:modified "2017-06-19T20:13:18+02:00" ;
	dcterms:creator "od" .

d:MEl-45a236e00000c3a801410f6503287e16
	rdf:type FMC:Actor ;
	rdfs:label "Wait for Activation" ;
	rdfs:comment "<div><p>The kind of activation is determined:</p> <ul> <li>Up- or Down-Button</li> <li>Short or long activation: 'Short' is &lt; 0,4 sec.</li> <li>Do only wait until the distinction between 'short' or 'long' can be made!</li></ul> </div>" ;
	pig:revision "56" ;
	dcterms:modified "2017-06-19T20:13:21+02:00" ;
	dcterms:creator "od" .

d:MEl-45a3b13c0000c3a801415e97f5bc29d1
	rdf:type FMC:Actor ;
	rdfs:label "Wait for Deactivation" ;
	pig:revision "57" ;
	dcterms:modified "2017-06-19T20:13:21+02:00" ;
	dcterms:creator "od" .

d:MEl-5a4dd77b0000bca8013736c6912ad291
	rdf:type FMC:State ;
	rdfs:label "down" ;
	rdfs:comment "<div><p>The button to drive down the dimmer, shading or similar devices.</p> </div>" ;
	pig:revision "61" ;
	dcterms:modified "2017-06-19T20:13:22+02:00" ;
	dcterms:creator "od" .

d:MEl-5a99c89c0000bca801375d44cf9a50ca
	rdf:type FMC:State ;
	rdfs:label "Ground Cable" ;
	rdfs:comment "<div><ul> <li>Cable-diameter</li> <li>Wire-diameter</li> <li>Max-current</li></ul> </div>" ;
	pig:revision "64" ;
	dcterms:modified "2017-06-19T20:13:23+02:00" ;
	dcterms:creator "od" .

d:MEl-5a9929510000bca80137d23c81f1ca54
	rdf:type FMC:State ;
	rdfs:label "Load Cable" ;
	rdfs:comment "<div><ul> <li>Cable-diameter</li> <li>Wire-diameter</li> <li>Max-current</li></ul> </div>" ;
	pig:revision "67" ;
	dcterms:modified "2017-06-19T20:13:24+02:00" ;
	dcterms:creator "od" .

d:MEl-5c29fb8e0000bca80137eb9734c99bfd
	rdf:type FMC:State ;
	rdfs:label "Neutral Cable" ;
	rdfs:comment "<div><ul> <li>Cable-diameter</li> <li>Wire-diameter</li> <li>Max-current</li></ul> </div>" ;
	pig:revision "69" ;
	dcterms:modified "2017-06-19T20:13:24+02:00" ;
	dcterms:creator "od" .

d:MEl-5a77385f0000bca80137e1c7dc0b1721
	rdf:type FMC:State ;
	rdfs:label "Spring Clips" ;
	rdfs:comment "<div><p>Spring clips for mechanical connection.</p> </div>" ;
	pig:revision "74" ;
	dcterms:modified "2017-06-19T20:13:26+02:00" ;
	dcterms:creator "od" .

d:MEl-5a9888810000bca801375410ce1cc142
	rdf:type FMC:State ;
	rdfs:label "Supply Cable" ;
	rdfs:comment "<div><ul> <li>Cable-diameter</li> <li>Wire-diameter</li> <li>Max-current</li></ul> </div>" ;
	pig:revision "76" ;
	dcterms:modified "2017-06-19T20:13:27+02:00" ;
	dcterms:creator "od" .

d:MEl-5a4d6dee0000bca80137c1caf2f42349
	rdf:type FMC:State ;
	rdfs:label "up" ;
	rdfs:comment "<div><p>The button to drive up the dimmer, shading or similar devices.</p> </div>" ;
	pig:revision "79" ;
	dcterms:modified "2017-06-19T20:13:28+02:00" ;
	dcterms:creator "od" .

d:MEl-5a9b7a9b0000bca80137d768644696b7
	rdf:type FMC:Actor ;
	rdfs:label "Wireless Module" ;
	rdfs:comment "<div><p>Receives control commands via radio signal or the mechanical position of a mounted sensor unit. Sends electrical control signals to the mounted actuator module.</p> </div>" ;
	pig:revision "58" ;
	dcterms:modified "2017-06-19T20:13:22+02:00" ;
	dcterms:creator "od" .

d:MEl-463289cd0000c3a80141be3fc417034a
	rdf:type FMC:State ;
	rdfs:label "Wireless Network" ;
	pig:revision "80" ;
	dcterms:modified "2017-06-19T20:13:28+02:00" ;
	dcterms:creator "od" .

d:MEl-5a4c80c20000bca8013753b6999a4da8
	rdf:type FMC:State ;
	rdfs:label "Flush-mounted Shading Control" ;
	pig:revision "63" ;
	dcterms:modified "2017-06-19T20:13:23+02:00" ;
	dcterms:creator "od" .

d:MEl-5a4cfa830000bca801370d837f761f3e
	rdf:type FMC:State ;
	rdfs:label "straighten" ;
	rdfs:comment "<div><p>The button to straighten the shading elements.</p> </div>" ;
	pig:revision "75" ;
	dcterms:modified "2017-06-19T20:13:27+02:00" ;
	dcterms:creator "od" .

d:MEl-5a4d2bd00000bca80137a3f233cdffeb
	rdf:type FMC:State ;
	rdfs:label "tilt" ;
	rdfs:comment "<div><p>The button to tilt the shading elements.</p> </div>" ;
	pig:revision "78" ;
	dcterms:modified "2017-06-19T20:13:28+02:00" ;
	dcterms:creator "od" .

d:MEl-5a52b50c0000bca801377e3d15255f98
	rdf:type FMC:State ;
	rdfs:label "Intelligent Shading Drive" ;
	rdfs:comment "<div><p>An intelligent shading actuator with 2 drives for up/down straight/tilt motion. The unit comprises the control unit and the motors.</p> </div>" ;
	pig:revision "66" ;
	dcterms:modified "2017-06-19T20:13:24+02:00" ;
	dcterms:creator "od" .

d:MEl-5bcf35cf0000bca8013776d68023612a
	rdf:type FMC:State ;
	rdfs:label "M" ;
	rdfs:comment "<div><p>Actuator Motor 230V.</p> </div>" ;
	pig:revision "68" ;
	dcterms:modified "2017-06-19T20:13:24+02:00" ;
	dcterms:creator "od" .

d:MEl-5a51dd920000bca8013770a4395c83fc
	rdf:type FMC:State ;
	rdfs:label "Remote Control" ;
	pig:revision "72" ;
	dcterms:modified "2017-06-19T20:13:26+02:00" ;
	dcterms:creator "od" .

d:MEl-5a50d5b60000bca8013781532547ce93
	rdf:type FMC:Actor ;
	rdfs:label "SmartHome Controller" ;
	rdfs:comment "<div><p>The controller </p> <ul> <li>interconnects locally distributed sensors and actuators, </li> <li>coordinates different actuators where appropriate and </li> <li>performes automatic functions, such as switching external lamps dependend on ambient light.</li></ul> </div>" ;
	pig:revision "51" ;
	dcterms:modified "2017-06-19T20:13:19+02:00" ;
	dcterms:creator "od" .

d:MEl-5a47935a0000bca801377c17f8cb25b0
	rdf:type FMC:Actor ;
	rdfs:label "User" ;
	pig:revision "55" ;
	dcterms:modified "2017-06-19T20:13:21+02:00" ;
	dcterms:creator "od" .

d:MEl-608177820000bca801379179ebf3b6aa
	rdf:type FMC:Actor ;
	rdfs:label "Briefly press Down-button" ;
	rdfs:comment "<div><p>Press down-button &lt;400 ms.</p> </div>" ;
	pig:revision "40" ;
	dcterms:modified "2017-06-19T20:13:16+02:00" ;
	dcterms:creator "od" .

d:MEl-611366530000bca80137a97f194e96a3
	rdf:type FMC:Actor ;
	rdfs:label "Briefly press Up-button" ;
	rdfs:comment "<div><p>Press up-button &lt;400 ms.</p> </div>" ;
	pig:revision "41" ;
	dcterms:modified "2017-06-19T20:13:16+02:00" ;
	dcterms:creator "od" .

d:MEl-453862540000c3a801419d91bef48cfd
	rdf:type FMC:Event ;
	rdfs:label "Dim-down!" ;
	pig:revision "82" ;
	dcterms:modified "2017-06-19T20:13:29+02:00" ;
	dcterms:creator "od" .

d:MEl-45387c0b0000c3a801410aa03f6b9be4
	rdf:type FMC:Event ;
	rdfs:label "Dim-up!" ;
	pig:revision "83" ;
	dcterms:modified "2017-06-19T20:13:29+02:00" ;
	dcterms:creator "od" .

d:MEl-4538920b0000c3a801415c67e334b8a1
	rdf:type FMC:Event ;
	rdfs:label "Done!" ;
	pig:revision "83" ;
	dcterms:modified "2017-06-19T20:13:29+02:00" ;
	dcterms:creator "od" .

d:MEl-608239830000bca801373690c7d2af0f
	rdf:type FMC:Actor ;
	rdfs:label "Press and hold Down-button" ;
	rdfs:comment "<div><p>Press down-button &gt;400 ms.</p> </div>" ;
	pig:revision "48" ;
	dcterms:modified "2017-06-19T20:13:18+02:00" ;
	dcterms:creator "od" .

d:MEl-610b07100000bca80137c10f96c46247
	rdf:type FMC:Actor ;
	rdfs:label "Press and hold Up-button" ;
	rdfs:comment "<div><p>Press up-button &gt;400 ms.</p> </div>" ;
	pig:revision "49" ;
	dcterms:modified "2017-06-19T20:13:18+02:00" ;
	dcterms:creator "od" .

d:MEl-610e0b010000bca80137ac40800bb1b8
	rdf:type FMC:Actor ;
	rdfs:label "Release button" ;
	pig:revision "49" ;
	dcterms:modified "2017-06-19T20:13:18+02:00" ;
	dcterms:creator "od" .

d:MEl-459b92580000c3a80141cb4acb521ab1
	rdf:type FMC:Event ;
	rdfs:label "Stop dimming!" ;
	pig:revision "90" ;
	dcterms:modified "2017-06-19T20:13:31+02:00" ;
	dcterms:creator "od" .

d:MEl-45384cd10000c3a80141c1f85d7c26e6
	rdf:type FMC:Event ;
	rdfs:label "Switch-off!" ;
	pig:revision "91" ;
	dcterms:modified "2017-06-19T20:13:32+02:00" ;
	dcterms:creator "od" .

d:MEl-607f13b50000bca80137ba95f11856ab
	rdf:type FMC:Event ;
	rdfs:label "Switch-on!" ;
	pig:revision "91" ;
	dcterms:modified "2017-06-19T20:13:32+02:00" ;
	dcterms:creator "od" .

d:Iss-ee2abb630000c3a8013987a750219659
	rdf:type SpecIF:Issue ;
	dcterms:identifier "OPM_001" ;
	rdfs:label "An open issue with respect to mechanics" ;
	rdfs:comment "<div><p>This is the description of the issue and potential solution.</p> </div>" ;
	o:PC-IssueStatus oslc_cm:Inprogress ;
	SpecIF:Priority SpecIF:priorityLow ;
	SpecIF:DueDate "2012-09-30T12:00:00+02:00" ;
	pig:revision "35" ;
	dcterms:modified "2017-06-19T20:13:15+02:00" ;
	dcterms:creator "od" .

d:Iss-eee2d4e00000c3a801394148dcc58a52
	rdf:type SpecIF:Issue ;
	dcterms:identifier "OPS_001" ;
	rdfs:label "An open issue concerning software" ;
	rdfs:comment "<div><p>A description.</p> </div>" ;
	o:PC-IssueStatus o:V-Iss-Status-6 ;
	SpecIF:Priority SpecIF:priorityMedium ;
	SpecIF:Responsible "Vorname Nachname" ;
	SpecIF:DueDate "2012-09-30T12:00:00+02:00" ;
	pig:revision "37" ;
	dcterms:modified "2017-06-19T20:13:15+02:00" ;
	dcterms:creator "od" .

#################################################################
# Relationships
#################################################################

d:RSat-MEl-5a85347c0000bca80137ad485c7cd330-Req-d1c895230000c3a80150f8afd049f738
	rdf:type oslc_rm:satisfies ;
	oslc_rm:satisfies-toSource d:MEl-5a85347c0000bca80137ad485c7cd330 ;
	oslc_rm:satisfies-toTarget d:Req-d1c895230000c3a80150f8afd049f738 ;
	dcterms:modified "2017-06-19T20:13:49+02:00" ;
	dcterms:creator "od" .

d:R-RpgwxaijQtHjsE71uYHiTJyJW79
	rdf:type SpecIF:dependsOn ;
	SpecIF:dependsOn-toSource d:Req-d1c895230000c3a80150f8afd049f738 ;
	SpecIF:dependsOn-toTarget d:Req-d1cd7f370000c3a8015095e6ee21aab7 ;
	dcterms:modified "2017-06-19T20:13:49+02:00" ;
	dcterms:creator "od" .

d:R-tA5fx5sgbN3nJReiqqzE6PvBhbt
	rdf:type oslc_rm:satisfies ;
	oslc_rm:satisfies-toSource d:MEl-5a752ccc0000bca80137479a2e8bab30 ;
	oslc_rm:satisfies-toTarget d:Req-d1c895230000c3a80150f8afd049f738 ;
	dcterms:modified "2017-06-19T20:13:50+02:00" ;
	dcterms:creator "od" .

d:R-2hkTtbuV2BjIYernvDaRZXDFV1Q
	rdf:type oslc_rm:satisfies ;
	oslc_rm:satisfies-toSource d:MEl-5a808e2a0000bca80137bfd74268a84a ;
	oslc_rm:satisfies-toTarget d:Req-d1c895230000c3a80150f8afd049f738 ;
	dcterms:modified "2017-06-19T20:13:50+02:00" ;
	dcterms:creator "od" .

d:RSat-MEl-5a85347c0000bca80137ad485c7cd330-Req-d1d42a6a0000c3a8015091ec8d149b93
	rdf:type oslc_rm:satisfies ;
	oslc_rm:satisfies-toSource d:MEl-5a85347c0000bca80137ad485c7cd330 ;
	oslc_rm:satisfies-toTarget d:Req-d1d42a6a0000c3a8015091ec8d149b93 ;
	dcterms:modified "2017-06-19T20:13:50+02:00" ;
	dcterms:creator "od" .

d:R-Ch6fs9eKiVNhSacQ72yIBhF0Q3W
	rdf:type SpecIF:refersTo ;
	SpecIF:refersTo-toSource d:Iss-ee2abb630000c3a8013987a750219659 ;
	SpecIF:refersTo-toTarget d:Req-d1d42a6a0000c3a8015091ec8d149b93 ;
	dcterms:modified "2018-11-15T15:46:00+01:00" ;
	dcterms:creator "od" .

d:RSat-MEl-5a85347c0000bca80137ad485c7cd330-Req-d1cd7f370000c3a8015095e6ee21aab7
	rdf:type oslc_rm:satisfies ;
	oslc_rm:satisfies-toSource d:MEl-5a85347c0000bca80137ad485c7cd330 ;
	oslc_rm:satisfies-toTarget d:Req-d1cd7f370000c3a8015095e6ee21aab7 ;
	dcterms:modified "2017-06-19T20:13:51+02:00" ;
	dcterms:creator "od" .

d:RSat-MEl-5a71c4800000bca80137f2aaa7b63000-Req-5ba3512b0000bca801371cc0617eb4c1
	rdf:type oslc_rm:satisfies ;
	oslc_rm:satisfies-toSource d:MEl-5a71c4800000bca80137f2aaa7b63000 ;
	oslc_rm:satisfies-toTarget d:Req-5ba3512b0000bca801371cc0617eb4c1 ;
	dcterms:modified "2017-06-19T20:13:51+02:00" ;
	dcterms:creator "od" .

d:RSat-MEl-5a808e2a0000bca80137bfd74268a84a-Req-5b8fbb300000bca80137c73e3ce4c737
	rdf:type oslc_rm:satisfies ;
	oslc_rm:satisfies-toSource d:MEl-5a808e2a0000bca80137bfd74268a84a ;
	oslc_rm:satisfies-toTarget d:Req-5b8fbb300000bca80137c73e3ce4c737 ;
	dcterms:modified "2017-06-19T20:13:51+02:00" ;
	dcterms:creator "od" .

d:RSat-MEl-5a47935a0000bca801377c17f8cb25b0-Req-5b944fc70000bca8013763f44fdc0e03
	rdf:type oslc_rm:satisfies ;
	oslc_rm:satisfies-toSource d:MEl-5a47935a0000bca801377c17f8cb25b0 ;
	oslc_rm:satisfies-toTarget d:Req-5b944fc70000bca8013763f44fdc0e03 ;
	dcterms:modified "2017-06-19T20:13:51+02:00" ;
	dcterms:creator "od" .

d:RCnc-Iss-ee2abb630000c3a8013987a750219659-Req-5b944fc70000bca8013763f44fdc0e03
	rdf:type SpecIF:refersTo ;
	SpecIF:refersTo-toSource d:Iss-ee2abb630000c3a8013987a750219659 ;
	SpecIF:refersTo-toTarget d:Req-5b944fc70000bca8013763f44fdc0e03 ;
	dcterms:modified "2017-06-19T20:13:51+02:00" ;
	dcterms:creator "od" .

d:RSat-MEl-5a752ccc0000bca80137479a2e8bab30-Req-5ba140d60000bca801372b09f9888eca
	rdf:type oslc_rm:satisfies ;
	oslc_rm:satisfies-toSource d:MEl-5a752ccc0000bca80137479a2e8bab30 ;
	oslc_rm:satisfies-toTarget d:Req-5ba140d60000bca801372b09f9888eca ;
	dcterms:modified "2017-06-19T20:13:51+02:00" ;
	dcterms:creator "od" .

d:RSat-MEl-5a9b7a9b0000bca80137d768644696b7-Req-5ba140d60000bca801372b09f9888eca
	rdf:type oslc_rm:satisfies ;
	oslc_rm:satisfies-toSource d:MEl-5a9b7a9b0000bca80137d768644696b7 ;
	oslc_rm:satisfies-toTarget d:Req-5ba140d60000bca801372b09f9888eca ;
	dcterms:modified "2017-06-19T20:13:52+02:00" ;
	dcterms:creator "od" .

d:RSat-MEl-803fd3750000c3a8013cf1fdb3b26d33-Req-ee452cf20000c3a8014035290669304d
	rdf:type oslc_rm:satisfies ;
	oslc_rm:satisfies-toSource d:MEl-803fd3750000c3a8013cf1fdb3b26d33 ;
	oslc_rm:satisfies-toTarget d:Req-ee452cf20000c3a8014035290669304d ;
	dcterms:modified "2017-06-19T20:13:52+02:00" ;
	dcterms:creator "od" .

d:R-UZD4SQ8jYghL2Tsb4tZjoXDSYoM
	rdf:type oslc_rm:satisfies ;
	oslc_rm:satisfies-toSource d:MEl-5a752ccc0000bca80137479a2e8bab30 ;
	oslc_rm:satisfies-toTarget d:Req-ee452cf20000c3a8014035290669304d ;
	dcterms:modified "2017-06-19T20:13:52+02:00" ;
	dcterms:creator "od" .

d:RSat-MEl-5a489c300000bca80137ee1373c16844-Req-ee43fc4c0000c3a8014063d42c77767f
	rdf:type oslc_rm:satisfies ;
	oslc_rm:satisfies-toSource d:MEl-5a489c300000bca80137ee1373c16844 ;
	oslc_rm:satisfies-toTarget d:Req-ee43fc4c0000c3a8014063d42c77767f ;
	dcterms:modified "2017-06-19T20:13:52+02:00" ;
	dcterms:creator "od" .

d:RSat-MEl-5a4c80c20000bca8013753b6999a4da8-Req-ee43fc4c0000c3a8014063d42c77767f
	rdf:type oslc_rm:satisfies ;
	oslc_rm:satisfies-toSource d:MEl-5a4c80c20000bca8013753b6999a4da8 ;
	oslc_rm:satisfies-toTarget d:Req-ee43fc4c0000c3a8014063d42c77767f ;
	dcterms:modified "2017-06-19T20:13:52+02:00" ;
	dcterms:creator "od" .

d:RSat-MEl-5a52b50c0000bca801377e3d15255f98-Req-ee43fc4c0000c3a8014063d42c77767f
	rdf:type oslc_rm:satisfies ;
	oslc_rm:satisfies-toSource d:MEl-5a52b50c0000bca801377e3d15255f98 ;
	oslc_rm:satisfies-toTarget d:Req-ee43fc4c0000c3a8014063d42c77767f ;
	dcterms:modified "2017-06-19T20:13:53+02:00" ;
	dcterms:creator "od" .

d:RSat-MEl-5a50d5b60000bca8013781532547ce93-Req-ee43fc4c0000c3a8014063d42c77767f
	rdf:type oslc_rm:satisfies ;
	oslc_rm:satisfies-toSource d:MEl-5a50d5b60000bca8013781532547ce93 ;
	oslc_rm:satisfies-toTarget d:Req-ee43fc4c0000c3a8014063d42c77767f ;
	dcterms:modified "2017-06-19T20:13:53+02:00" ;
	dcterms:creator "od" .

d:RDep-Req-ee43fc4c0000c3a8014063d42c77767f-Req-5b9c950e0000bca801374f16615247b9
	rdf:type SpecIF:dependsOn ;
	SpecIF:dependsOn-toSource d:Req-ee43fc4c0000c3a8014063d42c77767f ;
	SpecIF:dependsOn-toTarget d:Req-5b9c950e0000bca801374f16615247b9 ;
	dcterms:modified "2017-06-19T20:13:53+02:00" ;
	dcterms:creator "od" .

d:RSat-MEl-5a808e2a0000bca80137bfd74268a84a-Req-5b9124bc0000bca80137fa2ce86f5eca
	rdf:type oslc_rm:satisfies ;
	oslc_rm:satisfies-toSource d:MEl-5a808e2a0000bca80137bfd74268a84a ;
	oslc_rm:satisfies-toTarget d:Req-5b9124bc0000bca80137fa2ce86f5eca ;
	dcterms:modified "2017-06-19T20:13:53+02:00" ;
	dcterms:creator "od" .

d:RSat-MEl-5a52b50c0000bca801377e3d15255f98-Req-5b9124bc0000bca80137fa2ce86f5eca
	rdf:type oslc_rm:satisfies ;
	oslc_rm:satisfies-toSource d:MEl-5a52b50c0000bca801377e3d15255f98 ;
	oslc_rm:satisfies-toTarget d:Req-5b9124bc0000bca80137fa2ce86f5eca ;
	dcterms:modified "2017-06-19T20:13:54+02:00" ;
	dcterms:creator "od" .

d:RSat-MEl-5a808e2a0000bca80137bfd74268a84a-Req-5b9e68530000bca801371362c49d2d08
	rdf:type oslc_rm:satisfies ;
	oslc_rm:satisfies-toSource d:MEl-5a808e2a0000bca80137bfd74268a84a ;
	oslc_rm:satisfies-toTarget d:Req-5b9e68530000bca801371362c49d2d08 ;
	dcterms:modified "2017-06-19T20:13:54+02:00" ;
	dcterms:creator "od" .

d:RSat-MEl-5a52b50c0000bca801377e3d15255f98-Req-5b9e68530000bca801371362c49d2d08
	rdf:type oslc_rm:satisfies ;
	oslc_rm:satisfies-toSource d:MEl-5a52b50c0000bca801377e3d15255f98 ;
	oslc_rm:satisfies-toTarget d:Req-5b9e68530000bca801371362c49d2d08 ;
	dcterms:modified "2017-06-19T20:13:54+02:00" ;
	dcterms:creator "od" .

d:RSat-MEl-803fd3750000c3a8013cf1fdb3b26d33-Req-eea1cd500000c3a80140fe00109eb7f4
	rdf:type oslc_rm:satisfies ;
	oslc_rm:satisfies-toSource d:MEl-803fd3750000c3a8013cf1fdb3b26d33 ;
	oslc_rm:satisfies-toTarget d:Req-eea1cd500000c3a80140fe00109eb7f4 ;
	dcterms:modified "2017-06-19T20:13:54+02:00" ;
	dcterms:creator "od" .

d:R-lELLVnNbbagfomwYyTBgGfXSalj
	rdf:type oslc_rm:satisfies ;
	oslc_rm:satisfies-toSource d:MEl-5a752ccc0000bca80137479a2e8bab30 ;
	oslc_rm:satisfies-toTarget d:Req-eea1cd500000c3a80140fe00109eb7f4 ;
	dcterms:modified "2017-06-19T20:13:54+02:00" ;
	dcterms:creator "od" .

d:RSat-MEl-5a489c300000bca80137ee1373c16844-Req-5b95fae40000bca801372becc933682d
	rdf:type oslc_rm:satisfies ;
	oslc_rm:satisfies-toSource d:MEl-5a489c300000bca80137ee1373c16844 ;
	oslc_rm:satisfies-toTarget d:Req-5b95fae40000bca801372becc933682d ;
	dcterms:modified "2017-06-19T20:13:54+02:00" ;
	dcterms:creator "od" .

d:RSat-MEl-5a4c80c20000bca8013753b6999a4da8-Req-5b95fae40000bca801372becc933682d
	rdf:type oslc_rm:satisfies ;
	oslc_rm:satisfies-toSource d:MEl-5a4c80c20000bca8013753b6999a4da8 ;
	oslc_rm:satisfies-toTarget d:Req-5b95fae40000bca801372becc933682d ;
	dcterms:modified "2017-06-19T20:13:55+02:00" ;
	dcterms:creator "od" .

d:RSat-MEl-5a489c300000bca80137ee1373c16844-Req-5b9ab8a50000bca801377ad0be3bbc89
	rdf:type oslc_rm:satisfies ;
	oslc_rm:satisfies-toSource d:MEl-5a489c300000bca80137ee1373c16844 ;
	oslc_rm:satisfies-toTarget d:Req-5b9ab8a50000bca801377ad0be3bbc89 ;
	dcterms:modified "2017-06-19T20:13:55+02:00" ;
	dcterms:creator "od" .

d:RSat-MEl-5a52b50c0000bca801377e3d15255f98-Req-5b9ab8a50000bca801377ad0be3bbc89
	rdf:type oslc_rm:satisfies ;
	oslc_rm:satisfies-toSource d:MEl-5a52b50c0000bca801377e3d15255f98 ;
	oslc_rm:satisfies-toTarget d:Req-5b9ab8a50000bca801377ad0be3bbc89 ;
	dcterms:modified "2017-06-19T20:13:55+02:00" ;
	dcterms:creator "od" .

d:R-NJ2iOLwt4CEpcf8IidN1z0P4d0m
	rdf:type oslc_rm:satisfies ;
	oslc_rm:satisfies-toSource d:MEl-5a752ccc0000bca80137479a2e8bab30 ;
	oslc_rm:satisfies-toTarget d:Req-5b9ab8a50000bca801377ad0be3bbc89 ;
	dcterms:modified "2017-06-19T20:13:55+02:00" ;
	dcterms:creator "od" .

d:RSat-MEl-5a808e2a0000bca80137bfd74268a84a-Req-728c69c80018b1a8014b974542c36edc
	rdf:type oslc_rm:satisfies ;
	oslc_rm:satisfies-toSource d:MEl-5a808e2a0000bca80137bfd74268a84a ;
	oslc_rm:satisfies-toTarget d:Req-728c69c80018b1a8014b974542c36edc ;
	dcterms:modified "2017-06-19T20:13:55+02:00" ;
	dcterms:creator "od" .

d:RSat-MEl-5a85347c0000bca80137ad485c7cd330-Req-5b9c950e0000bca801374f16615247b9
	rdf:type oslc_rm:satisfies ;
	oslc_rm:satisfies-toSource d:MEl-5a85347c0000bca80137ad485c7cd330 ;
	oslc_rm:satisfies-toTarget d:Req-5b9c950e0000bca801374f16615247b9 ;
	dcterms:modified "2017-06-19T20:13:55+02:00" ;
	dcterms:creator "od" .

d:RWri-MEl-5a76365c0000bca8013776e91afd1e8e-MEl-5a77385f0000bca80137e1c7dc0b1721
	rdf:type SpecIF:writes ;
	SpecIF:writes-toSource d:MEl-5a76365c0000bca8013776e91afd1e8e ;
	SpecIF:writes-toTarget d:MEl-5a77385f0000bca80137e1c7dc0b1721 ;
	dcterms:modified "2017-06-19T20:13:56+02:00" ;
	dcterms:creator "od" .

d:RRea-MEl-5a76365c0000bca8013776e91afd1e8e-MEl-5a77385f0000bca80137e1c7dc0b1721
	rdf:type SpecIF:reads ;
	SpecIF:reads-toSource d:MEl-5a76365c0000bca8013776e91afd1e8e ;
	SpecIF:reads-toTarget d:MEl-5a77385f0000bca80137e1c7dc0b1721 ;
	dcterms:modified "2017-06-19T20:13:57+02:00" ;
	dcterms:creator "od" .

d:RCtn-MEl-5a489c300000bca80137ee1373c16844-MEl-5a76365c0000bca8013776e91afd1e8e
	rdf:type SpecIF:contains ;
	SpecIF:contains-toSource d:MEl-5a489c300000bca80137ee1373c16844 ;
	SpecIF:contains-toTarget d:MEl-5a76365c0000bca8013776e91afd1e8e ;
	dcterms:modified "2017-06-19T20:13:57+02:00" ;
	dcterms:creator "od" .

d:RCtn-MEl-5a47935a0000bca801377c17f8cb25b0-MEl-608177820000bca801379179ebf3b6aa
	rdf:type SpecIF:contains ;
	SpecIF:contains-toSource d:MEl-5a47935a0000bca801377c17f8cb25b0 ;
	SpecIF:contains-toTarget d:MEl-608177820000bca801379179ebf3b6aa ;
	dcterms:modified "2017-06-19T20:13:57+02:00" ;
	dcterms:creator "od" .

d:RCtn-MEl-5a47935a0000bca801377c17f8cb25b0-MEl-611366530000bca80137a97f194e96a3
	rdf:type SpecIF:contains ;
	SpecIF:contains-toSource d:MEl-5a47935a0000bca801377c17f8cb25b0 ;
	SpecIF:contains-toTarget d:MEl-611366530000bca80137a97f194e96a3 ;
	dcterms:modified "2017-06-19T20:13:57+02:00" ;
	dcterms:creator "od" .

d:RRea-MEl-5bd6bd890000bca8013739588a3f43d6-MEl-5a489c300000bca80137ee1373c16844
	rdf:type SpecIF:reads ;
	SpecIF:reads-toSource d:MEl-5bd6bd890000bca8013739588a3f43d6 ;
	SpecIF:reads-toTarget d:MEl-5a489c300000bca80137ee1373c16844 ;
	dcterms:modified "2017-06-19T20:13:57+02:00" ;
	dcterms:creator "od" .

d:RCtn-MEl-5a85347c0000bca80137ad485c7cd330-MEl-45450be80000c3a801414f280f146c71
	rdf:type SpecIF:contains ;
	SpecIF:contains-toSource d:MEl-5a85347c0000bca80137ad485c7cd330 ;
	SpecIF:contains-toTarget d:MEl-45450be80000c3a801414f280f146c71 ;
	dcterms:modified "2017-06-19T20:13:57+02:00" ;
	dcterms:creator "od" .

d:RCtn-MEl-5a85347c0000bca80137ad485c7cd330-MEl-4536b0350000c3a801415986f8ea806a
	rdf:type SpecIF:contains ;
	SpecIF:contains-toSource d:MEl-5a85347c0000bca80137ad485c7cd330 ;
	SpecIF:contains-toTarget d:MEl-4536b0350000c3a801415986f8ea806a ;
	dcterms:modified "2017-06-19T20:13:57+02:00" ;
	dcterms:creator "od" .

d:RCtn-MEl-5a85347c0000bca80137ad485c7cd330-MEl-5b08ed8d0000bca8013719f554353b0e
	rdf:type SpecIF:contains ;
	SpecIF:contains-toSource d:MEl-5a85347c0000bca80137ad485c7cd330 ;
	SpecIF:contains-toTarget d:MEl-5b08ed8d0000bca8013719f554353b0e ;
	dcterms:modified "2017-06-19T20:13:58+02:00" ;
	dcterms:creator "od" .

d:RCtn-MEl-5a85347c0000bca80137ad485c7cd330-MEl-453dfb670000c3a8014191107df4565e
	rdf:type SpecIF:contains ;
	SpecIF:contains-toSource d:MEl-5a85347c0000bca80137ad485c7cd330 ;
	SpecIF:contains-toTarget d:MEl-453dfb670000c3a8014191107df4565e ;
	dcterms:modified "2017-06-19T20:13:58+02:00" ;
	dcterms:creator "od" .

d:RCtn-MEl-5a85347c0000bca80137ad485c7cd330-MEl-5b094f8a0000bca801374c798a6587ad
	rdf:type SpecIF:contains ;
	SpecIF:contains-toSource d:MEl-5a85347c0000bca80137ad485c7cd330 ;
	SpecIF:contains-toTarget d:MEl-5b094f8a0000bca801374c798a6587ad ;
	dcterms:modified "2017-06-19T20:13:58+02:00" ;
	dcterms:creator "od" .

d:RCtn-MEl-5a85347c0000bca80137ad485c7cd330-MEl-45428b930000c3a80141e28b7d4b5ae5
	rdf:type SpecIF:contains ;
	SpecIF:contains-toSource d:MEl-5a85347c0000bca80137ad485c7cd330 ;
	SpecIF:contains-toTarget d:MEl-45428b930000c3a80141e28b7d4b5ae5 ;
	dcterms:modified "2017-06-19T20:13:58+02:00" ;
	dcterms:creator "od" .

d:RCtn-MEl-5a85347c0000bca80137ad485c7cd330-MEl-5b078fa50000bca80137f36ed05c43cb
	rdf:type SpecIF:contains ;
	SpecIF:contains-toSource d:MEl-5a85347c0000bca80137ad485c7cd330 ;
	SpecIF:contains-toTarget d:MEl-5b078fa50000bca80137f36ed05c43cb ;
	dcterms:modified "2017-06-19T20:13:58+02:00" ;
	dcterms:creator "od" .

d:RCtn-MEl-5a85347c0000bca80137ad485c7cd330-MEl-453facbb0000c3a80141c43d2fb4f5e2
	rdf:type SpecIF:contains ;
	SpecIF:contains-toSource d:MEl-5a85347c0000bca80137ad485c7cd330 ;
	SpecIF:contains-toTarget d:MEl-453facbb0000c3a80141c43d2fb4f5e2 ;
	dcterms:modified "2017-06-19T20:13:58+02:00" ;
	dcterms:creator "od" .

d:RCtn-MEl-5a85347c0000bca80137ad485c7cd330-MEl-5b0839b90000bca801376dcca41ca7d0
	rdf:type SpecIF:contains ;
	SpecIF:contains-toSource d:MEl-5a85347c0000bca80137ad485c7cd330 ;
	SpecIF:contains-toTarget d:MEl-5b0839b90000bca801376dcca41ca7d0 ;
	dcterms:modified "2017-06-19T20:13:59+02:00" ;
	dcterms:creator "od" .

d:RCtn-MEl-5a85347c0000bca80137ad485c7cd330-MEl-5b07e6aa0000bca8013797aad9be69ae
	rdf:type SpecIF:contains ;
	SpecIF:contains-toSource d:MEl-5a85347c0000bca80137ad485c7cd330 ;
	SpecIF:contains-toTarget d:MEl-5b07e6aa0000bca8013797aad9be69ae ;
	dcterms:modified "2017-06-19T20:13:59+02:00" ;
	dcterms:creator "od" .

d:RCtn-MEl-5a85347c0000bca80137ad485c7cd330-MEl-4543fe900000c3a80141f5253ff13c35
	rdf:type SpecIF:contains ;
	SpecIF:contains-toSource d:MEl-5a85347c0000bca80137ad485c7cd330 ;
	SpecIF:contains-toTarget d:MEl-4543fe900000c3a80141f5253ff13c35 ;
	dcterms:modified "2017-06-19T20:13:59+02:00" ;
	dcterms:creator "od" .

d:RCtn-MEl-5a85347c0000bca80137ad485c7cd330-MEl-453d34af0000c3a80141918f84641161
	rdf:type SpecIF:contains ;
	SpecIF:contains-toSource d:MEl-5a85347c0000bca80137ad485c7cd330 ;
	SpecIF:contains-toTarget d:MEl-453d34af0000c3a80141918f84641161 ;
	dcterms:modified "2017-06-19T20:13:59+02:00" ;
	dcterms:creator "od" .

d:RRea-MEl-5a85347c0000bca80137ad485c7cd330-MEl-5a87083e0000bca801379bb412523737
	rdf:type SpecIF:reads ;
	SpecIF:reads-toSource d:MEl-5a85347c0000bca80137ad485c7cd330 ;
	SpecIF:reads-toTarget d:MEl-5a87083e0000bca801379bb412523737 ;
	dcterms:modified "2017-06-19T20:14:00+02:00" ;
	dcterms:creator "od" .

d:RRea-MEl-5a85347c0000bca80137ad485c7cd330-MEl-5a86b8980000bca80137ca6fde1a125e
	rdf:type SpecIF:reads ;
	SpecIF:reads-toSource d:MEl-5a85347c0000bca80137ad485c7cd330 ;
	SpecIF:reads-toTarget d:MEl-5a86b8980000bca80137ca6fde1a125e ;
	dcterms:modified "2017-06-19T20:14:00+02:00" ;
	dcterms:creator "od" .

d:RCtn-MEl-5a752ccc0000bca80137479a2e8bab30-MEl-5a85347c0000bca80137ad485c7cd330
	rdf:type SpecIF:contains ;
	SpecIF:contains-toSource d:MEl-5a752ccc0000bca80137479a2e8bab30 ;
	SpecIF:contains-toTarget d:MEl-5a85347c0000bca80137ad485c7cd330 ;
	dcterms:modified "2017-06-19T20:14:00+02:00" ;
	dcterms:creator "od" .

d:RWri-MEl-5a808e2a0000bca80137bfd74268a84a-MEl-5a99c89c0000bca801375d44cf9a50ca
	rdf:type SpecIF:writes ;
	SpecIF:writes-toSource d:MEl-5a808e2a0000bca80137bfd74268a84a ;
	SpecIF:writes-toTarget d:MEl-5a99c89c0000bca801375d44cf9a50ca ;
	dcterms:modified "2017-06-19T20:14:00+02:00" ;
	dcterms:creator "od" .

d:RRea-MEl-5a808e2a0000bca80137bfd74268a84a-MEl-5a99c89c0000bca801375d44cf9a50ca
	rdf:type SpecIF:reads ;
	SpecIF:reads-toSource d:MEl-5a808e2a0000bca80137bfd74268a84a ;
	SpecIF:reads-toTarget d:MEl-5a99c89c0000bca801375d44cf9a50ca ;
	dcterms:modified "2017-06-19T20:14:00+02:00" ;
	dcterms:creator "od" .

d:RWri-MEl-5a808e2a0000bca80137bfd74268a84a-MEl-5a9929510000bca80137d23c81f1ca54
	rdf:type SpecIF:writes ;
	SpecIF:writes-toSource d:MEl-5a808e2a0000bca80137bfd74268a84a ;
	SpecIF:writes-toTarget d:MEl-5a9929510000bca80137d23c81f1ca54 ;
	dcterms:modified "2017-06-19T20:14:01+02:00" ;
	dcterms:creator "od" .

d:RRea-MEl-5a808e2a0000bca80137bfd74268a84a-MEl-5a9929510000bca80137d23c81f1ca54
	rdf:type SpecIF:reads ;
	SpecIF:reads-toSource d:MEl-5a808e2a0000bca80137bfd74268a84a ;
	SpecIF:reads-toTarget d:MEl-5a9929510000bca80137d23c81f1ca54 ;
	dcterms:modified "2017-06-19T20:14:01+02:00" ;
	dcterms:creator "od" .

d:RWri-MEl-5a808e2a0000bca80137bfd74268a84a-MEl-5c29fb8e0000bca80137eb9734c99bfd
	rdf:type SpecIF:writes ;
	SpecIF:writes-toSource d:MEl-5a808e2a0000bca80137bfd74268a84a ;
	SpecIF:writes-toTarget d:MEl-5c29fb8e0000bca80137eb9734c99bfd ;
	dcterms:modified "2017-06-19T20:14:01+02:00" ;
	dcterms:creator "od" .

d:RRea-MEl-5a808e2a0000bca80137bfd74268a84a-MEl-5c29fb8e0000bca80137eb9734c99bfd
	rdf:type SpecIF:reads ;
	SpecIF:reads-toSource d:MEl-5a808e2a0000bca80137bfd74268a84a ;
	SpecIF:reads-toTarget d:MEl-5c29fb8e0000bca80137eb9734c99bfd ;
	dcterms:modified "2017-06-19T20:14:01+02:00" ;
	dcterms:creator "od" .

d:RWri-MEl-5a808e2a0000bca80137bfd74268a84a-MEl-5a9888810000bca801375410ce1cc142
	rdf:type SpecIF:writes ;
	SpecIF:writes-toSource d:MEl-5a808e2a0000bca80137bfd74268a84a ;
	SpecIF:writes-toTarget d:MEl-5a9888810000bca801375410ce1cc142 ;
	dcterms:modified "2017-06-19T20:14:01+02:00" ;
	dcterms:creator "od" .

d:RRea-MEl-5a808e2a0000bca80137bfd74268a84a-MEl-5a9888810000bca801375410ce1cc142
	rdf:type SpecIF:reads ;
	SpecIF:reads-toSource d:MEl-5a808e2a0000bca80137bfd74268a84a ;
	SpecIF:reads-toTarget d:MEl-5a9888810000bca801375410ce1cc142 ;
	dcterms:modified "2017-06-19T20:14:02+02:00" ;
	dcterms:creator "od" .

d:RWri-MEl-5a808e2a0000bca80137bfd74268a84a-MEl-5a86b8980000bca80137ca6fde1a125e
	rdf:type SpecIF:writes ;
	SpecIF:writes-toSource d:MEl-5a808e2a0000bca80137bfd74268a84a ;
	SpecIF:writes-toTarget d:MEl-5a86b8980000bca80137ca6fde1a125e ;
	dcterms:modified "2017-06-19T20:14:02+02:00" ;
	dcterms:creator "od" .

d:RWri-MEl-5a808e2a0000bca80137bfd74268a84a-MEl-5a87083e0000bca801379bb412523737
	rdf:type SpecIF:writes ;
	SpecIF:writes-toSource d:MEl-5a808e2a0000bca80137bfd74268a84a ;
	SpecIF:writes-toTarget d:MEl-5a87083e0000bca801379bb412523737 ;
	dcterms:modified "2017-06-19T20:14:02+02:00" ;
	dcterms:creator "od" .

d:RRea-MEl-5a808e2a0000bca80137bfd74268a84a-MEl-5a9ce0310000bca801378176dc4744e8
	rdf:type SpecIF:reads ;
	SpecIF:reads-toSource d:MEl-5a808e2a0000bca80137bfd74268a84a ;
	SpecIF:reads-toTarget d:MEl-5a9ce0310000bca801378176dc4744e8 ;
	dcterms:modified "2017-06-19T20:14:02+02:00" ;
	dcterms:creator "od" .

d:RRea-MEl-5a808e2a0000bca80137bfd74268a84a-MEl-5a820a3c0000bca801378c9093fb7d80
	rdf:type SpecIF:reads ;
	SpecIF:reads-toSource d:MEl-5a808e2a0000bca80137bfd74268a84a ;
	SpecIF:reads-toTarget d:MEl-5a820a3c0000bca801378c9093fb7d80 ;
	dcterms:modified "2017-06-19T20:14:03+02:00" ;
	dcterms:creator "od" .

d:RRea-MEl-5a808e2a0000bca80137bfd74268a84a-MEl-5a844d820000bca8013750b9a0410b6b
	rdf:type SpecIF:reads ;
	SpecIF:reads-toSource d:MEl-5a808e2a0000bca80137bfd74268a84a ;
	SpecIF:reads-toTarget d:MEl-5a844d820000bca8013750b9a0410b6b ;
	dcterms:modified "2017-06-19T20:14:03+02:00" ;
	dcterms:creator "od" .

d:RRea-MEl-5a808e2a0000bca80137bfd74268a84a-MEl-5a82ec6f0000bca801372ef053a71bdf
	rdf:type SpecIF:reads ;
	SpecIF:reads-toSource d:MEl-5a808e2a0000bca80137bfd74268a84a ;
	SpecIF:reads-toTarget d:MEl-5a82ec6f0000bca801372ef053a71bdf ;
	dcterms:modified "2017-06-19T20:14:03+02:00" ;
	dcterms:creator "od" .

d:RCtn-MEl-5a752ccc0000bca80137479a2e8bab30-MEl-5a808e2a0000bca80137bfd74268a84a
	rdf:type SpecIF:contains ;
	SpecIF:contains-toSource d:MEl-5a752ccc0000bca80137479a2e8bab30 ;
	SpecIF:contains-toTarget d:MEl-5a808e2a0000bca80137bfd74268a84a ;
	dcterms:modified "2017-06-19T20:14:04+02:00" ;
	dcterms:creator "od" .

d:RCtn-MEl-5a752ccc0000bca80137479a2e8bab30-MEl-5a8009a00000bca80137ef95bc3f643f
	rdf:type SpecIF:contains ;
	SpecIF:contains-toSource d:MEl-5a752ccc0000bca80137479a2e8bab30 ;
	SpecIF:contains-toTarget d:MEl-5a8009a00000bca80137ef95bc3f643f ;
	dcterms:modified "2017-06-19T20:14:04+02:00" ;
	dcterms:creator "od" .

d:RCtn-MEl-5a752ccc0000bca80137479a2e8bab30-MEl-5a844d820000bca8013750b9a0410b6b
	rdf:type SpecIF:contains ;
	SpecIF:contains-toSource d:MEl-5a752ccc0000bca80137479a2e8bab30 ;
	SpecIF:contains-toTarget d:MEl-5a844d820000bca8013750b9a0410b6b ;
	dcterms:modified "2017-06-19T20:14:04+02:00" ;
	dcterms:creator "od" .

d:RCtn-MEl-5a752ccc0000bca80137479a2e8bab30-MEl-5a86b8980000bca80137ca6fde1a125e
	rdf:type SpecIF:contains ;
	SpecIF:contains-toSource d:MEl-5a752ccc0000bca80137479a2e8bab30 ;
	SpecIF:contains-toTarget d:MEl-5a86b8980000bca80137ca6fde1a125e ;
	dcterms:modified "2017-06-19T20:14:04+02:00" ;
	dcterms:creator "od" .

d:RCtn-MEl-5a752ccc0000bca80137479a2e8bab30-MEl-5a87083e0000bca801379bb412523737
	rdf:type SpecIF:contains ;
	SpecIF:contains-toSource d:MEl-5a752ccc0000bca80137479a2e8bab30 ;
	SpecIF:contains-toTarget d:MEl-5a87083e0000bca801379bb412523737 ;
	dcterms:modified "2017-06-19T20:14:04+02:00" ;
	dcterms:creator "od" .

d:RCtn-MEl-5a752ccc0000bca80137479a2e8bab30-MEl-5a82ec6f0000bca801372ef053a71bdf
	rdf:type SpecIF:contains ;
	SpecIF:contains-toSource d:MEl-5a752ccc0000bca80137479a2e8bab30 ;
	SpecIF:contains-toTarget d:MEl-5a82ec6f0000bca801372ef053a71bdf ;
	dcterms:modified "2017-06-19T20:14:04+02:00" ;
	dcterms:creator "od" .

d:RCtn-MEl-5a752ccc0000bca80137479a2e8bab30-MEl-5a820a3c0000bca801378c9093fb7d80
	rdf:type SpecIF:contains ;
	SpecIF:contains-toSource d:MEl-5a752ccc0000bca80137479a2e8bab30 ;
	SpecIF:contains-toTarget d:MEl-5a820a3c0000bca801378c9093fb7d80 ;
	dcterms:modified "2017-06-19T20:14:05+02:00" ;
	dcterms:creator "od" .

d:RRea-MEl-5a752ccc0000bca80137479a2e8bab30-MEl-5a9ce0310000bca801378176dc4744e8
	rdf:type SpecIF:reads ;
	SpecIF:reads-toSource d:MEl-5a752ccc0000bca80137479a2e8bab30 ;
	SpecIF:reads-toTarget d:MEl-5a9ce0310000bca801378176dc4744e8 ;
	dcterms:modified "2017-06-19T20:14:05+02:00" ;
	dcterms:creator "od" .

d:RCtn-MEl-5a489c300000bca80137ee1373c16844-MEl-5a752ccc0000bca80137479a2e8bab30
	rdf:type SpecIF:contains ;
	SpecIF:contains-toSource d:MEl-5a489c300000bca80137ee1373c16844 ;
	SpecIF:contains-toTarget d:MEl-5a752ccc0000bca80137479a2e8bab30 ;
	dcterms:modified "2017-06-19T20:14:05+02:00" ;
	dcterms:creator "od" .

d:RWri-MEl-5a71c4800000bca80137f2aaa7b63000-MEl-5a77385f0000bca80137e1c7dc0b1721
	rdf:type SpecIF:writes ;
	SpecIF:writes-toSource d:MEl-5a71c4800000bca80137f2aaa7b63000 ;
	SpecIF:writes-toTarget d:MEl-5a77385f0000bca80137e1c7dc0b1721 ;
	dcterms:modified "2017-06-19T20:14:06+02:00" ;
	dcterms:creator "od" .

d:RRea-MEl-5a71c4800000bca80137f2aaa7b63000-MEl-5a77385f0000bca80137e1c7dc0b1721
	rdf:type SpecIF:reads ;
	SpecIF:reads-toSource d:MEl-5a71c4800000bca80137f2aaa7b63000 ;
	SpecIF:reads-toTarget d:MEl-5a77385f0000bca80137e1c7dc0b1721 ;
	dcterms:modified "2017-06-19T20:14:06+02:00" ;
	dcterms:creator "od" .

d:RWri-MEl-5a71c4800000bca80137f2aaa7b63000-MEl-5a7776c50000bca8013765ae93af9209
	rdf:type SpecIF:writes ;
	SpecIF:writes-toSource d:MEl-5a71c4800000bca80137f2aaa7b63000 ;
	SpecIF:writes-toTarget d:MEl-5a7776c50000bca8013765ae93af9209 ;
	dcterms:modified "2017-06-19T20:14:06+02:00" ;
	dcterms:creator "od" .

d:RRea-MEl-5a71c4800000bca80137f2aaa7b63000-MEl-5a4dd77b0000bca8013736c6912ad291
	rdf:type SpecIF:reads ;
	SpecIF:reads-toSource d:MEl-5a71c4800000bca80137f2aaa7b63000 ;
	SpecIF:reads-toTarget d:MEl-5a4dd77b0000bca8013736c6912ad291 ;
	dcterms:modified "2017-06-19T20:14:06+02:00" ;
	dcterms:creator "od" .

d:RRea-MEl-5a71c4800000bca80137f2aaa7b63000-MEl-5a4d6dee0000bca80137c1caf2f42349
	rdf:type SpecIF:reads ;
	SpecIF:reads-toSource d:MEl-5a71c4800000bca80137f2aaa7b63000 ;
	SpecIF:reads-toTarget d:MEl-5a4d6dee0000bca80137c1caf2f42349 ;
	dcterms:modified "2017-06-19T20:14:06+02:00" ;
	dcterms:creator "od" .

d:RCtn-MEl-5a489c300000bca80137ee1373c16844-MEl-5a71c4800000bca80137f2aaa7b63000
	rdf:type SpecIF:contains ;
	SpecIF:contains-toSource d:MEl-5a489c300000bca80137ee1373c16844 ;
	SpecIF:contains-toTarget d:MEl-5a71c4800000bca80137f2aaa7b63000 ;
	dcterms:modified "2017-06-19T20:14:07+02:00" ;
	dcterms:creator "od" .

d:RCtn-MEl-606f16ac0000bca801373587fda932b3-MEl-45450be80000c3a801414f280f146c71
	rdf:type SpecIF:contains ;
	SpecIF:contains-toSource d:MEl-606f16ac0000bca801373587fda932b3 ;
	SpecIF:contains-toTarget d:MEl-45450be80000c3a801414f280f146c71 ;
	dcterms:modified "2017-06-19T20:14:07+02:00" ;
	dcterms:creator "od" .

d:RCtn-MEl-606f16ac0000bca801373587fda932b3-MEl-4536b0350000c3a801415986f8ea806a
	rdf:type SpecIF:contains ;
	SpecIF:contains-toSource d:MEl-606f16ac0000bca801373587fda932b3 ;
	SpecIF:contains-toTarget d:MEl-4536b0350000c3a801415986f8ea806a ;
	dcterms:modified "2017-06-19T20:14:07+02:00" ;
	dcterms:creator "od" .

d:RCtn-MEl-606f16ac0000bca801373587fda932b3-MEl-453facbb0000c3a80141c43d2fb4f5e2
	rdf:type SpecIF:contains ;
	SpecIF:contains-toSource d:MEl-606f16ac0000bca801373587fda932b3 ;
	SpecIF:contains-toTarget d:MEl-453facbb0000c3a80141c43d2fb4f5e2 ;
	dcterms:modified "2017-06-19T20:14:07+02:00" ;
	dcterms:creator "od" .

d:RCtn-MEl-606f16ac0000bca801373587fda932b3-MEl-4543fe900000c3a80141f5253ff13c35
	rdf:type SpecIF:contains ;
	SpecIF:contains-toSource d:MEl-606f16ac0000bca801373587fda932b3 ;
	SpecIF:contains-toTarget d:MEl-4543fe900000c3a80141f5253ff13c35 ;
	dcterms:modified "2017-06-19T20:14:08+02:00" ;
	dcterms:creator "od" .

d:RCtn-MEl-606f16ac0000bca801373587fda932b3-MEl-453d34af0000c3a80141918f84641161
	rdf:type SpecIF:contains ;
	SpecIF:contains-toSource d:MEl-606f16ac0000bca801373587fda932b3 ;
	SpecIF:contains-toTarget d:MEl-453d34af0000c3a80141918f84641161 ;
	dcterms:modified "2017-06-19T20:14:08+02:00" ;
	dcterms:creator "od" .

d:RCtn-MEl-606f16ac0000bca801373587fda932b3-MEl-45a236e00000c3a801410f6503287e16
	rdf:type SpecIF:contains ;
	SpecIF:contains-toSource d:MEl-606f16ac0000bca801373587fda932b3 ;
	SpecIF:contains-toTarget d:MEl-45a236e00000c3a801410f6503287e16 ;
	dcterms:modified "2017-06-19T20:14:08+02:00" ;
	dcterms:creator "od" .

d:RCtn-MEl-606f16ac0000bca801373587fda932b3-MEl-45a3b13c0000c3a801415e97f5bc29d1
	rdf:type SpecIF:contains ;
	SpecIF:contains-toSource d:MEl-606f16ac0000bca801373587fda932b3 ;
	SpecIF:contains-toTarget d:MEl-45a3b13c0000c3a801415e97f5bc29d1 ;
	dcterms:modified "2017-06-19T20:14:08+02:00" ;
	dcterms:creator "od" .

d:RCnc-Iss-ee2abb630000c3a8013987a750219659-MEl-5a8009a00000bca80137ef95bc3f643f
	rdf:type SpecIF:refersTo ;
	SpecIF:refersTo-toSource d:Iss-ee2abb630000c3a8013987a750219659 ;
	SpecIF:refersTo-toTarget d:MEl-5a8009a00000bca80137ef95bc3f643f ;
	dcterms:modified "2017-06-19T20:13:56+02:00" ;
	dcterms:creator "od" .

d:RWri-MEl-5a8009a00000bca80137ef95bc3f643f-MEl-5a77385f0000bca80137e1c7dc0b1721
	rdf:type SpecIF:writes ;
	SpecIF:writes-toSource d:MEl-5a8009a00000bca80137ef95bc3f643f ;
	SpecIF:writes-toTarget d:MEl-5a77385f0000bca80137e1c7dc0b1721 ;
	dcterms:modified "2017-06-19T20:14:08+02:00" ;
	dcterms:creator "od" .

d:RRea-MEl-5a8009a00000bca80137ef95bc3f643f-MEl-5a77385f0000bca80137e1c7dc0b1721
	rdf:type SpecIF:reads ;
	SpecIF:reads-toSource d:MEl-5a8009a00000bca80137ef95bc3f643f ;
	SpecIF:reads-toTarget d:MEl-5a77385f0000bca80137e1c7dc0b1721 ;
	dcterms:modified "2017-06-19T20:14:08+02:00" ;
	dcterms:creator "od" .

d:RWri-MEl-5a8009a00000bca80137ef95bc3f643f-MEl-5a844d820000bca8013750b9a0410b6b
	rdf:type SpecIF:writes ;
	SpecIF:writes-toSource d:MEl-5a8009a00000bca80137ef95bc3f643f ;
	SpecIF:writes-toTarget d:MEl-5a844d820000bca8013750b9a0410b6b ;
	dcterms:modified "2017-06-19T20:14:09+02:00" ;
	dcterms:creator "od" .

d:RWri-MEl-5a8009a00000bca80137ef95bc3f643f-MEl-5a82ec6f0000bca801372ef053a71bdf
	rdf:type SpecIF:writes ;
	SpecIF:writes-toSource d:MEl-5a8009a00000bca80137ef95bc3f643f ;
	SpecIF:writes-toTarget d:MEl-5a82ec6f0000bca801372ef053a71bdf ;
	dcterms:modified "2017-06-19T20:14:09+02:00" ;
	dcterms:creator "od" .

d:RWri-MEl-5a8009a00000bca80137ef95bc3f643f-MEl-5a820a3c0000bca801378c9093fb7d80
	rdf:type SpecIF:writes ;
	SpecIF:writes-toSource d:MEl-5a8009a00000bca80137ef95bc3f643f ;
	SpecIF:writes-toTarget d:MEl-5a820a3c0000bca801378c9093fb7d80 ;
	dcterms:modified "2017-06-19T20:14:09+02:00" ;
	dcterms:creator "od" .

d:RCtn-MEl-5a47935a0000bca801377c17f8cb25b0-MEl-608239830000bca801373690c7d2af0f
	rdf:type SpecIF:contains ;
	SpecIF:contains-toSource d:MEl-5a47935a0000bca801377c17f8cb25b0 ;
	SpecIF:contains-toTarget d:MEl-608239830000bca801373690c7d2af0f ;
	dcterms:modified "2017-06-19T20:14:10+02:00" ;
	dcterms:creator "od" .

d:RCtn-MEl-5a47935a0000bca801377c17f8cb25b0-MEl-610b07100000bca80137c10f96c46247
	rdf:type SpecIF:contains ;
	SpecIF:contains-toSource d:MEl-5a47935a0000bca801377c17f8cb25b0 ;
	SpecIF:contains-toTarget d:MEl-610b07100000bca80137c10f96c46247 ;
	dcterms:modified "2017-06-19T20:14:10+02:00" ;
	dcterms:creator "od" .

d:RCtn-MEl-5a47935a0000bca801377c17f8cb25b0-MEl-610e0b010000bca80137ac40800bb1b8
	rdf:type SpecIF:contains ;
	SpecIF:contains-toSource d:MEl-5a47935a0000bca801377c17f8cb25b0 ;
	SpecIF:contains-toTarget d:MEl-610e0b010000bca80137ac40800bb1b8 ;
	dcterms:modified "2017-06-19T20:14:10+02:00" ;
	dcterms:creator "od" .

d:RRea-MEl-5bcfb01d0000bca80137f303272a5557-MEl-5a52b50c0000bca801377e3d15255f98
	rdf:type SpecIF:reads ;
	SpecIF:reads-toSource d:MEl-5bcfb01d0000bca80137f303272a5557 ;
	SpecIF:reads-toTarget d:MEl-5a52b50c0000bca801377e3d15255f98 ;
	dcterms:modified "2017-06-19T20:14:10+02:00" ;
	dcterms:creator "od" .

d:RWri-MEl-5a50d5b60000bca8013781532547ce93-MEl-5a489c300000bca80137ee1373c16844
	rdf:type SpecIF:writes ;
	SpecIF:writes-toSource d:MEl-5a50d5b60000bca8013781532547ce93 ;
	SpecIF:writes-toTarget d:MEl-5a489c300000bca80137ee1373c16844 ;
	dcterms:modified "2017-06-19T20:14:10+02:00" ;
	dcterms:creator "od" .

d:RRea-MEl-5a50d5b60000bca8013781532547ce93-MEl-5a489c300000bca80137ee1373c16844
	rdf:type SpecIF:reads ;
	SpecIF:reads-toSource d:MEl-5a50d5b60000bca8013781532547ce93 ;
	SpecIF:reads-toTarget d:MEl-5a489c300000bca80137ee1373c16844 ;
	dcterms:modified "2017-06-19T20:14:11+02:00" ;
	dcterms:creator "od" .

d:RWri-MEl-5a50d5b60000bca8013781532547ce93-MEl-5a52b50c0000bca801377e3d15255f98
	rdf:type SpecIF:writes ;
	SpecIF:writes-toSource d:MEl-5a50d5b60000bca8013781532547ce93 ;
	SpecIF:writes-toTarget d:MEl-5a52b50c0000bca801377e3d15255f98 ;
	dcterms:modified "2017-06-19T20:14:11+02:00" ;
	dcterms:creator "od" .

d:RRea-MEl-5a50d5b60000bca8013781532547ce93-MEl-5a4c80c20000bca8013753b6999a4da8
	rdf:type SpecIF:reads ;
	SpecIF:reads-toSource d:MEl-5a50d5b60000bca8013781532547ce93 ;
	SpecIF:reads-toTarget d:MEl-5a4c80c20000bca8013753b6999a4da8 ;
	dcterms:modified "2017-06-19T20:14:11+02:00" ;
	dcterms:creator "od" .

d:RRea-MEl-5a50d5b60000bca8013781532547ce93-MEl-5a51dd920000bca8013770a4395c83fc
	rdf:type SpecIF:reads ;
	SpecIF:reads-toSource d:MEl-5a50d5b60000bca8013781532547ce93 ;
	SpecIF:reads-toTarget d:MEl-5a51dd920000bca8013770a4395c83fc ;
	dcterms:modified "2017-06-19T20:14:11+02:00" ;
	dcterms:creator "od" .

d:RCtn-MEl-803fd3750000c3a8013cf1fdb3b26d33-MEl-5a50d5b60000bca8013781532547ce93
	rdf:type SpecIF:contains ;
	SpecIF:contains-toSource d:MEl-803fd3750000c3a8013cf1fdb3b26d33 ;
	SpecIF:contains-toTarget d:MEl-5a50d5b60000bca8013781532547ce93 ;
	dcterms:modified "2017-06-19T20:14:11+02:00" ;
	dcterms:creator "od" .

d:RCtn-MEl-5a47935a0000bca801377c17f8cb25b0-MEl-453862540000c3a801419d91bef48cfd
	rdf:type SpecIF:contains ;
	SpecIF:contains-toSource d:MEl-5a47935a0000bca801377c17f8cb25b0 ;
	SpecIF:contains-toTarget d:MEl-453862540000c3a801419d91bef48cfd ;
	dcterms:modified "2017-06-19T20:14:12+02:00" ;
	dcterms:creator "od" .

d:RCtn-MEl-5a47935a0000bca801377c17f8cb25b0-MEl-45387c0b0000c3a801410aa03f6b9be4
	rdf:type SpecIF:contains ;
	SpecIF:contains-toSource d:MEl-5a47935a0000bca801377c17f8cb25b0 ;
	SpecIF:contains-toTarget d:MEl-45387c0b0000c3a801410aa03f6b9be4 ;
	dcterms:modified "2017-06-19T20:14:12+02:00" ;
	dcterms:creator "od" .

d:RCtn-MEl-5a47935a0000bca801377c17f8cb25b0-MEl-4538920b0000c3a801415c67e334b8a1
	rdf:type SpecIF:contains ;
	SpecIF:contains-toSource d:MEl-5a47935a0000bca801377c17f8cb25b0 ;
	SpecIF:contains-toTarget d:MEl-4538920b0000c3a801415c67e334b8a1 ;
	dcterms:modified "2017-06-19T20:14:12+02:00" ;
	dcterms:creator "od" .

d:RCtn-MEl-5a47935a0000bca801377c17f8cb25b0-MEl-459b92580000c3a80141cb4acb521ab1
	rdf:type SpecIF:contains ;
	SpecIF:contains-toSource d:MEl-5a47935a0000bca801377c17f8cb25b0 ;
	SpecIF:contains-toTarget d:MEl-459b92580000c3a80141cb4acb521ab1 ;
	dcterms:modified "2017-06-19T20:14:13+02:00" ;
	dcterms:creator "od" .

d:RCtn-MEl-5a47935a0000bca801377c17f8cb25b0-MEl-607f13b50000bca80137ba95f11856ab
	rdf:type SpecIF:contains ;
	SpecIF:contains-toSource d:MEl-5a47935a0000bca801377c17f8cb25b0 ;
	SpecIF:contains-toTarget d:MEl-607f13b50000bca80137ba95f11856ab ;
	dcterms:modified "2017-06-19T20:14:13+02:00" ;
	dcterms:creator "od" .

d:RCtn-MEl-5a47935a0000bca801377c17f8cb25b0-MEl-45384cd10000c3a80141c1f85d7c26e6
	rdf:type SpecIF:contains ;
	SpecIF:contains-toSource d:MEl-5a47935a0000bca801377c17f8cb25b0 ;
	SpecIF:contains-toTarget d:MEl-45384cd10000c3a80141c1f85d7c26e6 ;
	dcterms:modified "2017-06-19T20:14:13+02:00" ;
	dcterms:creator "od" .

d:RWri-MEl-5a47935a0000bca801377c17f8cb25b0-MEl-5a51dd920000bca8013770a4395c83fc
	rdf:type SpecIF:writes ;
	SpecIF:writes-toSource d:MEl-5a47935a0000bca801377c17f8cb25b0 ;
	SpecIF:writes-toTarget d:MEl-5a51dd920000bca8013770a4395c83fc ;
	dcterms:modified "2017-06-19T20:14:14+02:00" ;
	dcterms:creator "od" .

d:RWri-MEl-5a47935a0000bca801377c17f8cb25b0-MEl-5a4c80c20000bca8013753b6999a4da8
	rdf:type SpecIF:writes ;
	SpecIF:writes-toSource d:MEl-5a47935a0000bca801377c17f8cb25b0 ;
	SpecIF:writes-toTarget d:MEl-5a4c80c20000bca8013753b6999a4da8 ;
	dcterms:modified "2017-06-19T20:14:14+02:00" ;
	dcterms:creator "od" .

d:RWri-MEl-5a47935a0000bca801377c17f8cb25b0-MEl-5a489c300000bca80137ee1373c16844
	rdf:type SpecIF:writes ;
	SpecIF:writes-toSource d:MEl-5a47935a0000bca801377c17f8cb25b0 ;
	SpecIF:writes-toTarget d:MEl-5a489c300000bca80137ee1373c16844 ;
	dcterms:modified "2017-06-19T20:14:14+02:00" ;
	dcterms:creator "od" .

d:RCtn-MEl-5a489c300000bca80137ee1373c16844-MEl-5a9b7a9b0000bca80137d768644696b7
	rdf:type SpecIF:contains ;
	SpecIF:contains-toSource d:MEl-5a489c300000bca80137ee1373c16844 ;
	SpecIF:contains-toTarget d:MEl-5a9b7a9b0000bca80137d768644696b7 ;
	dcterms:modified "2017-06-19T20:14:14+02:00" ;
	dcterms:creator "od" .

d:RWri-MEl-5a9b7a9b0000bca80137d768644696b7-MEl-5a77385f0000bca80137e1c7dc0b1721
	rdf:type SpecIF:writes ;
	SpecIF:writes-toSource d:MEl-5a9b7a9b0000bca80137d768644696b7 ;
	SpecIF:writes-toTarget d:MEl-5a77385f0000bca80137e1c7dc0b1721 ;
	dcterms:modified "2017-06-19T20:14:14+02:00" ;
	dcterms:creator "od" .

d:RRea-MEl-5a9b7a9b0000bca80137d768644696b7-MEl-5a77385f0000bca80137e1c7dc0b1721
	rdf:type SpecIF:reads ;
	SpecIF:reads-toSource d:MEl-5a9b7a9b0000bca80137d768644696b7 ;
	SpecIF:reads-toTarget d:MEl-5a77385f0000bca80137e1c7dc0b1721 ;
	dcterms:modified "2017-06-19T20:14:15+02:00" ;
	dcterms:creator "od" .

d:RWri-MEl-5a9b7a9b0000bca80137d768644696b7-MEl-463289cd0000c3a80141be3fc417034a
	rdf:type SpecIF:writes ;
	SpecIF:writes-toSource d:MEl-5a9b7a9b0000bca80137d768644696b7 ;
	SpecIF:writes-toTarget d:MEl-463289cd0000c3a80141be3fc417034a ;
	dcterms:modified "2017-06-19T20:14:15+02:00" ;
	dcterms:creator "od" .

d:RRea-MEl-5a9b7a9b0000bca80137d768644696b7-MEl-463289cd0000c3a80141be3fc417034a
	rdf:type SpecIF:reads ;
	SpecIF:reads-toSource d:MEl-5a9b7a9b0000bca80137d768644696b7 ;
	SpecIF:reads-toTarget d:MEl-463289cd0000c3a80141be3fc417034a ;
	dcterms:modified "2017-06-19T20:14:15+02:00" ;
	dcterms:creator "od" .

d:RWri-MEl-5a9b7a9b0000bca80137d768644696b7-MEl-5a9ce0310000bca801378176dc4744e8
	rdf:type SpecIF:writes ;
	SpecIF:writes-toSource d:MEl-5a9b7a9b0000bca80137d768644696b7 ;
	SpecIF:writes-toTarget d:MEl-5a9ce0310000bca801378176dc4744e8 ;
	dcterms:modified "2017-06-19T20:14:15+02:00" ;
	dcterms:creator "od" .

d:RRea-MEl-5a9b7a9b0000bca80137d768644696b7-MEl-5a7776c50000bca8013765ae93af9209
	rdf:type SpecIF:reads ;
	SpecIF:reads-toSource d:MEl-5a9b7a9b0000bca80137d768644696b7 ;
	SpecIF:reads-toTarget d:MEl-5a7776c50000bca8013765ae93af9209 ;
	dcterms:modified "2017-06-19T20:14:16+02:00" ;
	dcterms:creator "od" .

d:RCtn-MEl-5a489c300000bca80137ee1373c16844-MEl-5a7776c50000bca8013765ae93af9209
	rdf:type SpecIF:contains ;
	SpecIF:contains-toSource d:MEl-5a489c300000bca80137ee1373c16844 ;
	SpecIF:contains-toTarget d:MEl-5a7776c50000bca8013765ae93af9209 ;
	dcterms:modified "2017-06-19T20:14:16+02:00" ;
	dcterms:creator "od" .

d:RCtn-MEl-5a489c300000bca80137ee1373c16844-MEl-5a9ce0310000bca801378176dc4744e8
	rdf:type SpecIF:contains ;
	SpecIF:contains-toSource d:MEl-5a489c300000bca80137ee1373c16844 ;
	SpecIF:contains-toTarget d:MEl-5a9ce0310000bca801378176dc4744e8 ;
	dcterms:modified "2017-06-19T20:14:16+02:00" ;
	dcterms:creator "od" .

d:RCtn-MEl-5a489c300000bca80137ee1373c16844-MEl-5a4dd77b0000bca8013736c6912ad291
	rdf:type SpecIF:contains ;
	SpecIF:contains-toSource d:MEl-5a489c300000bca80137ee1373c16844 ;
	SpecIF:contains-toTarget d:MEl-5a4dd77b0000bca8013736c6912ad291 ;
	dcterms:modified "2017-06-19T20:14:16+02:00" ;
	dcterms:creator "od" .

d:RCtn-MEl-5a4c80c20000bca8013753b6999a4da8-MEl-5a4dd77b0000bca8013736c6912ad291
	rdf:type SpecIF:contains ;
	SpecIF:contains-toSource d:MEl-5a4c80c20000bca8013753b6999a4da8 ;
	SpecIF:contains-toTarget d:MEl-5a4dd77b0000bca8013736c6912ad291 ;
	dcterms:modified "2017-06-19T20:14:16+02:00" ;
	dcterms:creator "od" .

d:RCtn-MEl-5a51dd920000bca8013770a4395c83fc-MEl-5a4dd77b0000bca8013736c6912ad291
	rdf:type SpecIF:contains ;
	SpecIF:contains-toSource d:MEl-5a51dd920000bca8013770a4395c83fc ;
	SpecIF:contains-toTarget d:MEl-5a4dd77b0000bca8013736c6912ad291 ;
	dcterms:modified "2017-06-19T20:14:16+02:00" ;
	dcterms:creator "od" .

d:RCtn-MEl-5a489c300000bca80137ee1373c16844-MEl-5a4d6dee0000bca80137c1caf2f42349
	rdf:type SpecIF:contains ;
	SpecIF:contains-toSource d:MEl-5a489c300000bca80137ee1373c16844 ;
	SpecIF:contains-toTarget d:MEl-5a4d6dee0000bca80137c1caf2f42349 ;
	dcterms:modified "2017-06-19T20:14:17+02:00" ;
	dcterms:creator "od" .

d:RCtn-MEl-5a489c300000bca80137ee1373c16844-MEl-5a77385f0000bca80137e1c7dc0b1721
	rdf:type SpecIF:contains ;
	SpecIF:contains-toSource d:MEl-5a489c300000bca80137ee1373c16844 ;
	SpecIF:contains-toTarget d:MEl-5a77385f0000bca80137e1c7dc0b1721 ;
	dcterms:modified "2017-06-19T20:14:17+02:00" ;
	dcterms:creator "od" .

d:RCtn-MEl-803fd3750000c3a8013cf1fdb3b26d33-MEl-5a489c300000bca80137ee1373c16844
	rdf:type SpecIF:contains ;
	SpecIF:contains-toSource d:MEl-803fd3750000c3a8013cf1fdb3b26d33 ;
	SpecIF:contains-toTarget d:MEl-5a489c300000bca80137ee1373c16844 ;
	dcterms:modified "2017-06-19T20:14:17+02:00" ;
	dcterms:creator "od" .

d:RCtn-MEl-5a4c80c20000bca8013753b6999a4da8-MEl-5a4d6dee0000bca80137c1caf2f42349
	rdf:type SpecIF:contains ;
	SpecIF:contains-toSource d:MEl-5a4c80c20000bca8013753b6999a4da8 ;
	SpecIF:contains-toTarget d:MEl-5a4d6dee0000bca80137c1caf2f42349 ;
	dcterms:modified "2017-06-19T20:14:18+02:00" ;
	dcterms:creator "od" .

d:RCtn-MEl-5a4c80c20000bca8013753b6999a4da8-MEl-5a4cfa830000bca801370d837f761f3e
	rdf:type SpecIF:contains ;
	SpecIF:contains-toSource d:MEl-5a4c80c20000bca8013753b6999a4da8 ;
	SpecIF:contains-toTarget d:MEl-5a4cfa830000bca801370d837f761f3e ;
	dcterms:modified "2017-06-19T20:14:18+02:00" ;
	dcterms:creator "od" .

d:RCtn-MEl-5a4c80c20000bca8013753b6999a4da8-MEl-5a4d2bd00000bca80137a3f233cdffeb
	rdf:type SpecIF:contains ;
	SpecIF:contains-toSource d:MEl-5a4c80c20000bca8013753b6999a4da8 ;
	SpecIF:contains-toTarget d:MEl-5a4d2bd00000bca80137a3f233cdffeb ;
	dcterms:modified "2017-06-19T20:14:18+02:00" ;
	dcterms:creator "od" .

d:RCtn-MEl-803fd3750000c3a8013cf1fdb3b26d33-MEl-5a4c80c20000bca8013753b6999a4da8
	rdf:type SpecIF:contains ;
	SpecIF:contains-toSource d:MEl-803fd3750000c3a8013cf1fdb3b26d33 ;
	SpecIF:contains-toTarget d:MEl-5a4c80c20000bca8013753b6999a4da8 ;
	dcterms:modified "2017-06-19T20:14:19+02:00" ;
	dcterms:creator "od" .

d:RCtn-MEl-5a52b50c0000bca801377e3d15255f98-MEl-5bcf35cf0000bca8013776d68023612a
	rdf:type SpecIF:contains ;
	SpecIF:contains-toSource d:MEl-5a52b50c0000bca801377e3d15255f98 ;
	SpecIF:contains-toTarget d:MEl-5bcf35cf0000bca8013776d68023612a ;
	dcterms:modified "2017-06-19T20:14:19+02:00" ;
	dcterms:creator "od" .

d:RCtn-MEl-803fd3750000c3a8013cf1fdb3b26d33-MEl-5a52b50c0000bca801377e3d15255f98
	rdf:type SpecIF:contains ;
	SpecIF:contains-toSource d:MEl-803fd3750000c3a8013cf1fdb3b26d33 ;
	SpecIF:contains-toTarget d:MEl-5a52b50c0000bca801377e3d15255f98 ;
	dcterms:modified "2017-06-19T20:14:19+02:00" ;
	dcterms:creator "od" .

d:R-vxkoenpgAX6s6PxskSWlYPN8e4y
	rdf:type SpecIF:refersTo ;
	SpecIF:refersTo-toSource d:Iss-eee2d4e00000c3a801394148dcc58a52 ;
	SpecIF:refersTo-toTarget d:MEl-5a51dd920000bca8013770a4395c83fc ;
	dcterms:modified "2017-06-19T20:13:56+02:00" ;
	dcterms:creator "od" .

d:RCtn-MEl-5a51dd920000bca8013770a4395c83fc-MEl-5a4d6dee0000bca80137c1caf2f42349
	rdf:type SpecIF:contains ;
	SpecIF:contains-toSource d:MEl-5a51dd920000bca8013770a4395c83fc ;
	SpecIF:contains-toTarget d:MEl-5a4d6dee0000bca80137c1caf2f42349 ;
	dcterms:modified "2017-06-19T20:14:19+02:00" ;
	dcterms:creator "od" .

d:RCtn-MEl-803fd3750000c3a8013cf1fdb3b26d33-MEl-5a51dd920000bca8013770a4395c83fc
	rdf:type SpecIF:contains ;
	SpecIF:contains-toSource d:MEl-803fd3750000c3a8013cf1fdb3b26d33 ;
	SpecIF:contains-toTarget d:MEl-5a51dd920000bca8013770a4395c83fc ;
	dcterms:modified "2017-06-19T20:14:19+02:00" ;
	dcterms:creator "od" .

#################################################################
# Hierarchy
#################################################################

d:HierarchyRoot-ACP-59c8a7730000bca80137509a49b1218b
	rdf:type pig:HierarchyRoot ;
	dcterms:modified "2026-01-17T22:39:33.891Z" ;
	rdfs:label "Hierarchy Root" ;
	rdfs:comment "... anchoring all hierarchies of this graph (package)" ;
	pig:lists (
			d:HR-Fld-59c8a7730000bca80137509a49b1218b-info
			d:HR-Fld-5a5f54090000bca801375b04a668f1a7
			d:HR-Fld-5af3154d0000bca801379748537d7388
			d:HR-Fld-5b8e98550000bca801371afb0c7b671b
			d:HR-Fld-59c8a7730000bca80137509a49b1218b
			d:HR-k9qMB6fnxPTk942dvPKdyvnwnoQ
			d:HR-FolderGlossary-8001804519
		) .

d:HR-Fld-59c8a7730000bca80137509a49b1218b-info
	rdf:type pig:Outline ;
	rdfs:label "Dimmer - Semantically Integrated Specification (2021-01-28)" ;
	rdfs:comment "This specification method integrates and represents:\n- processes, system composition and requirements (dynamic, static and detail views)\n- mechanic, electric and software components with their interfaces.\n\nIt is important to understand, that all plans (diagrams) are views of a common system engineering model, sometimes called 'system repository'. Thus, consistency is always maintained.\n\nThe model elements are connected with relations, most of which are defined by positioning graph elements. For example, if a system component is drawn within another, a relationship 'contains' is created in the logic representation of the engineering model. Other relations, such as a system component 'satisfies' a requirement are created manually.  \n\nAlso, the documents are generated from the system engineering model. The ordering is in most projects (it can be rearranged, however, if appropriate):\n- All plans\n- A glossary with descriptions of all model elements appearing on one or more plans\n- A hierarchically ordered list of requirements\n- A list of open issues.\nPlease note that plans list related model elements and model elements list related requirements .. and vice versa. Active hyper-links are used, so that it is easy to jump between related model elements.\n\nFurther information is given in Appendix 'Method'." ;
	pig:category ReqIF:HierarchyRoot ;
	dcterms:modified "2026-01-17T22:39:33.435Z" ;
	pig:lists (
			d:Fld-59c8a7730000bca80137509a49b1218b-info
		) .

d:Fld-59c8a7730000bca80137509a49b1218b-info
	rdf:type pig:Outline ;
	rdfs:label "Project Information" ;
	rdfs:comment "<div> <p> <a href=\"https://enso-managers.de\" ><object data=\"files_and_images/enso-logo.png\" type=\"image/png\" >enso managers gmbh</object></a> </p> <p> This is a small show-case illustrating the basic concepts for integrated mechatronic system specification. In addition to the original text and diagrams you will find logical relations between the information elements. Most relations are derived automatically from the diagrams; the resulting semantic net lends itself for navigation, search and audit. </p> <p> The specification integrates and represents: </p><ul><li>processes, system composition and requirements (dynamic, static and detail views) </li><li>mechanic, electric and software components with their interfaces. </li></ul><p>It is an important characteristic, that all plans (diagrams) are views of a common system engineering model, sometimes called 'system repository'. Thus, consistency is always maintained. </p><p>The model elements are connected with relations, most of which are defined by positioning graph elements. For example, if a system component is drawn within another, a relationship 'contains' is created in the logic representation of the engineering model. Other relations, such as a system component 'satisfies' a requirement are created manually. </p><p>Also, the documents are generated from the system engineering model. The ordering is in most projects (it can be rearranged, however, if appropriate): </p><ul><li> All plans </li><li> A glossary with descriptions of all model elements appearing on one or more plans </li><li> A hierarchically ordered list of requirements </li> <li> A list of open issues. </li></ul><p> Please note that plans list related model elements and model elements list related requirements .. and vice versa. Active hyper-links are used, so that it is easy to jump between related model elements. </p><p><br/></p><p><strong>Stakeholders:</strong></p><table class=\"stdInlineWithBorder\"> <tbody> <tr> <th> Name </th><th>Organisation</th><th> Telephone </th> <th> Email </th> </tr> <tr> <td> Dr. Oskar v. Dungern </td> <td>enso managers GmbH</td> <td> </td> <td><a href=\"mailto:od@enso-managers.de\" >od@enso-managers.de</a></td> </tr> </tbody> </table> <p> <br /> </p> <p><strong>Legend:</strong> </p> <p> To distinguish their type, element names are preceded by one of the following symbols: </p> <table class=\"stdInlineWithBorder\"> <tbody> <tr> <td> ▣ </td><td> Plan </td> <td> A 'Diagram' is a graphical model view with a specific communication purpose, e.g. a business process or system composition. </td></tr><tr> <td> ■ </td><td> Actor (Role, Function) </td> <td> An 'Actor' is a fundamental model element type representing an active entity, be it an activity, a process step, a function, a system component or a role. </td> </tr> <tr> <td> ● </td> <td> State (Information) </td> <td> A 'State' is a fundamental model element type representing a passive entity, be it a value, a condition, an information storage or even a physical shape. </td> </tr> <tr> <td> ♦ </td> <td> Event </td> <td> An 'Event' is a fundamental model element type representing a time reference, a change in condition/value or more generally a synchronisation primitive. </td> </tr> <tr> <td> ✶ </td> <td> Feature </td> <td> A 'Feature' is an intentional distinguishing characteristic of a system, often a unique selling proposition. </td> </tr> <tr> <td> ↯ </td> <td> Requirement </td> <td> A 'Requirement' is a singular documented physical and functional need that a particular design, product or process must be able to perform. </td> </tr> </tbody> </table> <p class=\"sceditor-nlf\"> <br /> </p></div>" ;
	pig:revision "254" ;
	dcterms:modified "2018-05-04T17:18:18+02:00" ;
	dcterms:creator "od" .

d:HR-Fld-5a5f54090000bca801375b04a668f1a7
	rdf:type pig:Outline ;
	rdfs:label "Dimmer - Semantically Integrated Specification (2021-01-28)" ;
	rdfs:comment "This specification method integrates and represents:\n- processes, system composition and requirements (dynamic, static and detail views)\n- mechanic, electric and software components with their interfaces.\n\nIt is important to understand, that all plans (diagrams) are views of a common system engineering model, sometimes called 'system repository'. Thus, consistency is always maintained.\n\nThe model elements are connected with relations, most of which are defined by positioning graph elements. For example, if a system component is drawn within another, a relationship 'contains' is created in the logic representation of the engineering model. Other relations, such as a system component 'satisfies' a requirement are created manually.  \n\nAlso, the documents are generated from the system engineering model. The ordering is in most projects (it can be rearranged, however, if appropriate):\n- All plans\n- A glossary with descriptions of all model elements appearing on one or more plans\n- A hierarchically ordered list of requirements\n- A list of open issues.\nPlease note that plans list related model elements and model elements list related requirements .. and vice versa. Active hyper-links are used, so that it is easy to jump between related model elements.\n\nFurther information is given in Appendix 'Method'." ;
	pig:category ReqIF:HierarchyRoot ;
	dcterms:modified "2026-01-17T22:39:33.435Z" ;
	pig:lists (
			d:Fld-5a5f54090000bca801375b04a668f1a7
		) .

d:Fld-5a5f54090000bca801375b04a668f1a7
	rdf:type pig:Outline ;
	rdfs:label "System Composition" ;
	rdfs:comment "<div><p>.. showing the system and its composition of modules (at a higher level) and components (at a lower level). The relevant interfaces between the disciplines mechanical, electrical and software engineering are shown.</p> </div>" ;
	pig:revision "13" ;
	dcterms:modified "2017-06-19T20:13:02+02:00" ;
	dcterms:creator "od" ;
	pig:lists (
			d:Pln-27420ffc0000c3a8013ab527ca1b71f5
			d:Pln-5a4755dd0000bca801375293a62c90a8
			d:Pln-5a6cdea50000bca80137d6b2d6e8a3a0
			d:Pln-5a7f99af0000bca8013754f2ef12d3e5
		) .

d:HR-Fld-5af3154d0000bca801379748537d7388
	rdf:type pig:Outline ;
	rdfs:label "Dimmer - Semantically Integrated Specification (2021-01-28)" ;
	rdfs:comment "This specification method integrates and represents:\n- processes, system composition and requirements (dynamic, static and detail views)\n- mechanic, electric and software components with their interfaces.\n\nIt is important to understand, that all plans (diagrams) are views of a common system engineering model, sometimes called 'system repository'. Thus, consistency is always maintained.\n\nThe model elements are connected with relations, most of which are defined by positioning graph elements. For example, if a system component is drawn within another, a relationship 'contains' is created in the logic representation of the engineering model. Other relations, such as a system component 'satisfies' a requirement are created manually.  \n\nAlso, the documents are generated from the system engineering model. The ordering is in most projects (it can be rearranged, however, if appropriate):\n- All plans\n- A glossary with descriptions of all model elements appearing on one or more plans\n- A hierarchically ordered list of requirements\n- A list of open issues.\nPlease note that plans list related model elements and model elements list related requirements .. and vice versa. Active hyper-links are used, so that it is easy to jump between related model elements.\n\nFurther information is given in Appendix 'Method'." ;
	pig:category ReqIF:HierarchyRoot ;
	dcterms:modified "2026-01-17T22:39:33.435Z" ;
	pig:lists (
			d:Fld-5af3154d0000bca801379748537d7388
		) .

d:Fld-5af3154d0000bca801379748537d7388
	rdf:type pig:Outline ;
	rdfs:label "Scenarios" ;
	rdfs:comment "<div><p>.. showing the behavioral aspects of system design, both from external user perspective ('black box') and from internal perspective ('white box').</p> </div>" ;
	pig:revision "13" ;
	dcterms:modified "2017-06-19T20:13:02+02:00" ;
	dcterms:creator "od" ;
	pig:lists (
			d:Fld-5b6a99f10000bca80137b78cda65fc07
		) .

d:Fld-5b6a99f10000bca80137b78cda65fc07
	rdf:type pig:Outline ;
	rdfs:label "Dimming" ;
	pig:revision "20" ;
	dcterms:modified "2017-06-19T20:13:04+02:00" ;
	dcterms:creator "od" ;
	pig:lists (
			d:Pln-606e76c70000bca801376ec3133a1181
			d:Pln-45a1c8930000c3a801414cd1eaa70b5a
			d:Pln-5af364560000bca80137b84017f4e832
		) .

d:HR-Fld-5b8e98550000bca801371afb0c7b671b
	rdf:type pig:Outline ;
	rdfs:label "Dimmer - Semantically Integrated Specification (2021-01-28)" ;
	rdfs:comment "This specification method integrates and represents:\n- processes, system composition and requirements (dynamic, static and detail views)\n- mechanic, electric and software components with their interfaces.\n\nIt is important to understand, that all plans (diagrams) are views of a common system engineering model, sometimes called 'system repository'. Thus, consistency is always maintained.\n\nThe model elements are connected with relations, most of which are defined by positioning graph elements. For example, if a system component is drawn within another, a relationship 'contains' is created in the logic representation of the engineering model. Other relations, such as a system component 'satisfies' a requirement are created manually.  \n\nAlso, the documents are generated from the system engineering model. The ordering is in most projects (it can be rearranged, however, if appropriate):\n- All plans\n- A glossary with descriptions of all model elements appearing on one or more plans\n- A hierarchically ordered list of requirements\n- A list of open issues.\nPlease note that plans list related model elements and model elements list related requirements .. and vice versa. Active hyper-links are used, so that it is easy to jump between related model elements.\n\nFurther information is given in Appendix 'Method'." ;
	pig:category ReqIF:HierarchyRoot ;
	dcterms:modified "2026-01-17T22:39:33.435Z" ;
	pig:lists (
			d:Fld-5b8e98550000bca801371afb0c7b671b
		) .

d:Fld-5b8e98550000bca801371afb0c7b671b
	rdf:type pig:Outline ;
	rdfs:label "Requirements" ;
	pig:revision "14" ;
	dcterms:modified "2017-06-19T20:13:02+02:00" ;
	dcterms:creator "od" ;
	pig:lists (
			d:Fld-d1b1698a0000c3a801505b1b5698b7a1
			d:Fld-d1b1d6c60000c3a80150fe9ce40e6588
			d:Fld-d1b314890000c3a80150b71a1473d374
		) .

d:Fld-d1b1698a0000c3a801505b1b5698b7a1
	rdf:type pig:Outline ;
	rdfs:label "Function" ;
	rdfs:comment "<div><p>The requirements related to the product function.</p> </div>" ;
	pig:revision "22" ;
	dcterms:modified "2017-06-19T20:13:06+02:00" ;
	dcterms:creator "od" ;
	pig:lists (
			d:Req-d1c895230000c3a80150f8afd049f738
			d:Req-d1d42a6a0000c3a8015091ec8d149b93
			d:Req-d1cd7f370000c3a8015095e6ee21aab7
			d:Req-5ba3512b0000bca801371cc0617eb4c1
			d:Req-5b8fbb300000bca80137c73e3ce4c737
		) .

d:Fld-d1b1d6c60000c3a80150fe9ce40e6588
	rdf:type pig:Outline ;
	rdfs:label "Quality" ;
	rdfs:comment "<div><p>The requirements related to quality characteristics of the product.</p> </div>" ;
	pig:revision "25" ;
	dcterms:modified "2017-06-19T20:13:08+02:00" ;
	dcterms:creator "od" ;
	pig:lists (
			d:Req-5b944fc70000bca8013763f44fdc0e03
			d:Req-5ba140d60000bca801372b09f9888eca
			d:Req-ee452cf20000c3a8014035290669304d
			d:Req-ee43fc4c0000c3a8014063d42c77767f
			d:Req-5b9124bc0000bca80137fa2ce86f5eca
			d:Req-5b9e68530000bca801371362c49d2d08
		) .

d:Fld-d1b314890000c3a80150b71a1473d374
	rdf:type pig:Outline ;
	rdfs:label "Constraints" ;
	rdfs:comment "<div><p>The requirements related to constraints for product conception, such as regulations or technical choices made upfront.</p> </div>" ;
	pig:revision "30" ;
	dcterms:modified "2017-06-19T20:13:12+02:00" ;
	dcterms:creator "od" ;
	pig:lists (
			d:Req-eea1cd500000c3a80140fe00109eb7f4
			d:Req-5b95fae40000bca801372becc933682d
			d:Req-5b9ab8a50000bca801377ad0be3bbc89
			d:Req-728c69c80018b1a8014b974542c36edc
			d:Req-5b9c950e0000bca801374f16615247b9
		) .

d:HR-Fld-59c8a7730000bca80137509a49b1218b
	rdf:type pig:Outline ;
	rdfs:label "Dimmer - Semantically Integrated Specification (2021-01-28)" ;
	rdfs:comment "This specification method integrates and represents:\n- processes, system composition and requirements (dynamic, static and detail views)\n- mechanic, electric and software components with their interfaces.\n\nIt is important to understand, that all plans (diagrams) are views of a common system engineering model, sometimes called 'system repository'. Thus, consistency is always maintained.\n\nThe model elements are connected with relations, most of which are defined by positioning graph elements. For example, if a system component is drawn within another, a relationship 'contains' is created in the logic representation of the engineering model. Other relations, such as a system component 'satisfies' a requirement are created manually.  \n\nAlso, the documents are generated from the system engineering model. The ordering is in most projects (it can be rearranged, however, if appropriate):\n- All plans\n- A glossary with descriptions of all model elements appearing on one or more plans\n- A hierarchically ordered list of requirements\n- A list of open issues.\nPlease note that plans list related model elements and model elements list related requirements .. and vice versa. Active hyper-links are used, so that it is easy to jump between related model elements.\n\nFurther information is given in Appendix 'Method'." ;
	pig:category ReqIF:HierarchyRoot ;
	dcterms:modified "2026-01-17T22:39:33.435Z" ;
	pig:lists (
			d:Fld-59c8a7730000bca80137509a49b1218b
		) .

d:Fld-59c8a7730000bca80137509a49b1218b
	rdf:type pig:Outline ;
	rdfs:label "Parts List" ;
	rdfs:comment "<div>This Parts List has been automatically generated from the model. </div>" ;
	pig:revision "17" ;
	dcterms:modified "2017-06-19T20:13:02+02:00" ;
	dcterms:creator "od" ;
	pig:lists (
			d:MEl-5bd6bd890000bca8013739588a3f43d6
			d:MEl-5bcfb01d0000bca80137f303272a5557
			d:MEl-803fd3750000c3a8013cf1fdb3b26d33
			d:MEl-5a47935a0000bca801377c17f8cb25b0
		) .

d:HR-k9qMB6fnxPTk942dvPKdyvnwnoQ
	rdf:type pig:Outline ;
	rdfs:label "Dimmer - Semantically Integrated Specification (2021-01-28)" ;
	rdfs:comment "This specification method integrates and represents:\n- processes, system composition and requirements (dynamic, static and detail views)\n- mechanic, electric and software components with their interfaces.\n\nIt is important to understand, that all plans (diagrams) are views of a common system engineering model, sometimes called 'system repository'. Thus, consistency is always maintained.\n\nThe model elements are connected with relations, most of which are defined by positioning graph elements. For example, if a system component is drawn within another, a relationship 'contains' is created in the logic representation of the engineering model. Other relations, such as a system component 'satisfies' a requirement are created manually.  \n\nAlso, the documents are generated from the system engineering model. The ordering is in most projects (it can be rearranged, however, if appropriate):\n- All plans\n- A glossary with descriptions of all model elements appearing on one or more plans\n- A hierarchically ordered list of requirements\n- A list of open issues.\nPlease note that plans list related model elements and model elements list related requirements .. and vice versa. Active hyper-links are used, so that it is easy to jump between related model elements.\n\nFurther information is given in Appendix 'Method'." ;
	pig:category ReqIF:HierarchyRoot ;
	dcterms:modified "2026-01-17T22:39:33.435Z" ;
	pig:lists (
			d:Fld-ef47e6970000c3a80139dc747c5df319
		) .

d:Fld-ef47e6970000c3a80139dc747c5df319
	rdf:type pig:Outline ;
	rdfs:label "Open Issues" ;
	pig:revision "15" ;
	dcterms:modified "2017-06-19T20:13:02+02:00" ;
	dcterms:creator "od" ;
	pig:lists (
			d:Fld-ee29463e0000c3a80139627bbced50ae
			d:Fld-ee2a15040000c3a80139d27de6704f15
		) .

d:Fld-ee29463e0000c3a80139627bbced50ae
	rdf:type pig:Outline ;
	rdfs:label "Mechanical" ;
	pig:revision "34" ;
	dcterms:modified "2017-06-19T20:13:14+02:00" ;
	dcterms:creator "od" ;
	pig:lists (
			d:Iss-ee2abb630000c3a8013987a750219659
		) .

d:Fld-ee2a15040000c3a80139d27de6704f15
	rdf:type pig:Outline ;
	rdfs:label "Software" ;
	pig:revision "36" ;
	dcterms:modified "2017-06-19T20:13:15+02:00" ;
	dcterms:creator "od" ;
	pig:lists (
			d:Iss-eee2d4e00000c3a801394148dcc58a52
		) .

d:HR-FolderGlossary-8001804519
	rdf:type pig:Outline ;
	rdfs:label "Dimmer - Semantically Integrated Specification (2021-01-28)" ;
	rdfs:comment "This specification method integrates and represents:\n- processes, system composition and requirements (dynamic, static and detail views)\n- mechanic, electric and software components with their interfaces.\n\nIt is important to understand, that all plans (diagrams) are views of a common system engineering model, sometimes called 'system repository'. Thus, consistency is always maintained.\n\nThe model elements are connected with relations, most of which are defined by positioning graph elements. For example, if a system component is drawn within another, a relationship 'contains' is created in the logic representation of the engineering model. Other relations, such as a system component 'satisfies' a requirement are created manually.  \n\nAlso, the documents are generated from the system engineering model. The ordering is in most projects (it can be rearranged, however, if appropriate):\n- All plans\n- A glossary with descriptions of all model elements appearing on one or more plans\n- A hierarchically ordered list of requirements\n- A list of open issues.\nPlease note that plans list related model elements and model elements list related requirements .. and vice versa. Active hyper-links are used, so that it is easy to jump between related model elements.\n\nFurther information is given in Appendix 'Method'." ;
	pig:category ReqIF:HierarchyRoot ;
	dcterms:modified "2026-01-17T22:39:33.435Z" ;
	pig:lists (
			d:FolderGlossary-8001804519
		) .

d:FolderGlossary-8001804519
	rdf:type pig:Outline ;
	rdfs:label "Model Elements (Glossary)" ;
	pig:category SpecIF:Glossary ;
	dcterms:modified "2026-01-17T22:39:20.717Z" ;
	pig:lists (
			d:MEl-5a7776c50000bca8013765ae93af9209
			d:MEl-5a76365c0000bca8013776e91afd1e8e
			d:MEl-608177820000bca801379179ebf3b6aa
			d:MEl-611366530000bca80137a97f194e96a3
			d:MEl-5bd6bd890000bca8013739588a3f43d6
			d:MEl-5a9ce0310000bca801378176dc4744e8
			d:MEl-5b2f95ec0000bca8013709bfa81d701f
			d:MEl-453862540000c3a801419d91bef48cfd
			d:MEl-45387c0b0000c3a801410aa03f6b9be4
			d:MEl-5a85347c0000bca80137ad485c7cd330
			d:MEl-5a808e2a0000bca80137bfd74268a84a
			d:MEl-5a752ccc0000bca80137479a2e8bab30
			d:MEl-4538920b0000c3a801415c67e334b8a1
			d:MEl-5a71c4800000bca80137f2aaa7b63000
			d:MEl-606f16ac0000bca801373587fda932b3
			d:MEl-5a4dd77b0000bca8013736c6912ad291
			d:MEl-45450be80000c3a801414f280f146c71
			d:MEl-4536b0350000c3a801415986f8ea806a
			d:MEl-5a844d820000bca8013750b9a0410b6b
			d:MEl-5a489c300000bca80137ee1373c16844
			d:MEl-5a4c80c20000bca8013753b6999a4da8
			d:MEl-5a99c89c0000bca801375d44cf9a50ca
			d:MEl-5a8009a00000bca80137ef95bc3f643f
			d:MEl-5a87083e0000bca801379bb412523737
			d:MEl-5b149eab0000bca80137aad99b6eea7b
			d:MEl-5a52b50c0000bca801377e3d15255f98
			d:MEl-5b08ed8d0000bca8013719f554353b0e
			d:MEl-5a9929510000bca80137d23c81f1ca54
			d:MEl-5bcf35cf0000bca8013776d68023612a
			d:MEl-453dfb670000c3a8014191107df4565e
			d:MEl-5b094f8a0000bca801374c798a6587ad
			d:MEl-45428b930000c3a80141e28b7d4b5ae5
			d:MEl-5b078fa50000bca80137f36ed05c43cb
			d:MEl-5c29fb8e0000bca80137eb9734c99bfd
			d:MEl-5a82ec6f0000bca801372ef053a71bdf
			d:MEl-608239830000bca801373690c7d2af0f
			d:MEl-610b07100000bca80137c10f96c46247
			d:MEl-5a86b8980000bca80137ca6fde1a125e
			d:MEl-610e0b010000bca80137ac40800bb1b8
			d:MEl-453facbb0000c3a80141c43d2fb4f5e2
			d:MEl-5a51dd920000bca8013770a4395c83fc
			d:MEl-5bcfb01d0000bca80137f303272a5557
			d:MEl-5a50d5b60000bca8013781532547ce93
			d:MEl-803fd3750000c3a8013cf1fdb3b26d33
			d:MEl-5a77385f0000bca80137e1c7dc0b1721
			d:MEl-5b2d29070000bca801378a6c020cf8f5
			d:MEl-5b1750f80000bca801373b2d143d7478
			d:MEl-459b92580000c3a80141cb4acb521ab1
			d:MEl-5b2ddad80000bca80137c44d62ba97d8
			d:MEl-5b2449180000bca8013722c01c9d35a5
			d:MEl-5a4cfa830000bca801370d837f761f3e
			d:MEl-5a9888810000bca801375410ce1cc142
			d:MEl-5b0839b90000bca801376dcca41ca7d0
			d:MEl-45384cd10000c3a80141c1f85d7c26e6
			d:MEl-5b07e6aa0000bca8013797aad9be69ae
			d:MEl-607f13b50000bca80137ba95f11856ab
			d:MEl-5a820a3c0000bca801378c9093fb7d80
			d:MEl-5a4d2bd00000bca80137a3f233cdffeb
			d:MEl-5a4d6dee0000bca80137c1caf2f42349
			d:MEl-4543fe900000c3a80141f5253ff13c35
			d:MEl-453d34af0000c3a80141918f84641161
			d:MEl-5a47935a0000bca801377c17f8cb25b0
			d:MEl-45a236e00000c3a801410f6503287e16
			d:MEl-45a3b13c0000c3a801415e97f5bc29d1
			d:MEl-5a9b7a9b0000bca80137d768644696b7
			d:MEl-463289cd0000c3a80141be3fc417034a
		) .
