{
  "@context": {
    "rdf": "http://www.w3.org/1999/02/22-rdf-syntax-ns#",
    "rdfs": "http://www.w3.org/2000/01/rdf-schema#",
    "owl": "http://www.w3.org/2002/07/owl#",
    "sh": "http://www.w3.org/ns/shacl#",
    "dcterms": "http://purl.org/dc/terms/",
    "W3C": "https://www.w3.org/standards/semanticweb#",
    "pig": "https://product-information-graph.org/schema/#",
    "DDP": "http://www.prostep.org/dictionary/2.0#",
    "SpecIF": "https://specif.de/v1.1/schema#"
  },
  "@graph": [
    {
      "@id": "https://product-information-graph.org/examples/Dictionary.xsd#",
      "@type": "owl:Ontology",
      "rdfs:comment": "Ontology derived from DDP Schema Version 2.0 created 10.03.2023 08:09:28 by Michael Kirsch, :em engineering methods AG on behalf of prostep iViP Association",
      "rdfs:label": "Ontology as defined by prostep iViP DDP",
      "owl:imports": [
        {
          "@id": "http://www.w3.org/1999/02/22-rdf-syntax-ns#"
        },
        {
          "@id": "http://www.w3.org/2000/01/rdf-schema#"
        }
      ]
    },
    {
      "@id": "DDP:Person",
      "@type": "owl:Class",
      "dcterms:modified": "2025-07-25T13:51:29.486Z",
      "rdfs:comment": "Represents a real person, but may also be a system user that appears in source data. The FOAF (Friend of a Friend) Ontology has been considered, but is not used as it does not provide a structured representation for firstname, lastname and title of a person.",
      "rdfs:label": "Person",
      "rdfs:subClassOf": {
        "@id": "owl:Thing"
      },
      "pig:itemType": {
        "@id": "pig:EntityClass"
      }
    },
    {
      "@id": "DDP:Employee",
      "@type": "owl:Class",
      "dcterms:modified": "2025-07-25T13:51:29.486Z",
      "rdfs:label": "Employee",
      "rdfs:subClassOf": {
        "@id": "DDP:Person"
      },
      "pig:itemType": {
        "@id": "pig:EntityClass"
      }
    },
    {
      "@id": "DDP:Role",
      "@type": "owl:Class",
      "dcterms:modified": "2025-07-25T13:51:29.486Z",
      "rdfs:comment": "A defined function to be performed by a project team member, such as testing, filing, inspecting, coding.https://intranet.prostep.org/display/PROJ/Glossary",
      "rdfs:label": "Role",
      "rdfs:subClassOf": {
        "@id": "owl:Thing"
      },
      "pig:itemType": {
        "@id": "pig:EntityClass"
      }
    },
    {
      "@id": "DDP:OrganizationUnit",
      "@type": "owl:Class",
      "dcterms:modified": "2025-07-25T13:51:29.486Z",
      "rdfs:comment": "An organization unit is part of a corporate structure. It comprises persons as well as sub-organization units.",
      "rdfs:label": "OrganizationUnit",
      "rdfs:subClassOf": {
        "@id": "owl:Thing"
      },
      "pig:itemType": {
        "@id": "pig:EntityClass"
      }
    },
    {
      "@id": "https://product-information-graph.org/examples/Dictionary.xsd#R-q0Oh7DFaqgCY5RdaEQWAtBv1MNS",
      "@type": "DDP:Employee",
      "dcterms:modified": "2025-07-25T13:55:57.846Z",
      "DDP:firstname": "Anouk",
      "DDP:lastname": "Aim√©e",
      "DDP:phone": "0033 12 345678",
      "pig:itemType": {
        "@id": "pig:Entity"
      }
    },
    {
      "@id": "pig:Entity",
      "@type": "owl:Class"
    },
    {
      "@id": "pig:EntityClass",
      "@type": "owl:Class"
    },
    {
      "@id": "pig:itemType",
      "@type": "owl:ObjectProperty",
      "rdfs:label": "has PIG metamodel item type",
      "rdfs:range": [
        {
          "@id": "pig:OrganizerClass"
        },
        {
          "@id": "pig:Organizer"
        },
        {
          "@id": "pig:EntityClass"
        },
        {
          "@id": "pig:Entity"
        },
        {
          "@id": "pig:RelationshipClass"
        },
        {
          "@id": "pig:Relationship"
        },
        {
          "@id": "pig:PropertyClass"
        }
      ]
    }
  ]
}