
@prefix rdf: <http://www.w3.org/1999/02/22-rdf-syntax-ns#> .
@prefix rdfs: <http://www.w3.org/2000/01/rdf-schema#> .
@prefix owl: <http://www.w3.org/2002/07/owl#> .
@prefix sh: <http://www.w3.org/ns/shacl#> .
@prefix xs: <http://www.w3.org/2001/XMLSchema#> .
@prefix dcterms: <http://purl.org/dc/terms/> .
@prefix schema: <http://schema.org/> .
@prefix pig: <https://product-information-graph.org/ontology/2026-01-20/foundation#> .
@prefix pigShapes_rdfs: <https://product-information-graph.org/ontology/2026-01-20/shapes/rdfs#> .
@prefix pigShapes_schema: <https://product-information-graph.org/ontology/2026-01-20/shapes/schema#> .
@prefix pigShapes_pig: <https://product-information-graph.org/ontology/2026-01-20/shapes/pig#> .

@prefix o: <https://alice.org/ontology#> .
@prefix d: <https://alice.org/data#> .

#################################################################
# Project Metadata
#################################################################

pig:
	rdf:type owl:Ontology ;
	rdfs:label "CASCaRA Foundation" ;
	rdfs:comment "Attaches the CASCaRA Ontology to the metamodel items" ;
	owl:imports <http://www.w3.org/1999/02/22-rdf-syntax-ns#> ,
		<http://www.w3.org/2000/01/rdf-schema#> ;
	dcterms:license <https://creativecommons.org/licenses/by-sa/4.0/> ;
	dcterms:modified "2026-01-20T09:38:26.464Z" .

#################################################################
# PIG Metamodel (pig:)
#################################################################

pig:Entity
	rdf:type owl:Class ;
	rdfs:label "Entity" ;
	rdfs:comment "A PIG meta-model item used for entities (aka resources or artifacts)." .

pigShapes_pig:Entity
	rdf:type sh:NodeShape ;
	sh:targetClass pig:Entity ;
	sh:property pigShapes_rdfs:label ,
		pigShapes_rdfs:comment ,
		pigShapes_pig:category ,
		pigShapes_pig:icon .

pig:Organizer
	rdfs:subClassOf pig:Entity ;
	rdfs:label "Organizer" ;
	rdfs:comment "An element organizing model elements. An example is a list of requirements or a diagram using a certain notation." .

pigShapes_pig:Organizer
	rdf:type sh:NodeShape ;
	sh:targetClass pig:Organizer ;
	sh:property pigShapes_rdfs:label ,
		pigShapes_rdfs:comment ,
		pigShapes_pig:category .

pig:HierarchyRoot
	rdfs:subClassOf pig:Organizer ;
	rdfs:label "Hierarchy Root" ;
	rdfs:comment "A subclass of PIG organizer serving as a root for hierarchically organized graph elements." .

pigShapes_pig:HierarchyRoot
	rdf:type sh:NodeShape ;
	sh:targetClass pig:HierarchyRoot ;
	sh:property pigShapes_rdfs:label ,
		pigShapes_rdfs:comment ,
		pigShapes_pig:lists .

pig:Outline
	rdfs:subClassOf pig:Organizer ;
	rdfs:label "Outline" ;
	rdfs:comment "A subclass of PIG organizer comprising all information items of a human-readable document. As usual, the outline is hierarchically organized." .

pigShapes_pig:Outline
	rdf:type sh:NodeShape ;
	sh:targetClass pig:Outline ;
	sh:property pigShapes_rdfs:label ,
		pigShapes_rdfs:comment ,
		pigShapes_pig:category ,
		pigShapes_pig:lists .

pig:View
	rdfs:subClassOf pig:Organizer ;
	rdfs:label "View" ;
	rdfs:comment "A subclass of PIG organizer representing a model view (diagram) using a certain notation showing selected model elements." .

pigShapes_pig:View
	rdf:type sh:NodeShape ;
	sh:targetClass pig:View ;
	sh:property pigShapes_rdfs:label ,
		pigShapes_rdfs:comment ,
		pigShapes_pig:category ,
		pigShapes_pig:icon ,
		pigShapes_pig:shows ,
		pigShapes_pig:depicts .

pig:Relationship
	rdf:type owl:Class ;
	rdfs:label "Relationship" ;
	rdfs:comment "A PIG meta-model item used for reified relationships (aka predicates)." .

pigShapes_pig:Relationship
	rdf:type sh:NodeShape ;
	sh:targetClass pig:Relationship ;
	sh:property pigShapes_rdfs:label ,
		pigShapes_rdfs:comment ,
		pigShapes_pig:category ,
		pigShapes_pig:icon ,
		pigShapes_pig:SourceLink ,
		pigShapes_pig:TargetLink .

pig:Property
	rdf:type owl:DatatypeProperty ;
	rdfs:label "Property" ;
	rdfs:comment "A PIG meta-model item used for properties (aka attributes)." .

pigShapes_pig:Property
	rdf:type sh:PropertyShape ;
	sh:path pig:Property ;
	sh:datatype xs:anyType .

pig:icon
	rdfs:subPropertyOf pig:Property ;
	rdfs:label "has icon" ;
	rdfs:comment "Specifies an icon for a model element (entity or relationship)." .

pigShapes_pig:icon
	rdf:type sh:PropertyShape ;
	sh:path pig:icon ;
	sh:datatype xs:string ;
	sh:minCount "0" ;
	sh:maxCount "1" .

pig:category
	rdfs:subPropertyOf dcterms:type ;
	rdfs:label "has category" ;
	rdfs:comment "Specifies a category for an element (entity, relationship or organizer)." .

pigShapes_pig:category
	rdf:type sh:PropertyShape ;
	sh:path pig:category ;
	sh:datatype xs:string ;
	sh:maxLength "32" ;
	sh:minCount "0" ;
	sh:maxCount "1" .

pig:Link
	rdf:type owl:ObjectProperty ;
	rdfs:range [ owl:unionOf(
			pig:Entity
			pig:Relationship
		)] ;
	rdfs:label "linked with" ;
	rdfs:comment "A PIG meta-model item connecting a reified relationship with its source or target. Also connects an organizer to a model element" .

pigShapes_pig:Link
	rdf:type sh:PropertyShape ;
	sh:path pig:Link ;
	sh:or (
			[ sh:class pig:Entity ]
			[ sh:class pig:Relationship ]
		) .

pig:SourceLink
	rdfs:subPropertyOf pig:Link ;
	rdfs:range [ owl:unionOf(
			pig:Entity
			pig:Relationship
		)] ;
	rdfs:label "to source" ;
	rdfs:comment "Connects the source of a reified relationship." .

pigShapes_pig:SourceLink
	rdf:type sh:PropertyShape ;
	sh:path pig:SourceLink ;
	sh:or (
			[ sh:class pig:Entity ]
			[ sh:class pig:Relationship ]
		) .

pig:TargetLink
	rdfs:subPropertyOf pig:Link ;
	rdfs:range [ owl:unionOf(
			pig:Entity
			pig:Relationship
		)] ;
	rdfs:label "to target" ;
	rdfs:comment "Connects the target of a reified relationship or an organizer." .

pigShapes_pig:TargetLink
	rdf:type sh:PropertyShape ;
	sh:path pig:TargetLink ;
	sh:or (
			[ sh:class pig:Entity ]
			[ sh:class pig:Relationship ]
		) .

pig:lists
	rdfs:subPropertyOf pig:TargetLink ;
	rdfs:range [ owl:unionOf(
			pig:Entity
			pig:Relationship
			pig:Organizer
		)] ;
	rdfs:label "lists" ;
	rdfs:comment "Lists an entity, a relationship or a subordinated organizer." .

pigShapes_pig:lists
	rdf:type sh:PropertyShape ;
	sh:path pig:lists ;
	sh:or (
			[ sh:class pig:Entity ]
			[ sh:class pig:Relationship ]
			[ sh:class pig:Organizer ]
		) .

pig:shows
	rdfs:subPropertyOf pig:TargetLink ;
	rdfs:range [ owl:unionOf(
			pig:Entity
			pig:Relationship
		)] ;
	rdfs:label "shows" ;
	rdfs:comment "Shows an entity or a relationship." .

pigShapes_pig:shows
	rdf:type sh:PropertyShape ;
	sh:path pig:shows ;
	sh:or (
			[ sh:class pig:Entity ]
			[ sh:class pig:Relationship ]
		) .

pig:depicts
	rdfs:subPropertyOf pig:TargetLink ;
	rdfs:range pig:Entity ;
	rdfs:label "depicts" ;
	rdfs:comment "Depicts an entity; inverse of uml:ownedDiagram." .

pigShapes_pig:depicts
	rdf:type sh:PropertyShape ;
	sh:path pig:depicts ;
	sh:or (
			[ sh:class pig:Entity ]
		) .

#################################################################
# Classes
#################################################################

schema:Person
	rdfs:subClassOf pig:Entity ;
	rdfs:label "Person" ;
	rdfs:comment "A person (alive, dead, undead, or fictional)." .
	
pigShapes_schema:Person
	rdf:type sh:NodeShape ;
	sh:targetClass schema:Person ;
	sh:property pigShapes_rdfs:label ,
		pigShapes_rdfs:comment ,
		pigShapes_schema:familyName ,
		pigShapes_schema:givenName ,
		pigShapes_schema:birthDate .

schema:Organization
	rdfs:subClassOf pig:Entity ;
	rdfs:label "Organization" ;
	rdfs:comment "An organization such as a school, NGO, corporation, club, etc." .
	
pigShapes_schema:Organization
	rdf:type sh:NodeShape ;
	sh:targetClass schema:Organization ;
	sh:property pigShapes_rdfs:label ,
		pigShapes_rdfs:comment ,
		pigShapes_schema:legalName ,
		pigShapes_schema:taxID .

schema:birthDate
	rdfs:subPropertyOf pig:Property ;
	rdfs:label "birth date" ;
	rdfs:comment "Date of birth." .

pigShapes_schema:birthDate
	rdf:type sh:PropertyShape ;
	sh:path schema:birthDate ;
	sh:datatype xs:date ;
	sh:minCount "0" ;
	sh:maxCount "1" .

schema:familyName
	rdfs:subPropertyOf pig:Property ;
	rdfs:label "family name" ;
	rdfs:comment "Family name. In the U.S., the last name of a Person." .

pigShapes_schema:familyName
	rdf:type sh:PropertyShape ;
	sh:path schema:familyName ;
	sh:datatype xs:string ;
	sh:minCount "0" ;
	sh:maxCount "1" .

schema:givenName
	rdfs:subPropertyOf pig:Property ;
	rdfs:label "given name" ;
	rdfs:comment "Family name. In the U.S., the last name of a Person." .

pigShapes_schema:givenName
	rdf:type sh:PropertyShape ;
	sh:path schema:givenName ;
	sh:datatype xs:string ;
	sh:minCount "0" ;
	sh:maxCount "1" .

schema:legalName
	rdfs:subPropertyOf pig:Property ;
	rdfs:label "legal name" ;
	rdfs:comment "The official name of the organization, e.g. the registered company name." .

pigShapes_schema:legalName
	rdf:type sh:PropertyShape ;
	sh:path schema:legalName ;
	sh:datatype xs:string ;
	sh:minCount "0" ;
	sh:maxCount "1" .

schema:taxID
	rdfs:subPropertyOf pig:Property ;
	rdfs:label "tax ID" ;
	rdfs:comment "The Tax / Fiscal ID of the organization or person, e.g. the TIN in the US or the CIF/NIF in Spain." .

pigShapes_schema:taxID
	rdf:type sh:PropertyShape ;
	sh:path schema:taxID ;
	sh:datatype xs:string ;
	sh:minCount "0" ;
	sh:maxCount "1" .
	
schema:WorksFor
	rdfs:subClassOf pig:Relationship ;
	rdfs:label "works for" ;
	rdfs:comment "Organizations that the person works for." .

o:Employee
	rdfs:subPropertyOf pig:SourceLink ;
	rdfs:label "employee" ;
	rdfs:comment "The employee in a 'worksFor' relationship" ;
	rdfs:domain schema:WorksFor ;
	rdfs:range schema:Person .

o:Employer
	rdfs:subPropertyOf pig:TargetLink ;
	rdfs:label "employer" ;
	rdfs:comment "The employer in a 'worksFor' relationship" ;
	rdfs:domain schema:WorksFor ;
	rdfs:range schema:Organization .

pigShapes_schema:WorksFor
	rdf:type sh:NodeShape ;
	sh:targetClass schema:WorksFor ;
	sh:property pigShapes_rdfs:label ;
	sh:property pigShapes_rdfs:comment ;
	sh:property [ 
		sh:path o:Employee ;
		sh:or (
			[ sh:class schema:Person ]
		) ;
		sh:minCount 1 ;
		sh:maxCount 1
	] ;
	sh:property [ 
		sh:path o:Employer ;
		sh:or (
			[ sh:class schema:Organization ]
		) ;
		sh:minCount 1 ;
		sh:maxCount 1
	] .

#################################################################
# Individuals (the "payload")
#################################################################

d:ACME
	rdfs:label "ACME Corp." ;
	rdf:type schema:Organization ;
	schema:legalName "ACME Corp." ;
	schema:taxID "DE_123456789" .
	
d:Alice
	rdfs:label "Alice" ;
	rdf:type schema:Person ;
	schema:familyName "Carpenter" ;
	schema:givenName "Alice" .
	
d:Alice_worksFor_ACME
	rdf:type schema:WorksFor ;
	o:Employee d:Alice ;
	o:Employer d:ACME .
