
@prefix rdf: <http://www.w3.org/1999/02/22-rdf-syntax-ns#> .
@prefix rdfs: <http://www.w3.org/2000/01/rdf-schema#> .
@prefix owl: <http://www.w3.org/2002/07/owl#> .
@prefix sh: <https://www.w3.org/ns/shacl> .
@prefix W3C: <https://www.w3.org/standards/semanticweb#> .
@prefix dcterms: <http://purl.org/dc/terms/> .
@prefix pig: <https://product-information-graph.org/schema/#> .
@prefix DDP: <http://www.prostep.org/dictionary/2.0#> .
@prefix SpecIF: <https://specif.de/v1.1/schema#> .
@prefix sh: <http://www.w3.org/ns/shacl#> .

@prefix : <https://product-information-graph.org/examples/Dictionary.xsd#> .

#################################################################
# Project Metadata
#################################################################

:
	rdf:type owl:Ontology ;
	rdfs:label "Ontology as defined by prostep iViP DDP" ;
	rdfs:comment "Ontology derived from DDP Schema Version 2.0 created 10.03.2023 08:09:28 by Michael Kirsch, :em engineering methods AG on behalf of prostep iViP Association" ;
	owl:imports <http://www.w3.org/1999/02/22-rdf-syntax-ns#> ,
		<http://www.w3.org/2000/01/rdf-schema#> .

#################################################################
# Resource Classes
#################################################################

pig:EntityClass
	rdf:type owl:Class .

pig:Entity
	rdf:type owl:Class .
	
pig:itemType
	rdf:type owl:ObjectProperty ;
    rdfs:range 
		pig:OrganizerClass ,
		pig:Organizer ,
		pig:EntityClass ,
		pig:Entity ,
		pig:RelationshipClass ,
		pig:Relationship ,
		pig:PropertyClass ;
    rdfs:label "has PIG metamodel item type" .

DDP:Person 
	rdf:type owl:Class ;
    rdfs:subClassOf owl:Thing ;
	pig:itemType pig:EntityClass ;
	rdfs:label "Person" ;
	rdfs:comment "Represents a real person, but may also be a system user that appears in source data. The FOAF (Friend of a Friend) Ontology has been considered, but is not used as it does not provide a structured representation for firstname, lastname and title of a person." ;
	dcterms:modified "2025-07-25T13:51:29.486Z" .

DDP:Employee
	a owl:Class ;
    rdfs:subClassOf DDP:Person ;
	pig:itemType pig:EntityClass ;
	rdfs:label "Employee" ;
	dcterms:modified "2025-07-25T13:51:29.486Z" .

DDP:Role
	rdf:type owl:Class ;
    rdfs:subClassOf owl:Thing ;
	pig:itemType pig:EntityClass ;
	rdfs:label "Role" ;
	rdfs:comment "A defined function to be performed by a project team member, such as testing, filing, inspecting, coding.https://intranet.prostep.org/display/PROJ/Glossary" ;
	dcterms:modified "2025-07-25T13:51:29.486Z" .

DDP:OrganizationUnit
	a owl:Class ;
    rdfs:subClassOf owl:Thing ;
	pig:itemType pig:EntityClass ;
	rdfs:label "OrganizationUnit" ;
	rdfs:comment "An organization unit is part of a corporate structure. It comprises persons as well as sub-organization units." ;
	dcterms:modified "2025-07-25T13:51:29.486Z" .


#################################################################
# Resources
#################################################################

:R-q0Oh7DFaqgCY5RdaEQWAtBv1MNS
	rdf:type DDP:Employee ;
	pig:itemType pig:Entity ;
	DDP:firstname "Anouk" ;
	DDP:lastname "Aim√©e" ;
	DDP:phone "0033 12 345678" ;
	dcterms:modified "2025-07-25T13:55:57.846Z" .
